# baseURI: https://raw.githubusercontent.com/airs-linked-data/lov/latest/src/airs_vocabulary.ttl#
# imports: http://purl.org/dc/elements/1.1#
# imports: http://rdf.muninn-project.org/ontologies/appearances#
# imports: http://www.semanticdesktop.org/ontologies/2007/04/02/ncal#
# imports: http://www.w3.org/2006/vcard/ns#
# imports: http://www.w3.org/ns/org#

@prefix : <http://www.semanticweb.org/owl/owlapi/turtle#> .
@prefix airs: <https://raw.githubusercontent.com/airs-linked-data/lov/latest/src/airs_vocabulary.ttl#> .
@prefix appearances: <http://rdf.muninn-project.org/ontologies/appearances#> .
@prefix dc: <http://purl.org/dc/elements/1.1#> .
@prefix dcam: <http://purl.org/dc/dcam#> .
@prefix dct: <http://purl.org/dc/terms#> .
@prefix ncal: <http://www.semanticdesktop.org/ontologies/2007/04/02/ncal#> .
@prefix nrl: <http://www.semanticdesktop.org/ontologies/2007/08/15/nrl#> .
@prefix ogc: <http://www.opengis.net/rdf#> .
@prefix org: <http://www.w3.org/ns/org#> .
@prefix owl: <http://www.w3.org/2002/07/owl#> .
@prefix rdf: <http://www.w3.org/1999/02/22-rdf-syntax-ns#> .
@prefix rdfs: <http://www.w3.org/2000/01/rdf-schema#> .
@prefix skos: <http://www.w3.org/2004/02/skos/core#> .
@prefix vcard: <http://www.w3.org/2006/vcard/ns#> .
@prefix xhtm: <http://www.w3.org/1999/xhtml#> .
@prefix xml: <http://www.w3.org/XML/1998/namespace#> .
@prefix xsd: <http://www.w3.org/2001/XMLSchema#> .

<appearances:GenderStrict>
  rdf:type owl:Class ;
.
<http://purl.org/dc/aboutdcmi#DCMI>
  rdf:type owl:NamedIndividual ;
.
dcam:VocabularyEncodingScheme
  rdf:type owl:Class ;
.
<http://purl.org/dc/dcmitype/Collection>
  rdf:type owl:Class ;
.
dc:
  dct:modified "2012-06-14"^^xsd:date ;
  dct:publisher <http://purl.org/dc/aboutdcmi#DCMI> ;
  dct:title "Dublin Core Metadata Element Set, Version 1.1"@en ;
.
dc:contributor
  dct:description "Examples of a Contributor include a person, an organization, or a service. Typically, the name of a Contributor should be used to indicate the entity."@en ;
  dct:hasVersion <http://dublincore.org/usage/terms/history/#contributor-006> ;
  dct:issued "1999-07-02"^^xsd:date ;
  dct:modified "2008-01-14"^^xsd:date ;
  rdfs:comment "An entity responsible for making contributions to the resource."@en ;
  rdfs:isDefinedBy dc: ;
  rdfs:label "Contributor"@en ;
  skos:note "A second property with the same name as this property has been declared in the dcterms: namespace (http://purl.org/dc/terms/).  See the Introduction to the document \"DCMI Metadata Terms\" (http://dublincore.org/documents/dcmi-terms/) for an explanation."@en ;
.
dc:coverage
  dct:description "Spatial topic and spatial applicability may be a named place or a location specified by its geographic coordinates. Temporal topic may be a named period, date, or date range. A jurisdiction may be a named administrative entity or a geographic place to which the resource applies. Recommended best practice is to use a controlled vocabulary such as the Thesaurus of Geographic Names [TGN]. Where appropriate, named places or time periods can be used in preference to numeric identifiers such as sets of coordinates or date ranges."@en ;
  dct:hasVersion <http://dublincore.org/usage/terms/history/#coverage-006> ;
  dct:issued "1999-07-02"^^xsd:date ;
  dct:modified "2008-01-14"^^xsd:date ;
  rdfs:comment "The spatial or temporal topic of the resource, the spatial applicability of the resource, or the jurisdiction under which the resource is relevant."@en ;
  rdfs:isDefinedBy dc: ;
  rdfs:label "Coverage"@en ;
  skos:note "A second property with the same name as this property has been declared in the dcterms: namespace (http://purl.org/dc/terms/).  See the Introduction to the document \"DCMI Metadata Terms\" (http://dublincore.org/documents/dcmi-terms/) for an explanation."@en ;
.
dc:creator
  dct:description "Examples of a Creator include a person, an organization, or a service. Typically, the name of a Creator should be used to indicate the entity."@en ;
  dct:hasVersion <http://dublincore.org/usage/terms/history/#creator-006> ;
  dct:issued "1999-07-02"^^xsd:date ;
  dct:modified "2008-01-14"^^xsd:date ;
  rdfs:comment "An entity primarily responsible for making the resource."@en ;
  rdfs:isDefinedBy dc: ;
  rdfs:label "Creator"@en ;
  skos:note "A second property with the same name as this property has been declared in the dcterms: namespace (http://purl.org/dc/terms/).  See the Introduction to the document \"DCMI Metadata Terms\" (http://dublincore.org/documents/dcmi-terms/) for an explanation."@en ;
.
dc:date
  dct:description "Date may be used to express temporal information at any level of granularity.  Recommended best practice is to use an encoding scheme, such as the W3CDTF profile of ISO 8601 [W3CDTF]."@en ;
  dct:hasVersion <http://dublincore.org/usage/terms/history/#date-006> ;
  dct:issued "1999-07-02"^^xsd:date ;
  dct:modified "2008-01-14"^^xsd:date ;
  rdfs:comment "A point or period of time associated with an event in the lifecycle of the resource."@en ;
  rdfs:isDefinedBy dc: ;
  rdfs:label "Date"@en ;
  skos:note "A second property with the same name as this property has been declared in the dcterms: namespace (http://purl.org/dc/terms/).  See the Introduction to the document \"DCMI Metadata Terms\" (http://dublincore.org/documents/dcmi-terms/) for an explanation."@en ;
.
dc:description
  dct:description "Description may include but is not limited to: an abstract, a table of contents, a graphical representation, or a free-text account of the resource."@en ;
  dct:hasVersion <http://dublincore.org/usage/terms/history/#description-006> ;
  dct:issued "1999-07-02"^^xsd:date ;
  dct:modified "2008-01-14"^^xsd:date ;
  rdfs:comment "An account of the resource."@en ;
  rdfs:isDefinedBy dc: ;
  rdfs:label "Description"@en ;
  skos:note "A second property with the same name as this property has been declared in the dcterms: namespace (http://purl.org/dc/terms/).  See the Introduction to the document \"DCMI Metadata Terms\" (http://dublincore.org/documents/dcmi-terms/) for an explanation."@en ;
.
dc:format
  dct:description "Examples of dimensions include size and duration. Recommended best practice is to use a controlled vocabulary such as the list of Internet Media Types [MIME]."@en ;
  dct:hasVersion <http://dublincore.org/usage/terms/history/#format-007> ;
  dct:issued "1999-07-02"^^xsd:date ;
  dct:modified "2008-01-14"^^xsd:date ;
  rdfs:comment "The file format, physical medium, or dimensions of the resource."@en ;
  rdfs:isDefinedBy dc: ;
  rdfs:label "Format"@en ;
  skos:note "A second property with the same name as this property has been declared in the dcterms: namespace (http://purl.org/dc/terms/).  See the Introduction to the document \"DCMI Metadata Terms\" (http://dublincore.org/documents/dcmi-terms/) for an explanation."@en ;
.
dc:identifier
  dct:description "Recommended best practice is to identify the resource by means of a string conforming to a formal identification system. "@en ;
  dct:hasVersion <http://dublincore.org/usage/terms/history/#identifier-006> ;
  dct:issued "1999-07-02"^^xsd:date ;
  dct:modified "2008-01-14"^^xsd:date ;
  rdfs:comment "An unambiguous reference to the resource within a given context."@en ;
  rdfs:isDefinedBy dc: ;
  rdfs:label "Identifier"@en ;
  skos:note "A second property with the same name as this property has been declared in the dcterms: namespace (http://purl.org/dc/terms/).  See the Introduction to the document \"DCMI Metadata Terms\" (http://dublincore.org/documents/dcmi-terms/) for an explanation."@en ;
.
dc:language
  dct:description "Recommended best practice is to use a controlled vocabulary such as RFC 4646 [RFC4646]."@en ;
  dct:hasVersion <http://dublincore.org/usage/terms/history/#language-007> ;
  dct:issued "1999-07-02"^^xsd:date ;
  dct:modified "2008-01-14"^^xsd:date ;
  rdfs:comment "A language of the resource."@en ;
  rdfs:isDefinedBy dc: ;
  rdfs:label "Language"@en ;
  rdfs:seeAlso <http://www.ietf.org/rfc/rfc4646.txt> ;
  skos:note "A second property with the same name as this property has been declared in the dcterms: namespace (http://purl.org/dc/terms/).  See the Introduction to the document \"DCMI Metadata Terms\" (http://dublincore.org/documents/dcmi-terms/) for an explanation."@en ;
.
dc:publisher
  dct:description "Examples of a Publisher include a person, an organization, or a service. Typically, the name of a Publisher should be used to indicate the entity."@en ;
  dct:hasVersion <http://dublincore.org/usage/terms/history/#publisher-006> ;
  dct:issued "1999-07-02"^^xsd:date ;
  dct:modified "2008-01-14"^^xsd:date ;
  rdfs:comment "An entity responsible for making the resource available."@en ;
  rdfs:isDefinedBy dc: ;
  rdfs:label "Publisher"@en ;
  skos:note "A second property with the same name as this property has been declared in the dcterms: namespace (http://purl.org/dc/terms/).  See the Introduction to the document \"DCMI Metadata Terms\" (http://dublincore.org/documents/dcmi-terms/) for an explanation."@en ;
.
dc:relation
  dct:description "Recommended best practice is to identify the related resource by means of a string conforming to a formal identification system. "@en ;
  dct:hasVersion <http://dublincore.org/usage/terms/history/#relation-006> ;
  dct:issued "1999-07-02"^^xsd:date ;
  dct:modified "2008-01-14"^^xsd:date ;
  rdfs:comment "A related resource."@en ;
  rdfs:isDefinedBy dc: ;
  rdfs:label "Relation"@en ;
  skos:note "A second property with the same name as this property has been declared in the dcterms: namespace (http://purl.org/dc/terms/).  See the Introduction to the document \"DCMI Metadata Terms\" (http://dublincore.org/documents/dcmi-terms/) for an explanation."@en ;
.
dc:rights
  dct:description "Typically, rights information includes a statement about various property rights associated with the resource, including intellectual property rights."@en ;
  dct:hasVersion <http://dublincore.org/usage/terms/history/#rights-006> ;
  dct:issued "1999-07-02"^^xsd:date ;
  dct:modified "2008-01-14"^^xsd:date ;
  rdfs:comment "Information about rights held in and over the resource."@en ;
  rdfs:isDefinedBy dc: ;
  rdfs:label "Rights"@en ;
  skos:note "A second property with the same name as this property has been declared in the dcterms: namespace (http://purl.org/dc/terms/).  See the Introduction to the document \"DCMI Metadata Terms\" (http://dublincore.org/documents/dcmi-terms/) for an explanation."@en ;
.
dc:source
  dct:description "The described resource may be derived from the related resource in whole or in part. Recommended best practice is to identify the related resource by means of a string conforming to a formal identification system."@en ;
  dct:hasVersion <http://dublincore.org/usage/terms/history/#source-006> ;
  dct:issued "1999-07-02"^^xsd:date ;
  dct:modified "2008-01-14"^^xsd:date ;
  rdfs:comment "A related resource from which the described resource is derived."@en ;
  rdfs:isDefinedBy dc: ;
  rdfs:label "Source"@en ;
  skos:note "A second property with the same name as this property has been declared in the dcterms: namespace (http://purl.org/dc/terms/).  See the Introduction to the document \"DCMI Metadata Terms\" (http://dublincore.org/documents/dcmi-terms/) for an explanation."@en ;
.
dc:subject
  dct:description "Typically, the subject will be represented using keywords, key phrases, or classification codes. Recommended best practice is to use a controlled vocabulary."@en ;
  dct:hasVersion <http://dublincore.org/usage/terms/history/#subject-007> ;
  dct:issued "1999-07-02"^^xsd:date ;
  dct:modified "2012-06-14"^^xsd:date ;
  rdfs:comment "The topic of the resource."@en ;
  rdfs:isDefinedBy dc: ;
  rdfs:label "Subject"@en ;
  skos:note "A second property with the same name as this property has been declared in the dcterms: namespace (http://purl.org/dc/terms/).  See the Introduction to the document \"DCMI Metadata Terms\" (http://dublincore.org/documents/dcmi-terms/) for an explanation."@en ;
.
dc:title
  dct:hasVersion <http://dublincore.org/usage/terms/history/#title-006> ;
  dct:issued "1999-07-02"^^xsd:date ;
  dct:modified "2008-01-14"^^xsd:date ;
  rdfs:comment "A name given to the resource."@en ;
  rdfs:isDefinedBy dc: ;
  rdfs:label "Title"@en ;
  skos:note "A second property with the same name as this property has been declared in the dcterms: namespace (http://purl.org/dc/terms/).  See the Introduction to the document \"DCMI Metadata Terms\" (http://dublincore.org/documents/dcmi-terms/) for an explanation."@en ;
.
dc:type
  dct:description "Recommended best practice is to use a controlled vocabulary such as the DCMI Type Vocabulary [DCMITYPE]. To describe the file format, physical medium, or dimensions of the resource, use the Format element."@en ;
  dct:hasVersion <http://dublincore.org/usage/terms/history/#type-006> ;
  dct:issued "1999-07-02"^^xsd:date ;
  dct:modified "2008-01-14"^^xsd:date ;
  rdfs:comment "The nature or genre of the resource."@en ;
  rdfs:isDefinedBy dc: ;
  rdfs:label "Type"@en ;
  skos:note "A second property with the same name as this property has been declared in the dcterms: namespace (http://purl.org/dc/terms/).  See the Introduction to the document \"DCMI Metadata Terms\" (http://dublincore.org/documents/dcmi-terms/) for an explanation."@en ;
.
dct:
  rdf:type owl:NamedIndividual ;
  dct:modified "2012-06-14"^^xsd:date ;
  dct:publisher <http://purl.org/dc/aboutdcmi#DCMI> ;
  dct:title "DCMI Metadata Terms - other"@en ;
.
<http://purl.org/dc/terms#:description>
  rdf:type owl:Class ;
.
<http://purl.org/dc/terms#:identifier>
  rdf:type owl:Class ;
.
dct:Agent
  rdf:type dct:AgentClass ;
  rdf:type owl:Class ;
  rdf:type owl:NamedIndividual ;
  dct:description "Examples of Agent include person, organization, and software agent."@en ;
  dct:hasVersion <http://dublincore.org/usage/terms/history/#Agent-001> ;
  dct:issued "2008-01-14"^^xsd:date ;
  rdfs:comment "A resource that acts or has the power to act."@en ;
  rdfs:isDefinedBy dct: ;
  rdfs:label "Agent"@en ;
.
dct:AgentClass
  rdf:type owl:Class ;
  rdf:type owl:NamedIndividual ;
  dct:description "Examples of Agent Class include groups seen as classes, such as students, women, charities, lecturers."@en ;
  dct:hasVersion <http://dublincore.org/usage/terms/history/#AgentClass-003> ;
  dct:issued "2008-01-14"^^xsd:date ;
  dct:modified "2012-06-14"^^xsd:date ;
  rdfs:comment "A group of agents."@en ;
  rdfs:isDefinedBy dct: ;
  rdfs:label "Agent Class"@en ;
  rdfs:subClassOf rdfs:Class ;
.
dct:BibliographicResource
  rdf:type owl:Class ;
  rdf:type owl:NamedIndividual ;
  dct:hasVersion <http://dublincore.org/usage/terms/history/#BibliographicResource-001> ;
  dct:issued "2008-01-14"^^xsd:date ;
  rdfs:comment "A book, article, or other documentary resource."@en ;
  rdfs:isDefinedBy dct: ;
  rdfs:label "Bibliographic Resource"@en ;
.
dct:Box
  rdf:type rdfs:Datatype ;
  rdf:type owl:NamedIndividual ;
  dct:hasVersion <http://dublincore.org/usage/terms/history/#Box-003> ;
  dct:issued "2000-07-11"^^xsd:date ;
  dct:modified "2008-01-14"^^xsd:date ;
  rdfs:comment "The set of regions in space defined by their geographic coordinates according to the DCMI Box Encoding Scheme."@en ;
  rdfs:isDefinedBy dct: ;
  rdfs:label "DCMI Box"@en ;
  rdfs:seeAlso <http://dublincore.org/documents/dcmi-box/> ;
.
dct:DCMIType
  rdf:type dcam:VocabularyEncodingScheme ;
  rdf:type owl:NamedIndividual ;
  dct:hasVersion <http://dublincore.org/usage/terms/history/#DCMIType-005> ;
  dct:issued "2000-07-11"^^xsd:date ;
  dct:modified "2012-06-14"^^xsd:date ;
  rdfs:comment "The set of classes specified by the DCMI Type Vocabulary, used to categorize the nature or genre of the resource."@en ;
  rdfs:isDefinedBy dct: ;
  rdfs:label "DCMI Type Vocabulary"@en ;
  rdfs:seeAlso <http://purl.org/dc/dcmitype/> ;
.
dct:DDC
  rdf:type dcam:VocabularyEncodingScheme ;
  rdf:type owl:NamedIndividual ;
  dct:hasVersion <http://dublincore.org/usage/terms/history/#DDC-003> ;
  dct:issued "2000-07-11"^^xsd:date ;
  dct:modified "2008-01-14"^^xsd:date ;
  rdfs:comment "The set of conceptual resources specified by the Dewey Decimal Classification."@en ;
  rdfs:isDefinedBy dct: ;
  rdfs:label "DDC"@en ;
  rdfs:seeAlso <http://www.oclc.org/dewey/> ;
.
dct:FileFormat
  rdf:type owl:Class ;
  rdf:type owl:NamedIndividual ;
  dct:description "Examples include the formats defined by the list of Internet Media Types."@en ;
  dct:hasVersion <http://dublincore.org/usage/terms/history/#FileFormat-001> ;
  dct:issued "2008-01-14"^^xsd:date ;
  rdfs:comment "A digital resource format."@en ;
  rdfs:isDefinedBy dct: ;
  rdfs:label "File Format"@en ;
  rdfs:subClassOf dct:MediaType ;
.
dct:Frequency
  rdf:type owl:Class ;
  rdf:type owl:NamedIndividual ;
  dct:hasVersion <http://dublincore.org/usage/terms/history/#Frequency-001> ;
  dct:issued "2008-01-14"^^xsd:date ;
  rdfs:comment "A rate at which something recurs."@en ;
  rdfs:isDefinedBy dct: ;
  rdfs:label "Frequency"@en ;
.
dct:IMT
  rdf:type dcam:VocabularyEncodingScheme ;
  rdf:type owl:NamedIndividual ;
  dct:hasVersion <http://dublincore.org/usage/terms/history/#IMT-004> ;
  dct:issued "2000-07-11"^^xsd:date ;
  dct:modified "2008-01-14"^^xsd:date ;
  rdfs:comment "The set of media types specified by the Internet Assigned Numbers Authority."@en ;
  rdfs:isDefinedBy dct: ;
  rdfs:label "IMT"@en ;
  rdfs:seeAlso <http://www.iana.org/assignments/media-types/> ;
.
dct:ISO3166
  rdf:type rdfs:Datatype ;
  rdf:type owl:NamedIndividual ;
  dct:hasVersion <http://dublincore.org/usage/terms/history/#ISO3166-004> ;
  dct:issued "2000-07-11"^^xsd:date ;
  dct:modified "2008-01-14"^^xsd:date ;
  rdfs:comment "The set of codes listed in ISO 3166-1 for the representation of names of countries."@en ;
  rdfs:isDefinedBy dct: ;
  rdfs:label "ISO 3166"@en ;
  rdfs:seeAlso <http://www.iso.org/iso/en/prods-services/iso3166ma/02iso-3166-code-lists/list-en1.html> ;
.
dct:ISO639-2
  rdf:type rdfs:Datatype ;
  rdf:type owl:NamedIndividual ;
  dct:hasVersion <http://dublincore.org/usage/terms/history/#ISO639-2-003> ;
  dct:issued "2000-07-11"^^xsd:date ;
  dct:modified "2008-01-14"^^xsd:date ;
  rdfs:comment "The three-letter alphabetic codes listed in ISO639-2 for the representation of names of languages."@en ;
  rdfs:isDefinedBy dct: ;
  rdfs:label "ISO 639-2"@en ;
  rdfs:seeAlso <http://lcweb.loc.gov/standards/iso639-2/langhome.html> ;
.
dct:ISO639-3
  rdf:type rdfs:Datatype ;
  rdf:type owl:NamedIndividual ;
  dct:hasVersion <http://dublincore.org/usage/terms/history/#ISO639-3-001> ;
  dct:issued "2008-01-14"^^xsd:date ;
  rdfs:comment "The set of three-letter codes listed in ISO 639-3 for the representation of names of languages."@en ;
  rdfs:isDefinedBy dct: ;
  rdfs:label "ISO 639-3"@en ;
  rdfs:seeAlso <http://www.sil.org/iso639-3/> ;
.
dct:Jurisdiction
  rdf:type owl:Class ;
  rdf:type owl:NamedIndividual ;
  dct:hasVersion <http://dublincore.org/usage/terms/history/#Jurisdiction-001> ;
  dct:issued "2008-01-14"^^xsd:date ;
  rdfs:comment "The extent or range of judicial, law enforcement, or other authority."@en ;
  rdfs:isDefinedBy dct: ;
  rdfs:label "Jurisdiction"@en ;
  rdfs:subClassOf dct:LocationPeriodOrJurisdiction ;
.
dct:LCC
  rdf:type dcam:VocabularyEncodingScheme ;
  rdf:type owl:NamedIndividual ;
  dct:hasVersion <http://dublincore.org/usage/terms/history/#LCC-003> ;
  dct:issued "2000-07-11"^^xsd:date ;
  dct:modified "2008-01-14"^^xsd:date ;
  rdfs:comment "The set of conceptual resources specified by the Library of Congress Classification."@en ;
  rdfs:isDefinedBy dct: ;
  rdfs:label "LCC"@en ;
  rdfs:seeAlso <http://lcweb.loc.gov/catdir/cpso/lcco/lcco.html> ;
.
dct:LCSH
  rdf:type dcam:VocabularyEncodingScheme ;
  rdf:type owl:NamedIndividual ;
  dct:hasVersion <http://dublincore.org/usage/terms/history/#LCSH-003> ;
  dct:issued "2000-07-11"^^xsd:date ;
  dct:modified "2008-01-14"^^xsd:date ;
  rdfs:comment "The set of labeled concepts specified by the Library of Congress Subject Headings."@en ;
  rdfs:isDefinedBy dct: ;
  rdfs:label "LCSH"@en ;
.
dct:LicenseDocument
  rdf:type owl:Class ;
  rdf:type owl:NamedIndividual ;
  dct:hasVersion <http://dublincore.org/usage/terms/history/#LicenseDocument-001> ;
  dct:issued "2008-01-14"^^xsd:date ;
  rdfs:comment "A legal document giving official permission to do something with a Resource."@en ;
  rdfs:isDefinedBy dct: ;
  rdfs:label "License Document"@en ;
  rdfs:subClassOf dct:RightsStatement ;
.
dct:LinguisticSystem
  rdf:type owl:Class ;
  rdf:type owl:NamedIndividual ;
  dct:description "Examples include written, spoken, sign, and computer languages."@en ;
  dct:hasVersion <http://dublincore.org/usage/terms/history/#LinguisticSystem-001> ;
  dct:issued "2008-01-14"^^xsd:date ;
  rdfs:comment "A system of signs, symbols, sounds, gestures, or rules used in communication."@en ;
  rdfs:isDefinedBy dct: ;
  rdfs:label "Linguistic System"@en ;
.
dct:Location
  rdf:type owl:Class ;
  rdf:type owl:NamedIndividual ;
  dct:hasVersion <http://dublincore.org/usage/terms/history/#Location-001> ;
  dct:issued "2008-01-14"^^xsd:date ;
  rdfs:comment "A spatial region or named place."@en ;
  rdfs:isDefinedBy dct: ;
  rdfs:label "Location"@en ;
  rdfs:subClassOf dct:LocationPeriodOrJurisdiction ;
.
dct:LocationPeriodOrJurisdiction
  rdf:type owl:Class ;
  rdf:type owl:NamedIndividual ;
  dct:hasVersion <http://dublincore.org/usage/terms/history/#LocationPeriodOrJurisdiction-001> ;
  dct:issued "2008-01-14"^^xsd:date ;
  rdfs:comment "A location, period of time, or jurisdiction."@en ;
  rdfs:isDefinedBy dct: ;
  rdfs:label "Location, Period, or Jurisdiction"@en ;
.
dct:Location_1
  rdf:type dct:Location ;
.
dct:MESH
  rdf:type dcam:VocabularyEncodingScheme ;
  rdf:type owl:NamedIndividual ;
  dct:hasVersion <http://dublincore.org/usage/terms/history/#MESH-003> ;
  dct:issued "2000-07-11"^^xsd:date ;
  dct:modified "2008-01-14"^^xsd:date ;
  rdfs:comment "The set of labeled concepts specified by the Medical Subject Headings."@en ;
  rdfs:isDefinedBy dct: ;
  rdfs:label "MeSH"@en ;
  rdfs:seeAlso <http://www.nlm.nih.gov/mesh/meshhome.html> ;
.
dct:MediaType
  rdf:type owl:Class ;
  rdf:type owl:NamedIndividual ;
  dct:hasVersion <http://dublincore.org/usage/terms/history/#MediaType-001> ;
  dct:issued "2008-01-14"^^xsd:date ;
  rdfs:comment "A file format or physical medium."@en ;
  rdfs:isDefinedBy dct: ;
  rdfs:label "Media Type"@en ;
  rdfs:subClassOf dct:MediaTypeOrExtent ;
.
dct:MediaTypeOrExtent
  rdf:type owl:Class ;
  rdf:type owl:NamedIndividual ;
  dct:hasVersion <http://dublincore.org/usage/terms/history/#MediaTypeOrExtent-001> ;
  dct:issued "2008-01-14"^^xsd:date ;
  rdfs:comment "A media type or extent."@en ;
  rdfs:isDefinedBy dct: ;
  rdfs:label "Media Type or Extent"@en ;
.
dct:MethodOfAccrual
  rdf:type owl:Class ;
  rdf:type owl:NamedIndividual ;
  dct:hasVersion <http://dublincore.org/usage/terms/history/#MethodOfAccrual-001> ;
  dct:issued "2008-01-14"^^xsd:date ;
  rdfs:comment "A method by which resources are added to a collection."@en ;
  rdfs:isDefinedBy dct: ;
  rdfs:label "Method of Accrual"@en ;
.
dct:MethodOfInstruction
  rdf:type owl:Class ;
  rdf:type owl:NamedIndividual ;
  dct:hasVersion <http://dublincore.org/usage/terms/history/#MethodOfInstruction-001> ;
  dct:issued "2008-01-14"^^xsd:date ;
  rdfs:comment "A process that is used to engender knowledge, attitudes, and skills."@en ;
  rdfs:isDefinedBy dct: ;
  rdfs:label "Method of Instruction"@en ;
.
dct:NLM
  rdf:type dcam:VocabularyEncodingScheme ;
  rdf:type owl:NamedIndividual ;
  dct:hasVersion <http://dublincore.org/usage/terms/history/#NLM-002> ;
  dct:issued "2005-06-13"^^xsd:date ;
  dct:modified "2008-01-14"^^xsd:date ;
  rdfs:comment "The set of conceptual resources specified by the National Library of Medicine Classification."@en ;
  rdfs:isDefinedBy dct: ;
  rdfs:label "NLM"@en ;
  rdfs:seeAlso <http://wwwcf.nlm.nih.gov/class/> ;
.
dct:Period
  rdf:type rdfs:Datatype ;
  rdf:type owl:NamedIndividual ;
  dct:hasVersion <http://dublincore.org/usage/terms/history/#Period-003> ;
  dct:issued "2000-07-11"^^xsd:date ;
  dct:modified "2008-01-14"^^xsd:date ;
  rdfs:comment "The set of time intervals defined by their limits according to the DCMI Period Encoding Scheme."@en ;
  rdfs:isDefinedBy dct: ;
  rdfs:label "DCMI Period"@en ;
  rdfs:seeAlso <http://dublincore.org/documents/dcmi-period/> ;
.
dct:PeriodOfTime
  rdf:type owl:Class ;
  rdf:type owl:NamedIndividual ;
  dct:hasVersion <http://dublincore.org/usage/terms/history/#PeriodOfTime-001> ;
  dct:issued "2008-01-14"^^xsd:date ;
  rdfs:comment "An interval of time that is named or defined by its start and end dates."@en ;
  rdfs:isDefinedBy dct: ;
  rdfs:label "Period of Time"@en ;
  rdfs:subClassOf dct:LocationPeriodOrJurisdiction ;
.
dct:PhysicalMedium
  rdf:type owl:Class ;
  rdf:type owl:NamedIndividual ;
  dct:description "Examples include paper, canvas, or DVD."@en ;
  dct:hasVersion <http://dublincore.org/usage/terms/history/#PhysicalMedium-001> ;
  dct:issued "2008-01-14"^^xsd:date ;
  rdfs:comment "A physical material or carrier."@en ;
  rdfs:isDefinedBy dct: ;
  rdfs:label "Physical Medium"@en ;
  rdfs:subClassOf dct:MediaType ;
.
dct:PhysicalResource
  rdf:type owl:Class ;
  rdf:type owl:NamedIndividual ;
  dct:hasVersion <http://dublincore.org/usage/terms/history/#PhysicalResource-001> ;
  dct:issued "2008-01-14"^^xsd:date ;
  rdfs:comment "A material thing."@en ;
  rdfs:isDefinedBy dct: ;
  rdfs:label "Physical Resource"@en ;
.
dct:Point
  rdf:type rdfs:Datatype ;
  rdf:type owl:NamedIndividual ;
  dct:hasVersion <http://dublincore.org/usage/terms/history/#Point-003> ;
  dct:issued "2000-07-11"^^xsd:date ;
  dct:modified "2008-01-14"^^xsd:date ;
  rdfs:comment "The set of points in space defined by their geographic coordinates according to the DCMI Point Encoding Scheme."@en ;
  rdfs:isDefinedBy dct: ;
  rdfs:label "DCMI Point"@en ;
  rdfs:seeAlso <http://dublincore.org/documents/dcmi-point/> ;
.
dct:Policy
  rdf:type owl:Class ;
  rdf:type owl:NamedIndividual ;
  dct:hasVersion <http://dublincore.org/usage/terms/history/#Policy-001> ;
  dct:issued "2008-01-14"^^xsd:date ;
  rdfs:comment "A plan or course of action by an authority, intended to influence and determine decisions, actions, and other matters."@en ;
  rdfs:isDefinedBy dct: ;
  rdfs:label "Policy"@en ;
.
dct:ProvenanceStatement
  rdf:type owl:Class ;
  rdf:type owl:NamedIndividual ;
  dct:hasVersion <http://dublincore.org/usage/terms/history/#ProvenanceStatement-001> ;
  dct:issued "2008-01-14"^^xsd:date ;
  rdfs:comment "A statement of any changes in ownership and custody of a resource since its creation that are significant for its authenticity, integrity, and interpretation."@en ;
  rdfs:isDefinedBy dct: ;
  rdfs:label "Provenance Statement"@en ;
.
dct:RFC1766
  rdf:type rdfs:Datatype ;
  rdf:type owl:NamedIndividual ;
  dct:hasVersion <http://dublincore.org/usage/terms/history/#RFC1766-003> ;
  dct:issued "2000-07-11"^^xsd:date ;
  dct:modified "2008-01-14"^^xsd:date ;
  rdfs:comment "The set of tags, constructed according to RFC 1766, for the identification of languages."@en ;
  rdfs:isDefinedBy dct: ;
  rdfs:label "RFC 1766"@en ;
  rdfs:seeAlso <http://www.ietf.org/rfc/rfc1766.txt> ;
.
dct:RFC3066
  rdf:type rdfs:Datatype ;
  rdf:type owl:NamedIndividual ;
  dct:description "RFC 3066 has been obsoleted by RFC 4646."@en ;
  dct:hasVersion <http://dublincore.org/usage/terms/history/#RFC3066-002> ;
  dct:issued "2002-07-13"^^xsd:date ;
  dct:modified "2008-01-14"^^xsd:date ;
  rdfs:comment "The set of tags constructed according to RFC 3066 for the identification of languages."@en ;
  rdfs:isDefinedBy dct: ;
  rdfs:label "RFC 3066"@en ;
  rdfs:seeAlso <http://www.ietf.org/rfc/rfc3066.txt> ;
.
dct:RFC4646
  rdf:type rdfs:Datatype ;
  rdf:type owl:NamedIndividual ;
  dct:description "RFC 4646 obsoletes RFC 3066."@en ;
  dct:hasVersion <http://dublincore.org/usage/terms/history/#RFC4646-001> ;
  dct:issued "2008-01-14"^^xsd:date ;
  rdfs:comment "The set of tags constructed according to RFC 4646 for the identification of languages."@en ;
  rdfs:isDefinedBy dct: ;
  rdfs:label "RFC 4646"@en ;
  rdfs:seeAlso <http://www.ietf.org/rfc/rfc4646.txt> ;
.
dct:RFC5646
  rdf:type rdfs:Datatype ;
  rdf:type owl:NamedIndividual ;
  dct:description "RFC 5646 obsoletes RFC 4646."@en ;
  dct:hasVersion <http://dublincore.org/usage/terms/history/#RFC5646-001> ;
  dct:issued "2010-10-11"^^xsd:date ;
  rdfs:comment "The set of tags constructed according to RFC 5646 for the identification of languages."@en ;
  rdfs:isDefinedBy dct: ;
  rdfs:label "RFC 5646"@en ;
  rdfs:seeAlso <http://www.ietf.org/rfc/rfc5646.txt> ;
.
dct:RightsStatement
  rdf:type owl:Class ;
  rdf:type owl:NamedIndividual ;
  dct:hasVersion <http://dublincore.org/usage/terms/history/#RightsStatement-001> ;
  dct:issued "2008-01-14"^^xsd:date ;
  rdfs:comment "A statement about the intellectual property rights (IPR) held in or over a Resource, a legal document giving official permission to do something with a resource, or a statement about access rights."@en ;
  rdfs:isDefinedBy dct: ;
  rdfs:label "Rights Statement"@en ;
.
dct:SizeOrDuration
  rdf:type owl:Class ;
  rdf:type owl:NamedIndividual ;
  dct:description "Examples include a number of pages, a specification of length, width, and breadth, or a period in hours, minutes, and seconds."@en ;
  dct:hasVersion <http://dublincore.org/usage/terms/history/#SizeOrDuration-001> ;
  dct:issued "2008-01-14"^^xsd:date ;
  rdfs:comment "A dimension or extent, or a time taken to play or execute."@en ;
  rdfs:isDefinedBy dct: ;
  rdfs:label "Size or Duration"@en ;
  rdfs:subClassOf dct:MediaTypeOrExtent ;
.
dct:Standard
  rdf:type owl:Class ;
  rdf:type owl:NamedIndividual ;
  dct:hasVersion <http://dublincore.org/usage/terms/history/#Standard-001> ;
  dct:issued "2008-01-14"^^xsd:date ;
  rdfs:comment "A basis for comparison; a reference point against which other things can be evaluated."@en ;
  rdfs:isDefinedBy dct: ;
  rdfs:label "Standard"@en ;
.
dct:TGN
  rdf:type dcam:VocabularyEncodingScheme ;
  rdf:type owl:NamedIndividual ;
  dct:hasVersion <http://dublincore.org/usage/terms/history/#TGN-003> ;
  dct:issued "2000-07-11"^^xsd:date ;
  dct:modified "2008-01-14"^^xsd:date ;
  rdfs:comment "The set of places specified by the Getty Thesaurus of Geographic Names."@en ;
  rdfs:isDefinedBy dct: ;
  rdfs:label "TGN"@en ;
  rdfs:seeAlso <http://www.getty.edu/research/tools/vocabulary/tgn/index.html> ;
.
dct:UDC
  rdf:type dcam:VocabularyEncodingScheme ;
  rdf:type owl:NamedIndividual ;
  dct:hasVersion <http://dublincore.org/usage/terms/history/#UDC-003> ;
  dct:issued "2000-07-11"^^xsd:date ;
  dct:modified "2008-01-14"^^xsd:date ;
  rdfs:comment "The set of conceptual resources specified by the Universal Decimal Classification."@en ;
  rdfs:isDefinedBy dct: ;
  rdfs:label "UDC"@en ;
  rdfs:seeAlso <http://www.udcc.org/> ;
.
dct:URI
  rdf:type rdfs:Datatype ;
  rdf:type owl:NamedIndividual ;
  dct:hasVersion <http://dublincore.org/usage/terms/history/#URI-003> ;
  dct:issued "2000-07-11"^^xsd:date ;
  dct:modified "2008-01-14"^^xsd:date ;
  rdfs:comment "The set of identifiers constructed according to the generic syntax for Uniform Resource Identifiers as specified by the Internet Engineering Task Force."@en ;
  rdfs:isDefinedBy dct: ;
  rdfs:label "URI"@en ;
  rdfs:seeAlso <http://www.ietf.org/rfc/rfc3986.txt> ;
.
dct:W3CDTF
  rdf:type rdfs:Datatype ;
  rdf:type owl:NamedIndividual ;
  dct:hasVersion <http://dublincore.org/usage/terms/history/#W3CDTF-003> ;
  dct:issued "2000-07-11"^^xsd:date ;
  dct:modified "2008-01-14"^^xsd:date ;
  rdfs:comment "The set of dates and times constructed according to the W3C Date and Time Formats Specification."@en ;
  rdfs:isDefinedBy dct: ;
  rdfs:label "W3C-DTF"@en ;
  rdfs:seeAlso <http://www.w3.org/TR/NOTE-datetime> ;
.
dct:abstract
  rdf:type owl:AnnotationProperty ;
  rdf:type owl:NamedIndividual ;
  dct:hasVersion <http://dublincore.org/usage/terms/history/#abstract-003> ;
  dct:issued "2000-07-11"^^xsd:date ;
  dct:modified "2008-01-14"^^xsd:date ;
  rdfs:comment "A summary of the resource."@en ;
  rdfs:isDefinedBy dct: ;
  rdfs:label "Abstract"@en ;
  rdfs:subPropertyOf dc:description ;
  rdfs:subPropertyOf dct:description ;
.
dct:accessRights
  rdf:type owl:AnnotationProperty ;
  rdf:type owl:NamedIndividual ;
  rdf:type owl:ObjectProperty ;
  dct:description "Access Rights may include information regarding access or restrictions based on privacy, security, or other policies."@en ;
  dct:hasVersion <http://dublincore.org/usage/terms/history/#accessRights-002> ;
  dct:issued "2003-02-15"^^xsd:date ;
  dct:modified "2008-01-14"^^xsd:date ;
  rdfs:comment "Information about who can access the resource or an indication of its security status."@en ;
  rdfs:isDefinedBy dct: ;
  rdfs:label "Access Rights"@en ;
  rdfs:range dct:RightsStatement ;
  rdfs:subPropertyOf dc:rights ;
  rdfs:subPropertyOf dct:rights ;
.
dct:accrualMethod
  rdf:type owl:NamedIndividual ;
  rdf:type owl:ObjectProperty ;
  dct:hasVersion <http://dublincore.org/usage/terms/history/#accrualMethod-003> ;
  dct:issued "2005-06-13"^^xsd:date ;
  dct:modified "2010-10-11"^^xsd:date ;
  rdfs:comment "The method by which items are added to a collection."@en ;
  rdfs:domain <http://purl.org/dc/dcmitype/Collection> ;
  rdfs:isDefinedBy dct: ;
  rdfs:label "Accrual Method"@en ;
  rdfs:range dct:MethodOfAccrual ;
.
dct:accrualPeriodicity
  rdf:type owl:NamedIndividual ;
  rdf:type owl:ObjectProperty ;
  dct:hasVersion <http://dublincore.org/usage/terms/history/#accrualPeriodicity-003> ;
  dct:issued "2005-06-13"^^xsd:date ;
  dct:modified "2010-10-11"^^xsd:date ;
  rdfs:comment "The frequency with which items are added to a collection."@en ;
  rdfs:domain <http://purl.org/dc/dcmitype/Collection> ;
  rdfs:isDefinedBy dct: ;
  rdfs:label "Accrual Periodicity"@en ;
  rdfs:range dct:Frequency ;
.
dct:accrualPolicy
  rdf:type owl:NamedIndividual ;
  rdf:type owl:ObjectProperty ;
  dct:hasVersion <http://dublincore.org/usage/terms/history/#accrualPolicy-003> ;
  dct:issued "2005-06-13"^^xsd:date ;
  dct:modified "2010-10-11"^^xsd:date ;
  rdfs:comment "The policy governing the addition of items to a collection."@en ;
  rdfs:domain <http://purl.org/dc/dcmitype/Collection> ;
  rdfs:isDefinedBy dct: ;
  rdfs:label "Accrual Policy"@en ;
  rdfs:range dct:Policy ;
.
dct:alternative
  rdf:type owl:AnnotationProperty ;
  rdf:type owl:DatatypeProperty ;
  rdf:type owl:NamedIndividual ;
  dct:description "The distinction between titles and alternative titles is application-specific."@en ;
  dct:hasVersion <http://dublincore.org/usage/terms/history/#alternative-003> ;
  dct:issued "2000-07-11"^^xsd:date ;
  dct:modified "2010-10-11"^^xsd:date ;
  rdfs:comment "An alternative name for the resource."@en ;
  rdfs:isDefinedBy dct: ;
  rdfs:label "Alternative Title"@en ;
  rdfs:range rdfs:Literal ;
  rdfs:subPropertyOf dc:title ;
  rdfs:subPropertyOf dct:title ;
.
dct:audience
  rdf:type owl:NamedIndividual ;
  rdf:type owl:ObjectProperty ;
  dct:hasVersion <http://dublincore.org/usage/terms/history/#audience-003> ;
  dct:issued "2001-05-21"^^xsd:date ;
  dct:modified "2008-01-14"^^xsd:date ;
  rdfs:comment "A class of entity for whom the resource is intended or useful."@en ;
  rdfs:isDefinedBy dct: ;
  rdfs:label "Audience"@en ;
  rdfs:range dct:AgentClass ;
.
dct:available
  rdf:type owl:AnnotationProperty ;
  rdf:type owl:DatatypeProperty ;
  rdf:type owl:NamedIndividual ;
  dct:hasVersion <http://dublincore.org/usage/terms/history/#available-003> ;
  dct:issued "2000-07-11"^^xsd:date ;
  dct:modified "2008-01-14"^^xsd:date ;
  rdfs:comment "Date (often a range) that the resource became or will become available."@en ;
  rdfs:isDefinedBy dct: ;
  rdfs:label "Date Available"@en ;
  rdfs:range rdfs:Literal ;
  rdfs:subPropertyOf dc:date ;
  rdfs:subPropertyOf dct:date ;
.
dct:bibliographicCitation
  rdf:type owl:AnnotationProperty ;
  rdf:type owl:DatatypeProperty ;
  rdf:type owl:NamedIndividual ;
  dct:description "Recommended practice is to include sufficient bibliographic detail to identify the resource as unambiguously as possible."@en ;
  dct:hasVersion <http://dublincore.org/usage/terms/history/#bibliographicCitation-002> ;
  dct:issued "2003-02-15"^^xsd:date ;
  dct:modified "2008-01-14"^^xsd:date ;
  rdfs:comment "A bibliographic reference for the resource."@en ;
  rdfs:domain dct:BibliographicResource ;
  rdfs:isDefinedBy dct: ;
  rdfs:label "Bibliographic Citation"@en ;
  rdfs:range rdfs:Literal ;
  rdfs:subPropertyOf dc:identifier ;
  rdfs:subPropertyOf dct:identifier ;
.
dct:conformsTo
  rdf:type owl:AnnotationProperty ;
  rdf:type owl:NamedIndividual ;
  rdf:type owl:ObjectProperty ;
  dct:hasVersion <http://dublincore.org/usage/terms/history/#conformsTo-003> ;
  dct:issued "2001-05-21"^^xsd:date ;
  dct:modified "2008-01-14"^^xsd:date ;
  rdfs:comment "An established standard to which the described resource conforms."@en ;
  rdfs:isDefinedBy dct: ;
  rdfs:label "Conforms To"@en ;
  rdfs:range dct:Standard ;
  rdfs:subPropertyOf dc:relation ;
  rdfs:subPropertyOf dct:relation ;
.
dct:contributor
  rdf:type owl:AnnotationProperty ;
  rdf:type owl:NamedIndividual ;
  rdf:type owl:ObjectProperty ;
  dct:description "Examples of a Contributor include a person, an organization, or a service."@en ;
  dct:hasVersion <http://dublincore.org/usage/terms/history/#contributorT-001> ;
  dct:issued "2008-01-14"^^xsd:date ;
  dct:modified "2010-10-11"^^xsd:date ;
  rdfs:comment "An entity responsible for making contributions to the resource."@en ;
  rdfs:isDefinedBy dct: ;
  rdfs:label "Contributor"@en ;
  rdfs:range dct:Agent ;
  rdfs:subPropertyOf dc:contributor ;
.
dct:coverage
  rdf:type owl:AnnotationProperty ;
  rdf:type owl:NamedIndividual ;
  rdf:type owl:ObjectProperty ;
  dct:description "Spatial topic and spatial applicability may be a named place or a location specified by its geographic coordinates. Temporal topic may be a named period, date, or date range. A jurisdiction may be a named administrative entity or a geographic place to which the resource applies. Recommended best practice is to use a controlled vocabulary such as the Thesaurus of Geographic Names [TGN]. Where appropriate, named places or time periods can be used in preference to numeric identifiers such as sets of coordinates or date ranges."@en ;
  dct:hasVersion <http://dublincore.org/usage/terms/history/#coverageT-001> ;
  dct:issued "2008-01-14"^^xsd:date ;
  dct:modified "2008-01-14"^^xsd:date ;
  rdfs:comment "The spatial or temporal topic of the resource, the spatial applicability of the resource, or the jurisdiction under which the resource is relevant."@en ;
  rdfs:isDefinedBy dct: ;
  rdfs:label "Coverage"@en ;
  rdfs:range dct:LocationPeriodOrJurisdiction ;
  rdfs:subPropertyOf dc:coverage ;
.
dct:created
  rdf:type owl:AnnotationProperty ;
  rdf:type owl:DatatypeProperty ;
  rdf:type owl:NamedIndividual ;
  dct:hasVersion <http://dublincore.org/usage/terms/history/#created-003> ;
  dct:issued "2000-07-11"^^xsd:date ;
  dct:modified "2008-01-14"^^xsd:date ;
  rdfs:comment "Date of creation of the resource."@en ;
  rdfs:isDefinedBy dct: ;
  rdfs:label "Date Created"@en ;
  rdfs:range rdfs:Literal ;
  rdfs:subPropertyOf dc:date ;
  rdfs:subPropertyOf dct:date ;
.
dct:creator
  rdf:type owl:AnnotationProperty ;
  rdf:type owl:NamedIndividual ;
  rdf:type owl:ObjectProperty ;
  dct:description "Examples of a Creator include a person, an organization, or a service."@en ;
  dct:hasVersion <http://dublincore.org/usage/terms/history/#creatorT-002> ;
  dct:issued "2008-01-14"^^xsd:date ;
  dct:modified "2010-10-11"^^xsd:date ;
  rdfs:comment "An entity primarily responsible for making the resource."@en ;
  rdfs:isDefinedBy dct: ;
  rdfs:label "Creator"@en ;
  rdfs:range dct:Agent ;
  rdfs:subPropertyOf dc:creator ;
  rdfs:subPropertyOf dct:contributor ;
.
dct:date
  rdf:type owl:AnnotationProperty ;
  rdf:type owl:DatatypeProperty ;
  rdf:type owl:NamedIndividual ;
  dct:description "Date may be used to express temporal information at any level of granularity.  Recommended best practice is to use an encoding scheme, such as the W3CDTF profile of ISO 8601 [W3CDTF]."@en ;
  dct:hasVersion <http://dublincore.org/usage/terms/history/#dateT-001> ;
  dct:issued "2008-01-14"^^xsd:date ;
  dct:modified "2008-01-14"^^xsd:date ;
  rdfs:comment "A point or period of time associated with an event in the lifecycle of the resource."@en ;
  rdfs:isDefinedBy dct: ;
  rdfs:label "Date"@en ;
  rdfs:range rdfs:Literal ;
  rdfs:subPropertyOf dc:date ;
.
dct:dateAccepted
  rdf:type owl:AnnotationProperty ;
  rdf:type owl:DatatypeProperty ;
  rdf:type owl:NamedIndividual ;
  dct:description "Examples of resources to which a Date Accepted may be relevant are a thesis (accepted by a university department) or an article (accepted by a journal)."@en ;
  dct:hasVersion <http://dublincore.org/usage/terms/history/#dateAccepted-002> ;
  dct:issued "2002-07-13"^^xsd:date ;
  dct:modified "2008-01-14"^^xsd:date ;
  rdfs:comment "Date of acceptance of the resource."@en ;
  rdfs:isDefinedBy dct: ;
  rdfs:label "Date Accepted"@en ;
  rdfs:range rdfs:Literal ;
  rdfs:subPropertyOf dc:date ;
  rdfs:subPropertyOf dct:date ;
.
dct:dateCopyrighted
  rdf:type owl:AnnotationProperty ;
  rdf:type owl:DatatypeProperty ;
  rdf:type owl:NamedIndividual ;
  dct:hasVersion <http://dublincore.org/usage/terms/history/#dateCopyrighted-002> ;
  dct:issued "2002-07-13"^^xsd:date ;
  dct:modified "2008-01-14"^^xsd:date ;
  rdfs:comment "Date of copyright."@en ;
  rdfs:isDefinedBy dct: ;
  rdfs:label "Date Copyrighted"@en ;
  rdfs:range rdfs:Literal ;
  rdfs:subPropertyOf dc:date ;
  rdfs:subPropertyOf dct:date ;
.
dct:dateSubmitted
  rdf:type owl:AnnotationProperty ;
  rdf:type owl:DatatypeProperty ;
  rdf:type owl:NamedIndividual ;
  dct:description "Examples of resources to which a Date Submitted may be relevant are a thesis (submitted to a university department) or an article (submitted to a journal)."@en ;
  dct:hasVersion <http://dublincore.org/usage/terms/history/#dateSubmitted-002> ;
  dct:issued "2002-07-13"^^xsd:date ;
  dct:modified "2008-01-14"^^xsd:date ;
  rdfs:comment "Date of submission of the resource."@en ;
  rdfs:isDefinedBy dct: ;
  rdfs:label "Date Submitted"@en ;
  rdfs:range rdfs:Literal ;
  rdfs:subPropertyOf dc:date ;
  rdfs:subPropertyOf dct:date ;
.
dct:description
  rdf:type owl:AnnotationProperty ;
  rdf:type owl:NamedIndividual ;
  dct:description "Description may include but is not limited to: an abstract, a table of contents, a graphical representation, or a free-text account of the resource."@en ;
  dct:hasVersion <http://dublincore.org/usage/terms/history/#descriptionT-001> ;
  dct:issued "2008-01-14"^^xsd:date ;
  dct:modified "2008-01-14"^^xsd:date ;
  rdfs:comment "An account of the resource."@en ;
  rdfs:isDefinedBy dct: ;
  rdfs:label "Description"@en ;
  rdfs:subPropertyOf dc:description ;
.
dct:educationLevel
  rdf:type owl:NamedIndividual ;
  rdf:type owl:ObjectProperty ;
  dct:hasVersion <http://dublincore.org/usage/terms/history/#educationLevel-002> ;
  dct:issued "2002-07-13"^^xsd:date ;
  dct:modified "2008-01-14"^^xsd:date ;
  rdfs:comment "A class of entity, defined in terms of progression through an educational or training context, for which the described resource is intended."@en ;
  rdfs:isDefinedBy dct: ;
  rdfs:label "Audience Education Level"@en ;
  rdfs:range dct:AgentClass ;
  rdfs:subPropertyOf dct:audience ;
.
dct:extent
  rdf:type owl:AnnotationProperty ;
  rdf:type owl:NamedIndividual ;
  rdf:type owl:ObjectProperty ;
  dct:hasVersion <http://dublincore.org/usage/terms/history/#extent-003> ;
  dct:issued "2000-07-11"^^xsd:date ;
  dct:modified "2008-01-14"^^xsd:date ;
  rdfs:comment "The size or duration of the resource."@en ;
  rdfs:isDefinedBy dct: ;
  rdfs:label "Extent"@en ;
  rdfs:range dct:SizeOrDuration ;
  rdfs:subPropertyOf dc:format ;
  rdfs:subPropertyOf dct:format ;
.
dct:format
  rdf:type owl:AnnotationProperty ;
  rdf:type owl:NamedIndividual ;
  rdf:type owl:ObjectProperty ;
  dct:description "Examples of dimensions include size and duration. Recommended best practice is to use a controlled vocabulary such as the list of Internet Media Types [MIME]."@en ;
  dct:hasVersion <http://dublincore.org/usage/terms/history/#formatT-001> ;
  dct:issued "2008-01-14"^^xsd:date ;
  dct:modified "2008-01-14"^^xsd:date ;
  rdfs:comment "The file format, physical medium, or dimensions of the resource."@en ;
  rdfs:isDefinedBy dct: ;
  rdfs:label "Format"@en ;
  rdfs:range dct:MediaTypeOrExtent ;
  rdfs:subPropertyOf dc:format ;
.
dct:hasFormat
  rdf:type owl:AnnotationProperty ;
  rdf:type owl:NamedIndividual ;
  dct:hasVersion <http://dublincore.org/usage/terms/history/#hasFormat-003> ;
  dct:issued "2000-07-11"^^xsd:date ;
  dct:modified "2008-01-14"^^xsd:date ;
  rdfs:comment "A related resource that is substantially the same as the pre-existing described resource, but in another format."@en ;
  rdfs:isDefinedBy dct: ;
  rdfs:label "Has Format"@en ;
  rdfs:subPropertyOf dc:relation ;
  rdfs:subPropertyOf dct:relation ;
  skos:note "This term is intended to be used with non-literal values as defined in the DCMI Abstract Model (http://dublincore.org/documents/abstract-model/).  As of December 2007, the DCMI Usage Board is seeking a way to express this intention with a formal range declaration."@en ;
.
dct:hasPart
  rdf:type owl:AnnotationProperty ;
  rdf:type owl:NamedIndividual ;
  dct:hasVersion <http://dublincore.org/usage/terms/history/#hasPart-003> ;
  dct:issued "2000-07-11"^^xsd:date ;
  dct:modified "2008-01-14"^^xsd:date ;
  rdfs:comment "A related resource that is included either physically or logically in the described resource."@en ;
  rdfs:isDefinedBy dct: ;
  rdfs:label "Has Part"@en ;
  rdfs:subPropertyOf dc:relation ;
  rdfs:subPropertyOf dct:relation ;
  skos:note "This term is intended to be used with non-literal values as defined in the DCMI Abstract Model (http://dublincore.org/documents/abstract-model/).  As of December 2007, the DCMI Usage Board is seeking a way to express this intention with a formal range declaration."@en ;
.
dct:hasVersion
  rdf:type owl:AnnotationProperty ;
  rdf:type owl:NamedIndividual ;
  dct:hasVersion <http://dublincore.org/usage/terms/history/#hasVersion-003> ;
  dct:issued "2000-07-11"^^xsd:date ;
  dct:modified "2008-01-14"^^xsd:date ;
  rdfs:comment "A related resource that is a version, edition, or adaptation of the described resource."@en ;
  rdfs:isDefinedBy dct: ;
  rdfs:label "Has Version"@en ;
  rdfs:subPropertyOf dc:relation ;
  rdfs:subPropertyOf dct:relation ;
  skos:note "This term is intended to be used with non-literal values as defined in the DCMI Abstract Model (http://dublincore.org/documents/abstract-model/).  As of December 2007, the DCMI Usage Board is seeking a way to express this intention with a formal range declaration."@en ;
.
dct:identifier
  rdf:type owl:AnnotationProperty ;
  rdf:type owl:DatatypeProperty ;
  rdf:type owl:NamedIndividual ;
  dct:description "Recommended best practice is to identify the resource by means of a string conforming to a formal identification system. "@en ;
  dct:hasVersion <http://dublincore.org/usage/terms/history/#identifierT-001> ;
  dct:issued "2008-01-14"^^xsd:date ;
  dct:modified "2008-01-14"^^xsd:date ;
  rdfs:comment "An unambiguous reference to the resource within a given context."@en ;
  rdfs:isDefinedBy dct: ;
  rdfs:label "Identifier"@en ;
  rdfs:range rdfs:Literal ;
  rdfs:subPropertyOf dc:identifier ;
.
dct:instructionalMethod
  rdf:type owl:NamedIndividual ;
  rdf:type owl:ObjectProperty ;
  dct:description "Instructional Method will typically include ways of presenting instructional materials or conducting instructional activities, patterns of learner-to-learner and learner-to-instructor interactions, and mechanisms by which group and individual levels of learning are measured.  Instructional methods include all aspects of the instruction and learning processes from planning and implementation through evaluation and feedback."@en ;
  dct:hasVersion <http://dublincore.org/usage/terms/history/#instructionalMethod-002> ;
  dct:issued "2005-06-13"^^xsd:date ;
  dct:modified "2008-01-14"^^xsd:date ;
  rdfs:comment "A process, used to engender knowledge, attitudes and skills, that the described resource is designed to support."@en ;
  rdfs:isDefinedBy dct: ;
  rdfs:label "Instructional Method"@en ;
  rdfs:range dct:MethodOfInstruction ;
.
dct:isFormatOf
  rdf:type owl:AnnotationProperty ;
  rdf:type owl:NamedIndividual ;
  dct:hasVersion <http://dublincore.org/usage/terms/history/#isFormatOf-003> ;
  dct:issued "2000-07-11"^^xsd:date ;
  dct:modified "2008-01-14"^^xsd:date ;
  rdfs:comment "A related resource that is substantially the same as the described resource, but in another format."@en ;
  rdfs:isDefinedBy dct: ;
  rdfs:label "Is Format Of"@en ;
  rdfs:subPropertyOf dc:relation ;
  rdfs:subPropertyOf dct:relation ;
  skos:note "This term is intended to be used with non-literal values as defined in the DCMI Abstract Model (http://dublincore.org/documents/abstract-model/).  As of December 2007, the DCMI Usage Board is seeking a way to express this intention with a formal range declaration."@en ;
.
dct:isPartOf
  rdf:type owl:AnnotationProperty ;
  rdf:type owl:NamedIndividual ;
  dct:hasVersion <http://dublincore.org/usage/terms/history/#isPartOf-003> ;
  dct:issued "2000-07-11"^^xsd:date ;
  dct:modified "2008-01-14"^^xsd:date ;
  rdfs:comment "A related resource in which the described resource is physically or logically included."@en ;
  rdfs:isDefinedBy dct: ;
  rdfs:label "Is Part Of"@en ;
  rdfs:subPropertyOf dc:relation ;
  rdfs:subPropertyOf dct:relation ;
  skos:note "This term is intended to be used with non-literal values as defined in the DCMI Abstract Model (http://dublincore.org/documents/abstract-model/).  As of December 2007, the DCMI Usage Board is seeking a way to express this intention with a formal range declaration."@en ;
.
dct:isReferencedBy
  rdf:type owl:AnnotationProperty ;
  rdf:type owl:NamedIndividual ;
  dct:hasVersion <http://dublincore.org/usage/terms/history/#isReferencedBy-003> ;
  dct:issued "2000-07-11"^^xsd:date ;
  dct:modified "2008-01-14"^^xsd:date ;
  rdfs:comment "A related resource that references, cites, or otherwise points to the described resource."@en ;
  rdfs:isDefinedBy dct: ;
  rdfs:label "Is Referenced By"@en ;
  rdfs:subPropertyOf dc:relation ;
  rdfs:subPropertyOf dct:relation ;
  skos:note "This term is intended to be used with non-literal values as defined in the DCMI Abstract Model (http://dublincore.org/documents/abstract-model/).  As of December 2007, the DCMI Usage Board is seeking a way to express this intention with a formal range declaration."@en ;
.
dct:isReplacedBy
  rdf:type owl:AnnotationProperty ;
  rdf:type owl:NamedIndividual ;
  dct:hasVersion <http://dublincore.org/usage/terms/history/#isReplacedBy-003> ;
  dct:issued "2000-07-11"^^xsd:date ;
  dct:modified "2008-01-14"^^xsd:date ;
  rdfs:comment "A related resource that supplants, displaces, or supersedes the described resource."@en ;
  rdfs:isDefinedBy dct: ;
  rdfs:label "Is Replaced By"@en ;
  rdfs:subPropertyOf dc:relation ;
  rdfs:subPropertyOf dct:relation ;
  skos:note "This term is intended to be used with non-literal values as defined in the DCMI Abstract Model (http://dublincore.org/documents/abstract-model/).  As of December 2007, the DCMI Usage Board is seeking a way to express this intention with a formal range declaration."@en ;
.
dct:isRequiredBy
  rdf:type owl:AnnotationProperty ;
  rdf:type owl:NamedIndividual ;
  dct:hasVersion <http://dublincore.org/usage/terms/history/#isRequiredBy-003> ;
  dct:issued "2000-07-11"^^xsd:date ;
  dct:modified "2008-01-14"^^xsd:date ;
  rdfs:comment "A related resource that requires the described resource to support its function, delivery, or coherence."@en ;
  rdfs:isDefinedBy dct: ;
  rdfs:label "Is Required By"@en ;
  rdfs:subPropertyOf dc:relation ;
  rdfs:subPropertyOf dct:relation ;
  skos:note "This term is intended to be used with non-literal values as defined in the DCMI Abstract Model (http://dublincore.org/documents/abstract-model/).  As of December 2007, the DCMI Usage Board is seeking a way to express this intention with a formal range declaration."@en ;
.
dct:isVersionOf
  rdf:type owl:AnnotationProperty ;
  rdf:type owl:NamedIndividual ;
  dct:description "Changes in version imply substantive changes in content rather than differences in format."@en ;
  dct:hasVersion <http://dublincore.org/usage/terms/history/#isVersionOf-003> ;
  dct:issued "2000-07-11"^^xsd:date ;
  dct:modified "2008-01-14"^^xsd:date ;
  rdfs:comment "A related resource of which the described resource is a version, edition, or adaptation."@en ;
  rdfs:isDefinedBy dct: ;
  rdfs:label "Is Version Of"@en ;
  rdfs:subPropertyOf dc:relation ;
  rdfs:subPropertyOf dct:relation ;
  skos:note "This term is intended to be used with non-literal values as defined in the DCMI Abstract Model (http://dublincore.org/documents/abstract-model/).  As of December 2007, the DCMI Usage Board is seeking a way to express this intention with a formal range declaration."@en ;
.
dct:issued
  rdf:type owl:AnnotationProperty ;
  rdf:type owl:DatatypeProperty ;
  rdf:type owl:NamedIndividual ;
  dct:hasVersion <http://dublincore.org/usage/terms/history/#issued-003> ;
  dct:issued "2000-07-11"^^xsd:date ;
  dct:modified "2008-01-14"^^xsd:date ;
  rdfs:comment "Date of formal issuance (e.g., publication) of the resource."@en ;
  rdfs:isDefinedBy dct: ;
  rdfs:label "Date Issued"@en ;
  rdfs:range rdfs:Literal ;
  rdfs:subPropertyOf dc:date ;
  rdfs:subPropertyOf dct:date ;
.
dct:language
  rdf:type owl:AnnotationProperty ;
  rdf:type owl:NamedIndividual ;
  rdf:type owl:ObjectProperty ;
  dct:description "Recommended best practice is to use a controlled vocabulary such as RFC 4646 [RFC4646]."@en ;
  dct:hasVersion <http://dublincore.org/usage/terms/history/#languageT-001> ;
  dct:issued "2008-01-14"^^xsd:date ;
  dct:modified "2008-01-14"^^xsd:date ;
  rdfs:comment "A language of the resource."@en ;
  rdfs:isDefinedBy dct: ;
  rdfs:label "Language"@en ;
  rdfs:range dct:LinguisticSystem ;
  rdfs:subPropertyOf dc:language ;
.
dct:license
  rdf:type owl:AnnotationProperty ;
  rdf:type owl:NamedIndividual ;
  rdf:type owl:ObjectProperty ;
  dct:hasVersion <http://dublincore.org/usage/terms/history/#license-002> ;
  dct:issued "2004-06-14"^^xsd:date ;
  dct:modified "2008-01-14"^^xsd:date ;
  rdfs:comment "A legal document giving official permission to do something with the resource."@en ;
  rdfs:isDefinedBy dct: ;
  rdfs:label "License"@en ;
  rdfs:range dct:LicenseDocument ;
  rdfs:subPropertyOf dc:rights ;
  rdfs:subPropertyOf dct:rights ;
.
dct:mediator
  rdf:type owl:NamedIndividual ;
  rdf:type owl:ObjectProperty ;
  dct:description "In an educational context, a mediator might be a parent, teacher, teaching assistant, or care-giver."@en ;
  dct:hasVersion <http://dublincore.org/usage/terms/history/#mediator-003> ;
  dct:issued "2001-05-21"^^xsd:date ;
  dct:modified "2008-01-14"^^xsd:date ;
  rdfs:comment "An entity that mediates access to the resource and for whom the resource is intended or useful."@en ;
  rdfs:isDefinedBy dct: ;
  rdfs:label "Mediator"@en ;
  rdfs:range dct:AgentClass ;
  rdfs:subPropertyOf dct:audience ;
.
dct:medium
  rdf:type owl:AnnotationProperty ;
  rdf:type owl:NamedIndividual ;
  rdf:type owl:ObjectProperty ;
  dct:hasVersion <http://dublincore.org/usage/terms/history/#medium-003> ;
  dct:issued "2000-07-11"^^xsd:date ;
  dct:modified "2008-01-14"^^xsd:date ;
  rdfs:comment "The material or physical carrier of the resource."@en ;
  rdfs:domain dct:PhysicalResource ;
  rdfs:isDefinedBy dct: ;
  rdfs:label "Medium"@en ;
  rdfs:range dct:PhysicalMedium ;
  rdfs:subPropertyOf dc:format ;
  rdfs:subPropertyOf dct:format ;
.
dct:modified
  rdf:type owl:AnnotationProperty ;
  rdf:type owl:DatatypeProperty ;
  rdf:type owl:NamedIndividual ;
  dct:hasVersion <http://dublincore.org/usage/terms/history/#modified-003> ;
  dct:issued "2000-07-11"^^xsd:date ;
  dct:modified "2008-01-14"^^xsd:date ;
  rdfs:comment "Date on which the resource was changed."@en ;
  rdfs:isDefinedBy dct: ;
  rdfs:label "Date Modified"@en ;
  rdfs:range rdfs:Literal ;
  rdfs:subPropertyOf dc:date ;
  rdfs:subPropertyOf dct:date ;
.
dct:provenance
  rdf:type owl:NamedIndividual ;
  rdf:type owl:ObjectProperty ;
  dct:description "The statement may include a description of any changes successive custodians made to the resource."@en ;
  dct:hasVersion <http://dublincore.org/usage/terms/history/#provenance-002> ;
  dct:issued "2004-09-20"^^xsd:date ;
  dct:modified "2008-01-14"^^xsd:date ;
  rdfs:comment "A statement of any changes in ownership and custody of the resource since its creation that are significant for its authenticity, integrity, and interpretation."@en ;
  rdfs:isDefinedBy dct: ;
  rdfs:label "Provenance"@en ;
  rdfs:range dct:ProvenanceStatement ;
.
dct:publisher
  rdf:type owl:AnnotationProperty ;
  rdf:type owl:NamedIndividual ;
  rdf:type owl:ObjectProperty ;
  dct:description "Examples of a Publisher include a person, an organization, or a service."@en ;
  dct:hasVersion <http://dublincore.org/usage/terms/history/#publisherT-001> ;
  dct:issued "2008-01-14"^^xsd:date ;
  dct:modified "2010-10-11"^^xsd:date ;
  rdfs:comment "An entity responsible for making the resource available."@en ;
  rdfs:isDefinedBy dct: ;
  rdfs:label "Publisher"@en ;
  rdfs:range dct:Agent ;
  rdfs:subPropertyOf dc:publisher ;
.
dct:references
  rdf:type owl:AnnotationProperty ;
  rdf:type owl:NamedIndividual ;
  dct:hasVersion <http://dublincore.org/usage/terms/history/#references-003> ;
  dct:issued "2000-07-11"^^xsd:date ;
  dct:modified "2008-01-14"^^xsd:date ;
  rdfs:comment "A related resource that is referenced, cited, or otherwise pointed to by the described resource."@en ;
  rdfs:isDefinedBy dct: ;
  rdfs:label "References"@en ;
  rdfs:subPropertyOf dc:relation ;
  rdfs:subPropertyOf dct:relation ;
  skos:note "This term is intended to be used with non-literal values as defined in the DCMI Abstract Model (http://dublincore.org/documents/abstract-model/).  As of December 2007, the DCMI Usage Board is seeking a way to express this intention with a formal range declaration."@en ;
.
dct:relation
  rdf:type owl:AnnotationProperty ;
  rdf:type owl:NamedIndividual ;
  dct:description "Recommended best practice is to identify the related resource by means of a string conforming to a formal identification system. "@en ;
  dct:hasVersion <http://dublincore.org/usage/terms/history/#relationT-001> ;
  dct:issued "2008-01-14"^^xsd:date ;
  dct:modified "2008-01-14"^^xsd:date ;
  rdfs:comment "A related resource."@en ;
  rdfs:isDefinedBy dct: ;
  rdfs:label "Relation"@en ;
  rdfs:subPropertyOf dc:relation ;
  skos:note "This term is intended to be used with non-literal values as defined in the DCMI Abstract Model (http://dublincore.org/documents/abstract-model/).  As of December 2007, the DCMI Usage Board is seeking a way to express this intention with a formal range declaration."@en ;
.
dct:replaces
  rdf:type owl:AnnotationProperty ;
  rdf:type owl:NamedIndividual ;
  dct:hasVersion <http://dublincore.org/usage/terms/history/#replaces-003> ;
  dct:issued "2000-07-11"^^xsd:date ;
  dct:modified "2008-01-14"^^xsd:date ;
  rdfs:comment "A related resource that is supplanted, displaced, or superseded by the described resource."@en ;
  rdfs:isDefinedBy dct: ;
  rdfs:label "Replaces"@en ;
  rdfs:subPropertyOf dc:relation ;
  rdfs:subPropertyOf dct:relation ;
  skos:note "This term is intended to be used with non-literal values as defined in the DCMI Abstract Model (http://dublincore.org/documents/abstract-model/).  As of December 2007, the DCMI Usage Board is seeking a way to express this intention with a formal range declaration."@en ;
.
dct:requires
  rdf:type owl:AnnotationProperty ;
  rdf:type owl:NamedIndividual ;
  dct:hasVersion <http://dublincore.org/usage/terms/history/#requires-003> ;
  dct:issued "2000-07-11"^^xsd:date ;
  dct:modified "2008-01-14"^^xsd:date ;
  rdfs:comment "A related resource that is required by the described resource to support its function, delivery, or coherence."@en ;
  rdfs:isDefinedBy dct: ;
  rdfs:label "Requires"@en ;
  rdfs:subPropertyOf dc:relation ;
  rdfs:subPropertyOf dct:relation ;
  skos:note "This term is intended to be used with non-literal values as defined in the DCMI Abstract Model (http://dublincore.org/documents/abstract-model/).  As of December 2007, the DCMI Usage Board is seeking a way to express this intention with a formal range declaration."@en ;
.
dct:rights
  rdf:type owl:AnnotationProperty ;
  rdf:type owl:NamedIndividual ;
  rdf:type owl:ObjectProperty ;
  dct:description "Typically, rights information includes a statement about various property rights associated with the resource, including intellectual property rights."@en ;
  dct:hasVersion <http://dublincore.org/usage/terms/history/#rightsT-001> ;
  dct:issued "2008-01-14"^^xsd:date ;
  dct:modified "2008-01-14"^^xsd:date ;
  rdfs:comment "Information about rights held in and over the resource."@en ;
  rdfs:isDefinedBy dct: ;
  rdfs:label "Rights"@en ;
  rdfs:range dct:RightsStatement ;
  rdfs:subPropertyOf dc:rights ;
.
dct:rightsHolder
  rdf:type owl:NamedIndividual ;
  rdf:type owl:ObjectProperty ;
  dct:hasVersion <http://dublincore.org/usage/terms/history/#rightsHolder-002> ;
  dct:issued "2004-06-14"^^xsd:date ;
  dct:modified "2008-01-14"^^xsd:date ;
  rdfs:comment "A person or organization owning or managing rights over the resource."@en ;
  rdfs:isDefinedBy dct: ;
  rdfs:label "Rights Holder"@en ;
  rdfs:range dct:Agent ;
.
dct:source
  rdf:type owl:AnnotationProperty ;
  rdf:type owl:NamedIndividual ;
  dct:description "The described resource may be derived from the related resource in whole or in part. Recommended best practice is to identify the related resource by means of a string conforming to a formal identification system."@en ;
  dct:hasVersion <http://dublincore.org/usage/terms/history/#sourceT-001> ;
  dct:issued "2008-01-14"^^xsd:date ;
  dct:modified "2008-01-14"^^xsd:date ;
  rdfs:comment "A related resource from which the described resource is derived."@en ;
  rdfs:isDefinedBy dct: ;
  rdfs:label "Source"@en ;
  rdfs:subPropertyOf dc:source ;
  rdfs:subPropertyOf dct:relation ;
  skos:note "This term is intended to be used with non-literal values as defined in the DCMI Abstract Model (http://dublincore.org/documents/abstract-model/).  As of December 2007, the DCMI Usage Board is seeking a way to express this intention with a formal range declaration."@en ;
.
dct:spatial
  rdf:type owl:AnnotationProperty ;
  rdf:type owl:NamedIndividual ;
  rdf:type owl:ObjectProperty ;
  dct:hasVersion <http://dublincore.org/usage/terms/history/#spatial-003> ;
  dct:issued "2000-07-11"^^xsd:date ;
  dct:modified "2008-01-14"^^xsd:date ;
  rdfs:comment "Spatial characteristics of the resource."@en ;
  rdfs:isDefinedBy dct: ;
  rdfs:label "Spatial Coverage"@en ;
  rdfs:range dct:Location ;
  rdfs:subPropertyOf dc:coverage ;
  rdfs:subPropertyOf dct:coverage ;
.
dct:subject
  rdf:type owl:AnnotationProperty ;
  rdf:type owl:NamedIndividual ;
  dct:description "Typically, the subject will be represented using keywords, key phrases, or classification codes. Recommended best practice is to use a controlled vocabulary."@en ;
  dct:hasVersion <http://dublincore.org/usage/terms/history/#subjectT-002> ;
  dct:issued "2008-01-14"^^xsd:date ;
  dct:modified "2012-06-14"^^xsd:date ;
  rdfs:comment "The topic of the resource."@en ;
  rdfs:isDefinedBy dct: ;
  rdfs:label "Subject"@en ;
  rdfs:subPropertyOf dc:subject ;
  skos:note "This term is intended to be used with non-literal values as defined in the DCMI Abstract Model (http://dublincore.org/documents/abstract-model/).  As of December 2007, the DCMI Usage Board is seeking a way to express this intention with a formal range declaration."@en ;
.
dct:tableOfContents
  rdf:type owl:AnnotationProperty ;
  rdf:type owl:NamedIndividual ;
  dct:hasVersion <http://dublincore.org/usage/terms/history/#tableOfContents-003> ;
  dct:issued "2000-07-11"^^xsd:date ;
  dct:modified "2008-01-14"^^xsd:date ;
  rdfs:comment "A list of subunits of the resource."@en ;
  rdfs:isDefinedBy dct: ;
  rdfs:label "Table Of Contents"@en ;
  rdfs:subPropertyOf dc:description ;
  rdfs:subPropertyOf dct:description ;
.
dct:temporal
  rdf:type owl:AnnotationProperty ;
  rdf:type owl:NamedIndividual ;
  rdf:type owl:ObjectProperty ;
  dct:hasVersion <http://dublincore.org/usage/terms/history/#temporal-003> ;
  dct:issued "2000-07-11"^^xsd:date ;
  dct:modified "2008-01-14"^^xsd:date ;
  rdfs:comment "Temporal characteristics of the resource."@en ;
  rdfs:isDefinedBy dct: ;
  rdfs:label "Temporal Coverage"@en ;
  rdfs:range dct:PeriodOfTime ;
  rdfs:subPropertyOf dc:coverage ;
  rdfs:subPropertyOf dct:coverage ;
.
dct:title
  rdf:type owl:AnnotationProperty ;
  rdf:type owl:DatatypeProperty ;
  rdf:type owl:NamedIndividual ;
  dct:hasVersion <http://dublincore.org/usage/terms/history/#titleT-002> ;
  dct:issued "2008-01-14"^^xsd:date ;
  dct:modified "2010-10-11"^^xsd:date ;
  rdfs:comment "A name given to the resource."@en ;
  rdfs:isDefinedBy dct: ;
  rdfs:label "Title"@en ;
  rdfs:range rdfs:Literal ;
  rdfs:subPropertyOf dc:title ;
.
dct:type
  rdf:type owl:AnnotationProperty ;
  rdf:type owl:NamedIndividual ;
  rdf:type owl:ObjectProperty ;
  dct:description "Recommended best practice is to use a controlled vocabulary such as the DCMI Type Vocabulary [DCMITYPE]. To describe the file format, physical medium, or dimensions of the resource, use the Format element."@en ;
  dct:hasVersion <http://dublincore.org/usage/terms/history/#typeT-001> ;
  dct:issued "2008-01-14"^^xsd:date ;
  dct:modified "2008-01-14"^^xsd:date ;
  rdfs:comment "The nature or genre of the resource."@en ;
  rdfs:isDefinedBy dct: ;
  rdfs:label "Type"@en ;
  rdfs:range rdfs:Class ;
  rdfs:subPropertyOf dc:type ;
.
dct:valid
  rdf:type owl:AnnotationProperty ;
  rdf:type owl:DatatypeProperty ;
  rdf:type owl:NamedIndividual ;
  dct:hasVersion <http://dublincore.org/usage/terms/history/#valid-003> ;
  dct:issued "2000-07-11"^^xsd:date ;
  dct:modified "2008-01-14"^^xsd:date ;
  rdfs:comment "Date (often a range) of validity of a resource."@en ;
  rdfs:isDefinedBy dct: ;
  rdfs:label "Date Valid"@en ;
  rdfs:range rdfs:Literal ;
  rdfs:subPropertyOf dc:date ;
  rdfs:subPropertyOf dct:date ;
.
<http://purl.org/dc/terms/Location:title>
  rdf:type owl:Class ;
.
<http://purl.org/dc/terms:description>
  rdf:type owl:Class ;
.
<http://purl.org/dc/terms:identifier>
  rdf:type owl:Class ;
.
<http://purl.org/dc/terms:language>
  rdf:type owl:Class ;
.
<http://purl.org/dc/terms:title>
  rdf:type owl:Class ;
.
appearances:GenderStrict_1
  rdf:type <appearances:GenderStrict> ;
.
<http://www.opengis.net/rdf#:Point>
  rdf:type owl:Class ;
.
<http://www.semanticdesktop.org/ontologies/2007/01/19/nie#DataObject>
  rdf:type owl:Class ;
.
<http://www.semanticdesktop.org/ontologies/2007/01/19/nie#InformationElement>
  rdf:type owl:Class ;
.
<http://www.semanticdesktop.org/ontologies/2007/01/19/nie#comment>
  rdf:type owl:AnnotationProperty ;
.
<http://www.semanticdesktop.org/ontologies/2007/01/19/nie#created>
  rdf:type owl:AnnotationProperty ;
.
<http://www.semanticdesktop.org/ontologies/2007/01/19/nie#description>
  rdf:type owl:AnnotationProperty ;
.
<http://www.semanticdesktop.org/ontologies/2007/01/19/nie#generator>
  rdf:type owl:AnnotationProperty ;
.
<http://www.semanticdesktop.org/ontologies/2007/01/19/nie#generatorOption>
  rdf:type owl:AnnotationProperty ;
.
<http://www.semanticdesktop.org/ontologies/2007/01/19/nie#hasPart>
  rdf:type owl:AnnotationProperty ;
.
<http://www.semanticdesktop.org/ontologies/2007/01/19/nie#identifier>
  rdf:type owl:AnnotationProperty ;
.
<http://www.semanticdesktop.org/ontologies/2007/03/22/nco#Contact>
  rdf:type owl:Class ;
.
<http://www.semanticdesktop.org/ontologies/2007/03/22/nfo#Attachment>
  rdf:type owl:Class ;
.
ncal:AccessClassification
  rdf:type owl:Class ;
  rdfs:comment """Access classification of a calendar component. Introduced to express 
the set of values for the ncal:class property. The user may use instances
provided with this ontology or create his/her own with desired semantics.
See the documentation of ncal:class for details.""" ;
  rdfs:label "AccessClassification" ;
  rdfs:subClassOf rdfs:Resource ;
.
ncal:AccessClassification_1
  rdf:type ncal:AccessClassification ;
.
ncal:Alarm
  rdf:type owl:Class ;
  rdfs:comment "Provide a grouping of component properties that define an alarm." ;
  rdfs:label "Alarm" ;
  rdfs:subClassOf <http://www.semanticdesktop.org/ontologies/2007/01/19/nie#InformationElement> ;
  rdfs:subClassOf ncal:UnionOfAlarmEventFreebusyJournalTodo ;
  rdfs:subClassOf ncal:UnionOfAlarmEventFreebusyTodo ;
  rdfs:subClassOf ncal:UnionOfAlarmEventJournalTodo ;
  rdfs:subClassOf ncal:UnionOfAlarmEventTodo ;
.
ncal:AlarmAction
  rdf:type owl:Class ;
  rdfs:comment "Action to be performed on alarm. This class has been introduced to express the limited set of values of the ncal:action property. Please refer to the documentation of ncal:action for details." ;
  rdfs:label "AlarmAction" ;
  rdfs:subClassOf rdfs:Resource ;
.
ncal:Attachment
  rdf:type owl:Class ;
  rdfs:comment "An object attached to a calendar entity. This class has been introduced to serve as a structured value of the ncal:attach property. See the documentation of ncal:attach for details." ;
  rdfs:label "Attachment" ;
  rdfs:subClassOf <http://www.semanticdesktop.org/ontologies/2007/03/22/nfo#Attachment> ;
  rdfs:subClassOf rdfs:Resource ;
.
ncal:AttachmentEncoding
  rdf:type owl:Class ;
  rdfs:comment "Attachment encoding. This class has been introduced to express the limited vocabulary of values for the ncal:encoding property. See the documentation of ncal:encoding for details." ;
  rdfs:label "AttachmentEncoding" ;
  rdfs:subClassOf rdfs:Resource ;
.
ncal:Attendee
  rdf:type owl:Class ;
  rdfs:comment "An attendee of an event. This class has been introduced to serve as the range for ncal:attendee property. See documentation of ncal:attendee for details." ;
  rdfs:label "Attendee" ;
  rdfs:subClassOf ncal:AttendeeOrOrganizer ;
.
ncal:AttendeeOrOrganizer
  rdf:type owl:Class ;
  rdfs:comment "A common superclass for ncal:Attendee and ncal:Organizer." ;
  rdfs:label "AttendeeOrOrganizer" ;
  rdfs:subClassOf rdfs:Resource ;
.
ncal:AttendeeRole
  rdf:type owl:Class ;
  rdfs:comment "A role the attendee is going to play during an event. This class has been introduced to express the limited vocabulary for the values of ncal:role property. Please refer to the documentation of ncal:role for details." ;
  rdfs:label "AttendeeRole" ;
  rdfs:subClassOf rdfs:Resource ;
.
ncal:BydayRulePart
  rdf:type owl:Class ;
  rdfs:comment "Expresses the compound value of a byday part of a recurrence rule. It stores the weekday and the integer modifier. Inspired by RFC 2445 sec. 4.3.10" ;
  rdfs:label "BydayRulePart" ;
  rdfs:subClassOf rdfs:Resource ;
.
ncal:BydayRulePart_1
  rdf:type ncal:BydayRulePart ;
  ncal:bydayWeekday :Weekday_1 ;
.
ncal:BydayRulePart_2
  rdf:type ncal:BydayRulePart ;
  ncal:bydayWeekday :Weekday_2 ;
.
ncal:Calendar
  rdf:type owl:Class ;
  rdfs:comment "A calendar. Inspirations for this class can be traced to the VCALENDAR component defined in RFC 2445 sec. 4.4, but it may just as well be used to represent any kind of Calendar." ;
  rdfs:label "Calendar" ;
  rdfs:subClassOf <http://www.semanticdesktop.org/ontologies/2007/01/19/nie#InformationElement> ;
  rdfs:subClassOf [
      rdf:type owl:Restriction ;
      owl:allValuesFrom <ncal:Calendar> ;
      owl:onProperty airs:hasLanguageTimeOpen ;
    ] ;
.
ncal:CalendarDataObject
  rdf:type owl:Class ;
  rdfs:comment "A DataObject found in a calendar. It is usually interpreted as one of the calendar entity types (e.g. Event, Journal, Todo etc.)" ;
  rdfs:label "CalendarDataObject" ;
  rdfs:subClassOf <http://www.semanticdesktop.org/ontologies/2007/01/19/nie#DataObject> ;
.
ncal:CalendarScale
  rdf:type owl:Class ;
  rdfs:comment "A calendar scale. This class has been introduced to provide the limited vocabulary for the ncal:calscale property." ;
  rdfs:label "CalendarScale" ;
  rdfs:subClassOf rdfs:Resource ;
.
ncal:CalendarUserType
  rdf:type owl:Class ;
  rdfs:comment "A calendar user type. This class has been introduced to express the limited vocabulary for the ncal:cutype property. See documentation of ncal:cutype for details." ;
  rdfs:label "CalendarUserType" ;
  rdfs:subClassOf rdfs:Resource ;
.
ncal:Calendar_1
  rdf:type ncal:Calendar ;
  rdf:type owl:NamedIndividual ;
  ncal:component ncal:Event_1 ;
  ncal:prodid "7"^^xsd:string ;
  ncal:version "8"^^xsd:string ;
.
ncal:Calendar_2
  rdf:type ncal:Calendar ;
.
ncal:Calendar_3
  rdf:type ncal:Calendar ;
  ncal:component ncal:Event_3 ;
.
ncal:Event
  rdf:type owl:Class ;
  rdfs:comment "Provide a grouping of component properties that describe an event." ;
  rdfs:label "Event" ;
  rdfs:subClassOf <http://www.semanticdesktop.org/ontologies/2007/01/19/nie#InformationElement> ;
  rdfs:subClassOf ncal:UnionOfAlarmEventFreebusyJournalTodo ;
  rdfs:subClassOf ncal:UnionOfAlarmEventFreebusyTodo ;
  rdfs:subClassOf ncal:UnionOfAlarmEventJournalTodo ;
  rdfs:subClassOf ncal:UnionOfAlarmEventTodo ;
  rdfs:subClassOf ncal:UnionOfEventFreebusy ;
  rdfs:subClassOf ncal:UnionOfEventFreebusyJournalTodo ;
  rdfs:subClassOf ncal:UnionOfEventJournalTimezoneTodo ;
  rdfs:subClassOf ncal:UnionOfEventJournalTodo ;
  rdfs:subClassOf ncal:UnionOfEventTodo ;
  rdfs:subClassOf ncal:UnionOfTimezoneObservanceEventFreebusyJournalTimezoneTodo ;
  rdfs:subClassOf ncal:UnionOfTimezoneObservanceEventFreebusyTimezoneTodo ;
  rdfs:subClassOf ncal:UnionOfTimezoneObservanceEventJournalTimezoneTodo ;
.
ncal:EventStatus
  rdf:type owl:Class ;
  rdfs:comment """A status of an event. This class has been introduced to express
the limited set of values for the ncal:status property. The user may
use the instances provided with this ontology or create his/her own.
See the documentation for ncal:eventStatus for details.""" ;
  rdfs:label "EventStatus" ;
  rdfs:subClassOf rdfs:Resource ;
.
ncal:Event_1
  rdf:type ncal:Event ;
  ncal:class :AccessClassification_1 ;
  ncal:dtend :NcalDateTime_1 ;
  ncal:exrule :RecurrenceRule_1 ;
.
ncal:Event_2
  rdf:type ncal:Event ;
  ncal:dtstart :NcalDateTime_2 ;
  ncal:exdate :NcalDateTime_3 ;
  ncal:exrule :RecurrenceRule_2 ;
.
ncal:Event_3
  rdf:type ncal:Event ;
  ncal:exrule :RecurrenceRule_3 ;
.
ncal:Freebusy
  rdf:type owl:Class ;
  rdfs:comment "Provide a grouping of component properties that describe either a request for free/busy time, describe a response to a request for free/busy time or describe a published set of busy time." ;
  rdfs:label "Freebusy" ;
  rdfs:subClassOf <http://www.semanticdesktop.org/ontologies/2007/01/19/nie#InformationElement> ;
  rdfs:subClassOf ncal:UnionOfAlarmEventFreebusyJournalTodo ;
  rdfs:subClassOf ncal:UnionOfAlarmEventFreebusyTodo ;
  rdfs:subClassOf ncal:UnionOfEventFreebusy ;
  rdfs:subClassOf ncal:UnionOfEventFreebusyJournalTodo ;
  rdfs:subClassOf ncal:UnionOfTimezoneObservanceEventFreebusyJournalTimezoneTodo ;
  rdfs:subClassOf ncal:UnionOfTimezoneObservanceEventFreebusyTimezoneTodo ;
.
ncal:FreebusyPeriod
  rdf:type owl:Class ;
  rdfs:comment "An aggregate of a period and a freebusy type. This class has been introduced to serve as a range of the ncal:freebusy property. See documentation for ncal:freebusy for details. Note that the specification of freebusy property states that the period is to be expressed using UTC time, so the timezone properties should NOT be used for instances of this class." ;
  rdfs:label "FreebusyPeriod" ;
  rdfs:subClassOf ncal:NcalPeriod ;
.
ncal:FreebusyType
  rdf:type owl:Class ;
  rdfs:comment "Type of a Freebusy indication. This class has been introduced to serve as a limited set of values for the ncal:fbtype property. See the documentation of ncal:fbtype for details." ;
  rdfs:label "FreebusyType" ;
  rdfs:subClassOf rdfs:Resource ;
.
ncal:Journal
  rdf:type owl:Class ;
  rdfs:comment "Provide a grouping of component properties that describe a journal entry." ;
  rdfs:label "Journal" ;
  rdfs:subClassOf <http://www.semanticdesktop.org/ontologies/2007/01/19/nie#InformationElement> ;
  rdfs:subClassOf ncal:UnionOfAlarmEventFreebusyJournalTodo ;
  rdfs:subClassOf ncal:UnionOfAlarmEventJournalTodo ;
  rdfs:subClassOf ncal:UnionOfEventFreebusyJournalTodo ;
  rdfs:subClassOf ncal:UnionOfEventJournalTimezoneTodo ;
  rdfs:subClassOf ncal:UnionOfEventJournalTodo ;
  rdfs:subClassOf ncal:UnionOfTimezoneObservanceEventFreebusyJournalTimezoneTodo ;
  rdfs:subClassOf ncal:UnionOfTimezoneObservanceEventJournalTimezoneTodo ;
.
ncal:JournalStatus
  rdf:type owl:Class ;
  rdfs:comment """A status of a journal entry. This class has been introduced to express
the limited set of values for the ncal:status property. The user may
use the instances provided with this ontology or create his/her own.
See the documentation for ncal:journalStatus for details.""" ;
  rdfs:label "JournalStatus" ;
  rdfs:subClassOf rdfs:Resource ;
.
ncal:NcalDateTime
  rdf:type owl:Class ;
  rdfs:label "NcalDateTime" ;
  rdfs:subClassOf ncal:NcalTimeEntity ;
.
ncal:NcalDateTime_1
  rdf:type ncal:NcalDateTime ;
  ncal:date "2016-05-20"^^xsd:date ;
  ncal:ncalTimezone :Timezone_1 ;
.
ncal:NcalDateTime_2
  rdf:type ncal:NcalDateTime ;
  ncal:date "2014-07-20"^^xsd:date ;
.
ncal:NcalDateTime_3
  rdf:type ncal:NcalDateTime ;
.
ncal:NcalPeriod
  rdf:type owl:Class ;
  rdfs:comment "A period of time. Inspired by the PERIOD datatype specified in RFC 2445 sec. 4.3.9" ;
  rdfs:label "NcalPeriod" ;
  rdfs:subClassOf ncal:NcalTimeEntity ;
.
ncal:NcalTimeEntity
  rdf:type owl:Class ;
  rdfs:comment "A time entity. Conceived as a common superclass for NcalDateTime and NcalPeriod. According to RFC 2445 both DateTime and Period can be interpreted in different timezones. The first case is explored in many properties. The second case is theoretically possible in ncal:rdate property. Therefore the timezone properties have been defined at this level." ;
  rdfs:label "NcalTimeEntity" ;
  rdfs:subClassOf rdfs:Resource ;
.
ncal:Organizer
  rdf:type owl:Class ;
  rdfs:comment "An organizer of an event. This class has been introduced to serve as a range of ncal:organizer property. See documentation of ncal:organizer for details." ;
  rdfs:label "Organizer" ;
  rdfs:subClassOf ncal:AttendeeOrOrganizer ;
.
ncal:ParticipationStatus
  rdf:type owl:Class ;
  rdfs:comment "Participation Status. This class has been introduced to express the limited vocabulary of values for the ncal:partstat property. See the documentation of ncal:partstat for details." ;
  rdfs:label "ParticipationStatus" ;
  rdfs:subClassOf rdfs:Resource ;
.
ncal:RecurrenceFrequency
  rdf:type owl:Class ;
  rdfs:comment "Frequency of a recurrence rule. This class has been introduced to express a limited set of allowed values for the ncal:freq property. See the documentation of ncal:freq for details." ;
  rdfs:label "RecurrenceFrequency" ;
  rdfs:subClassOf rdfs:Resource ;
.
ncal:RecurrenceFrequency_1
  rdf:type ncal:RecurrenceFrequency ;
.
ncal:RecurrenceIdentifier
  rdf:type owl:Class ;
  rdfs:comment "Recurrence Identifier. Introduced to provide a structure for the value of ncal:recurrenceId property. See the documentation of ncal:recurrenceId for details." ;
  rdfs:label "RecurrenceIdentifier" ;
  rdfs:subClassOf rdfs:Resource ;
.
ncal:RecurrenceIdentifierRange
  rdf:type owl:Class ;
  rdfs:comment "Recurrence Identifier Range. This class has been created to provide means to express the limited set of values for the ncal:range property. See documentation for ncal:range for details." ;
  rdfs:label "RecurrenceIdentifierRange" ;
  rdfs:subClassOf rdfs:Resource ;
.
ncal:RecurrenceRule
  rdf:type owl:Class ;
  rdfs:label "RecurrenceRule" ;
  rdfs:subClassOf rdfs:Resource ;
.
ncal:RecurrenceRule_1
  rdf:type ncal:RecurrenceRule ;
  ncal:byday :BydayRulePart_1 ;
.
ncal:RecurrenceRule_2
  rdf:type ncal:RecurrenceRule ;
  ncal:byday :BydayRulePart_2 ;
  ncal:count 2 ;
  ncal:freq :RecurrenceFrequency_1 ;
  ncal:interval 3 ;
.
ncal:RecurrenceRule_3
  rdf:type ncal:RecurrenceRule ;
  ncal:bymonth 06 ;
.
ncal:RequestStatus
  rdf:type owl:Class ;
  rdfs:comment "Request Status. A class that was introduced to provide a structure for the value of ncal:requestStatus property. See documentation for ncal:requestStatus for details." ;
  rdfs:label "RequestStatus" ;
  rdfs:subClassOf rdfs:Resource ;
.
ncal:TimeTransparency
  rdf:type owl:Class ;
  rdfs:comment """Time transparency. Introduced to provide a way to express
the limited vocabulary for the values of ncal:transp property.
See documentation of ncal:transp for details.""" ;
  rdfs:label "TimeTransparency" ;
  rdfs:subClassOf rdfs:Resource ;
.
ncal:Timezone
  rdf:type owl:Class ;
  rdfs:comment "Provide a grouping of component properties that defines a time zone." ;
  rdfs:label "Timezone" ;
  rdfs:subClassOf <http://www.semanticdesktop.org/ontologies/2007/01/19/nie#InformationElement> ;
  rdfs:subClassOf ncal:UnionOfEventJournalTimezoneTodo ;
  rdfs:subClassOf ncal:UnionOfTimezoneObservanceEventFreebusyJournalTimezoneTodo ;
  rdfs:subClassOf ncal:UnionOfTimezoneObservanceEventFreebusyTimezoneTodo ;
  rdfs:subClassOf ncal:UnionOfTimezoneObservanceEventJournalTimezoneTodo ;
.
ncal:TimezoneObservance
  rdf:type owl:Class ;
  rdfs:label "TimezoneObservance" ;
  rdfs:subClassOf ncal:UnionOfTimezoneObservanceEventFreebusyJournalTimezoneTodo ;
  rdfs:subClassOf ncal:UnionOfTimezoneObservanceEventFreebusyTimezoneTodo ;
  rdfs:subClassOf ncal:UnionOfTimezoneObservanceEventJournalTimezoneTodo ;
.
ncal:Timezone_1
  rdf:type ncal:Timezone ;
  ncal:tzid "05"^^xsd:string ;
.
ncal:Todo
  rdf:type owl:Class ;
  rdfs:comment "Provide a grouping of calendar properties that describe a to-do." ;
  rdfs:label "Todo" ;
  rdfs:subClassOf <http://www.semanticdesktop.org/ontologies/2007/01/19/nie#InformationElement> ;
  rdfs:subClassOf ncal:UnionOfAlarmEventFreebusyJournalTodo ;
  rdfs:subClassOf ncal:UnionOfAlarmEventFreebusyTodo ;
  rdfs:subClassOf ncal:UnionOfAlarmEventJournalTodo ;
  rdfs:subClassOf ncal:UnionOfAlarmEventTodo ;
  rdfs:subClassOf ncal:UnionOfEventFreebusyJournalTodo ;
  rdfs:subClassOf ncal:UnionOfEventJournalTimezoneTodo ;
  rdfs:subClassOf ncal:UnionOfEventJournalTodo ;
  rdfs:subClassOf ncal:UnionOfEventTodo ;
  rdfs:subClassOf ncal:UnionOfTimezoneObservanceEventFreebusyJournalTimezoneTodo ;
  rdfs:subClassOf ncal:UnionOfTimezoneObservanceEventFreebusyTimezoneTodo ;
  rdfs:subClassOf ncal:UnionOfTimezoneObservanceEventJournalTimezoneTodo ;
.
ncal:TodoStatus
  rdf:type owl:Class ;
  rdfs:comment """A status of a calendar entity. This class has been introduced to express
the limited set of values for the ncal:status property. The user may
use the instances provided with this ontology or create his/her own.
See the documentation for ncal:todoStatus for details.""" ;
  rdfs:label "TodoStatus" ;
  rdfs:subClassOf rdfs:Resource ;
.
ncal:Trigger
  rdf:type owl:Class ;
  rdfs:comment "An alarm trigger. This class has been created to serve as the range of ncal:trigger property. See the documentation for ncal:trigger for more details." ;
  rdfs:label "Trigger" ;
  rdfs:subClassOf rdfs:Resource ;
.
ncal:TriggerRelation
  rdf:type owl:Class ;
  rdfs:comment "The relation between the trigger and its parent calendar component. This class has been introduced to express the limited vocabulary for the ncal:related property. See the documentation for ncal:related for more details." ;
  rdfs:label "TriggerRelation" ;
  rdfs:subClassOf rdfs:Resource ;
.
ncal:UnionOfAlarmEventFreebusyJournalTodo
  rdf:type owl:Class ;
  rdfs:label "UnionOfAlarmEventFreebusyJournalTodo" ;
  rdfs:subClassOf ncal:UnionParentClass ;
.
ncal:UnionOfAlarmEventFreebusyTodo
  rdf:type owl:Class ;
  rdfs:label "UnionOfAlarmEventFreebusyTodo" ;
  rdfs:subClassOf ncal:UnionParentClass ;
.
ncal:UnionOfAlarmEventJournalTodo
  rdf:type owl:Class ;
  rdfs:label "UnionOfAlarmEventJournalTodo" ;
  rdfs:subClassOf ncal:UnionParentClass ;
.
ncal:UnionOfAlarmEventTodo
  rdf:type owl:Class ;
  rdfs:label "UnionOfAlarmEventTodo" ;
  rdfs:subClassOf ncal:UnionParentClass ;
.
ncal:UnionOfEventFreebusy
  rdf:type owl:Class ;
  rdfs:label "UnionOfEventFreebusy" ;
  rdfs:subClassOf ncal:UnionParentClass ;
.
ncal:UnionOfEventFreebusyJournalTodo
  rdf:type owl:Class ;
  rdfs:label "UnionOfEventFreebusyJournalTodo" ;
  rdfs:subClassOf ncal:UnionParentClass ;
.
ncal:UnionOfEventJournalTimezoneTodo
  rdf:type owl:Class ;
  rdfs:label "UnionOfEventJournalTimezoneTodo" ;
  rdfs:subClassOf ncal:UnionParentClass ;
.
ncal:UnionOfEventJournalTodo
  rdf:type owl:Class ;
  rdfs:label "UnionOfEventJournalTodo" ;
  rdfs:subClassOf ncal:UnionParentClass ;
.
ncal:UnionOfEventTodo
  rdf:type owl:Class ;
  rdfs:label "UnionOfEventTodo" ;
  rdfs:subClassOf ncal:UnionParentClass ;
.
ncal:UnionOfTimezoneObservanceEventFreebusyJournalTimezoneTodo
  rdf:type owl:Class ;
  rdfs:label "UnionOfTimezoneObservanceEventFreebusyJournalTimezoneTodo" ;
  rdfs:subClassOf ncal:UnionParentClass ;
.
ncal:UnionOfTimezoneObservanceEventFreebusyTimezoneTodo
  rdf:type owl:Class ;
  rdfs:label "UnionOfTimezoneObservanceEventFreebusyTimezoneTodo" ;
  rdfs:subClassOf ncal:UnionParentClass ;
.
ncal:UnionOfTimezoneObservanceEventJournalTimezoneTodo
  rdf:type owl:Class ;
  rdfs:label "UnionOfTimezoneObservanceEventJournalTimezoneTodo" ;
  rdfs:subClassOf ncal:UnionParentClass ;
.
ncal:UnionParentClass
  rdf:type owl:Class ;
  rdfs:label "UnionParentClass" ;
  rdfs:subClassOf rdfs:Resource ;
.
ncal:Weekday
  rdf:type owl:Class ;
  rdfs:comment "Day of the week. This class has been created to provide the limited vocabulary for ncal:byday property. See the documentation for ncal:byday for details." ;
  rdfs:label "Weekday" ;
  rdfs:subClassOf rdfs:Resource ;
.
ncal:Weekday_1
  rdf:type ncal:Weekday ;
.
ncal:Weekday_2
  rdf:type ncal:Weekday ;
.
ncal:_8bitEncoding
  rdf:type ncal:AttachmentEncoding ;
  rdf:type owl:NamedIndividual ;
  rdfs:label "_8bitEncoding" ;
.
ncal:acceptedParticipationStatus
  rdf:type ncal:ParticipationStatus ;
  rdf:type owl:NamedIndividual ;
  rdfs:label "acceptedParticipationStatus" ;
.
ncal:action
  rdf:type owl:ObjectProperty ;
  rdfs:comment "This property defines the action to be invoked when an alarm is triggered. Inspired by RFC 2445 sec 4.8.6.1. Originally this property had a limited set of values. They are expressed as instances of the AlarmAction class." ;
  rdfs:domain ncal:Alarm ;
  rdfs:label "action" ;
  rdfs:range ncal:AlarmAction ;
.
ncal:attach
  rdf:type owl:AnnotationProperty ;
  rdf:type owl:ObjectProperty ;
  rdfs:comment "The property provides the capability to associate a document object with a calendar component. Defined in the RFC 2445 sec. 4.8.1.1" ;
  rdfs:domain ncal:UnionOfAlarmEventJournalTodo ;
  rdfs:label "attach" ;
  rdfs:range ncal:Attachment ;
  rdfs:subPropertyOf <http://www.semanticdesktop.org/ontologies/2007/01/19/nie#hasPart> ;
.
ncal:attachmentContent
  rdf:type owl:DatatypeProperty ;
  rdfs:comment "The uri of the attachment. Created to express the actual value of the ATTACH property defined in RFC 2445 sec. 4.8.1.1. This property expresses the BINARY datatype of that property. see ncal:attachmentUri for the URI datatype." ;
  rdfs:domain ncal:Attachment ;
  rdfs:label "attachmentContent" ;
  rdfs:range xsd:string ;
.
ncal:attachmentUri
  rdf:type owl:ObjectProperty ;
  nrl:maxCardinality 1 ;
  rdfs:comment "The uri of the attachment. Created to express the actual value of the ATTACH property defined in RFC 2445 sec. 4.8.1.1. This property expresses the default URI datatype of that property. see ncal:attachmentContents for the BINARY datatype." ;
  rdfs:domain ncal:Attachment ;
  rdfs:label "attachmentUri" ;
  rdfs:range rdfs:Resource ;
.
ncal:attendee
  rdf:type owl:ObjectProperty ;
  rdfs:comment "The property defines an \"Attendee\" within a calendar component. Inspired by RFC 2445 sec. 4.8.4.1. Originally this property accepted many parameters. The Attendee class has been introduced to express them all. Note that NCAL is aligned with NCO. The actual value (of the CAL-ADDRESS type) is expressed as an instance of nco:Contact. Remember that the CN parameter has been removed from NCAL. Instead that value should be expressed using nco:fullname property of the above mentioned nco:Contact instance. The RFC stated that whenever this property is attached to a Valarm instance, the Attendee cannot have any parameters apart from involvedContact." ;
  rdfs:domain ncal:UnionOfAlarmEventFreebusyJournalTodo ;
  rdfs:label "attendee" ;
  rdfs:range ncal:Attendee ;
.
ncal:audioAction
  rdf:type ncal:AlarmAction ;
  rdf:type owl:NamedIndividual ;
  rdfs:label "audioAction" ;
.
ncal:base64Encoding
  rdf:type ncal:AttachmentEncoding ;
  rdf:type owl:NamedIndividual ;
  rdfs:label "base64Encoding" ;
.
ncal:busyFreebusyType
  rdf:type ncal:FreebusyType ;
  rdf:type owl:NamedIndividual ;
  rdfs:label "busyFreebusyType" ;
.
ncal:busyTentativeFreebusyType
  rdf:type ncal:FreebusyType ;
  rdf:type owl:NamedIndividual ;
  rdfs:label "busyTentativeFreebusyType" ;
.
ncal:busyUnavailableFreebusyType
  rdf:type ncal:FreebusyType ;
  rdf:type owl:NamedIndividual ;
  rdfs:label "busyUnavailableFreebusyType" ;
.
ncal:byday
  rdf:type owl:ObjectProperty ;
  rdfs:comment "Weekdays the recurrence should occur. Defined in RFC 2445 sec. 4.3.10" ;
  rdfs:domain ncal:RecurrenceRule ;
  rdfs:label "byday" ;
  rdfs:range ncal:BydayRulePart ;
.
ncal:bydayModifier
  rdf:type owl:DatatypeProperty ;
  nrl:maxCardinality 1 ;
  rdfs:comment "An integer modifier for the BYDAY rule part.    Each BYDAY value can also be preceded by a positive (+n) or negative  (-n) integer. If present, this indicates the nth occurrence of the specific day within the MONTHLY or YEARLY RRULE. For example, within a MONTHLY rule, +1MO (or simply 1MO) represents the first Monday within the month, whereas -1MO represents the last Monday of the month. If an integer modifier is not present, it means all days of this type within the specified frequency. For example, within a MONTHLY rule, MO represents all Mondays within the month. Inspired by RFC 2445 sec. 4.3.10" ;
  rdfs:domain ncal:BydayRulePart ;
  rdfs:label "bydayModifier" ;
  rdfs:range xsd:integer ;
.
ncal:bydayWeekday
  rdf:type owl:ObjectProperty ;
  rdfs:comment "Connects a BydayRulePath with a weekday." ;
  rdfs:domain ncal:BydayRulePart ;
  rdfs:label "bydayWeekday" ;
  rdfs:range ncal:Weekday ;
.
ncal:byhour
  rdf:type owl:DatatypeProperty ;
  rdfs:comment "Hour of recurrence. Defined in RFC 2445 sec. 4.3.10" ;
  rdfs:domain ncal:RecurrenceRule ;
  rdfs:label "byhour" ;
  rdfs:range xsd:integer ;
.
ncal:byminute
  rdf:type owl:DatatypeProperty ;
  rdfs:comment "Minute of recurrence. Defined in RFC 2445 sec. 4.3.10" ;
  rdfs:domain ncal:RecurrenceRule ;
  rdfs:label "byminute" ;
  rdfs:range xsd:integer ;
.
ncal:bymonth
  rdf:type owl:DatatypeProperty ;
  rdfs:comment "Number of the month of the recurrence. Valid values are integers from 1 (January) to 12 (December). Defined in RFC 2445 sec. 4.3.10" ;
  rdfs:domain ncal:RecurrenceRule ;
  rdfs:label "bymonth" ;
  rdfs:range xsd:integer ;
.
ncal:bymonthday
  rdf:type owl:DatatypeProperty ;
  rdfs:comment "Day of the month when the event should recur. Defined in RFC 2445 sec. 4.3.10" ;
  rdfs:domain ncal:RecurrenceRule ;
  rdfs:label "bymonthday" ;
  rdfs:range xsd:integer ;
.
ncal:bysecond
  rdf:type owl:DatatypeProperty ;
  rdfs:comment "Second of a recurrence. Defined in RFC 2445 sec. 4.3.10" ;
  rdfs:domain ncal:RecurrenceRule ;
  rdfs:label "bysecond" ;
  rdfs:range xsd:integer ;
.
ncal:bysetpos
  rdf:type owl:DatatypeProperty ;
  rdfs:comment "The BYSETPOS rule part specify values which correspond to the nth occurrence within the set of events specified by the rule. Valid values are 1 to 366 or -366 to -1. It MUST only be used in conjunction with another BYxxx rule part. For example \"the last work day of the month\" could be represented as: RRULE: FREQ=MONTHLY; BYDAY=MO, TU, WE, TH, FR; BYSETPOS=-1. Each BYSETPOS value can include a positive (+n) or negative (-n)  integer. If present, this indicates the nth occurrence of the  specific occurrence within the set of events specified by the rule. Defined in RFC 2445 sec. 4.3.10" ;
  rdfs:domain ncal:RecurrenceRule ;
  rdfs:label "bysetpos" ;
  rdfs:range xsd:integer ;
.
ncal:byweekno
  rdf:type owl:DatatypeProperty ;
  rdfs:comment "The number of the week an event should recur. Defined in RFC 2445 sec. 4.3.10" ;
  rdfs:domain ncal:RecurrenceRule ;
  rdfs:label "byweekno" ;
  rdfs:range xsd:integer ;
.
ncal:byyearday
  rdf:type owl:DatatypeProperty ;
  rdfs:comment "Day of the year the event should occur. Defined in RFC 2445 sec. 4.3.10" ;
  rdfs:domain ncal:RecurrenceRule ;
  rdfs:label "byyearday" ;
  rdfs:range xsd:integer ;
.
ncal:calscale
  rdf:type owl:ObjectProperty ;
  nrl:maxCardinality 1 ;
  rdfs:comment "This property defines the calendar scale used for the calendar information specified in the iCalendar object. Defined in RFC 2445 sec. 4.7.1" ;
  rdfs:domain ncal:Calendar ;
  rdfs:label "calscale" ;
  rdfs:range ncal:CalendarScale ;
.
ncal:cancelledEventStatus
  rdf:type ncal:EventStatus ;
  rdf:type owl:NamedIndividual ;
  rdfs:label "cancelledEventStatus" ;
.
ncal:cancelledJournalStatus
  rdf:type ncal:JournalStatus ;
  rdf:type owl:NamedIndividual ;
  rdfs:label "cancelledJournalStatus" ;
.
ncal:cancelledTodoStatus
  rdf:type ncal:TodoStatus ;
  rdf:type owl:NamedIndividual ;
  rdfs:label "cancelledTodoStatus" ;
.
ncal:categories
  rdf:type owl:DatatypeProperty ;
  rdfs:comment "Categories for a calendar component. Inspired by RFC 2445 sec 4.8.1.2 with the following reservations: The LANGUAGE parameter has been discarded. Please use xml:lang literals to express multiple languages. This property can specify multiple comma-separated categories. The order of categories doesn't matter. Please use a separate triple for each category." ;
  rdfs:domain ncal:UnionOfEventJournalTodo ;
  rdfs:label "categories" ;
  rdfs:range xsd:string ;
.
ncal:chairRole
  rdf:type ncal:AttendeeRole ;
  rdf:type owl:NamedIndividual ;
  rdfs:label "chairRole" ;
.
ncal:class
  rdf:type owl:ObjectProperty ;
  nrl:maxCardinality 1 ;
  rdfs:comment "Defines the access classification for a calendar component. Inspired by RFC 2445 sec. 4.8.1.3 with the following reservations:  this property has limited vocabulary. Possible values are:  PUBLIC, PRIVATE and CONFIDENTIAL. The default is PUBLIC. Those values are expressed as instances of the AccessClassification class. The user may create his/her own if necessary." ;
  rdfs:domain ncal:UnionOfEventJournalTodo ;
  rdfs:label "class" ;
  rdfs:range ncal:AccessClassification ;
.
ncal:comment
  rdf:type owl:AnnotationProperty ;
  rdf:type owl:DatatypeProperty ;
  rdfs:comment "Non-processing information intended to provide a comment to the calendar user. Inspired by RFC 2445 sec. 4.8.1.4 with the following reservations:  the LANGUAGE parameter has been discarded. Please use xml:lang literals to express language. For the ALTREP parameter use the commentAltRep property." ;
  rdfs:domain ncal:UnionOfTimezoneObservanceEventFreebusyJournalTimezoneTodo ;
  rdfs:label "comment" ;
  rdfs:range xsd:string ;
  rdfs:subPropertyOf <http://www.semanticdesktop.org/ontologies/2007/01/19/nie#comment> ;
.
ncal:commentAltRep
  rdf:type owl:ObjectProperty ;
  rdfs:comment """Alternate representation of the comment. Introduced to cover 
the ALTREP parameter of the COMMENT property. See 
documentation of ncal:comment for details.""" ;
  rdfs:domain ncal:UnionOfTimezoneObservanceEventFreebusyJournalTimezoneTodo ;
  rdfs:label "commentAltRep" ;
  rdfs:range rdfs:Resource ;
.
ncal:completed
  rdf:type owl:DatatypeProperty ;
  nrl:maxCardinality 1 ;
  rdfs:comment "This property defines the date and time that a to-do was actually completed. Inspired by RFC 2445 sec. 4.8.2.1. Note that the RFC allows ONLY UTC time values for this property." ;
  rdfs:domain ncal:Todo ;
  rdfs:label "completed" ;
  rdfs:range xsd:dateTime ;
.
ncal:completedParticipationStatus
  rdf:type ncal:ParticipationStatus ;
  rdf:type owl:NamedIndividual ;
  rdfs:label "completedParticipationStatus" ;
.
ncal:completedStatus
  rdf:type ncal:TodoStatus ;
  rdf:type owl:NamedIndividual ;
  rdfs:label "completedStatus" ;
.
ncal:component
  rdf:type owl:AnnotationProperty ;
  rdf:type owl:ObjectProperty ;
  rdfs:comment "Links the Vcalendar instance with the calendar components. This property has no direct equivalent in the RFC specification. It has been introduced to express the containmnent relations." ;
  rdfs:domain ncal:Calendar ;
  rdfs:label "component" ;
  rdfs:range ncal:CalendarDataObject ;
  rdfs:subPropertyOf <http://www.semanticdesktop.org/ontologies/2007/01/19/nie#hasPart> ;
.
ncal:confidentialClassification
  rdf:type ncal:AccessClassification ;
  rdf:type owl:NamedIndividual ;
  rdfs:label "confidentialClassification" ;
.
ncal:confirmedStatus
  rdf:type ncal:EventStatus ;
  rdf:type owl:NamedIndividual ;
  rdfs:label "confirmedStatus" ;
.
ncal:contact
  rdf:type owl:DatatypeProperty ;
  rdfs:comment "The property is used to represent contact information or alternately a reference to contact information associated with the calendar component. Inspired by RFC 2445 sec. 4.8.4.2 with the following reservations: the LANGUAGE parameter has been discarded. Please use xml:lang literals to express language. For the ALTREP parameter use the contactAltRep property.RFC doesn't define any format for the string." ;
  rdfs:domain ncal:UnionOfEventFreebusyJournalTodo ;
  rdfs:label "contact" ;
  rdfs:range xsd:string ;
.
ncal:contactAltRep
  rdf:type owl:ObjectProperty ;
  rdfs:comment """Alternate representation of the contact property. Introduced to cover 
the ALTREP parameter of the CONTACT property. See 
documentation of ncal:contact for details.""" ;
  rdfs:domain ncal:UnionOfEventFreebusyJournalTodo ;
  rdfs:label "contactAltRep" ;
  rdfs:range rdfs:Resource ;
.
ncal:count
  rdf:type owl:DatatypeProperty ;
  nrl:maxCardinality 1 ;
  rdfs:comment "How many times should an event be repeated. Defined in RFC 2445 sec. 4.3.10" ;
  rdfs:domain ncal:RecurrenceRule ;
  rdfs:label "count" ;
  rdfs:range xsd:integer ;
.
ncal:created
  rdf:type owl:AnnotationProperty ;
  rdf:type owl:DatatypeProperty ;
  nrl:maxCardinality 1 ;
  rdfs:comment "This property specifies the date and time that the calendar information was created by the calendar user agent in the calendar store. Note: This is analogous to the creation date and time for a file in the file system. Inspired by RFC 2445 sec. 4.8.7.1. Note that this property is a subproperty of nie:created. The domain of nie:created is nie:DataObject. It is not a superclass of UnionOf_Vevent_Vjournal_Vtodo, but since that union is conceived as an 'abstract' class, and in real-life all resources referenced by this property will also be DataObjects, than this shouldn't cause too much of a problem. Note that RFC allows ONLY UTC time values for this property." ;
  rdfs:domain ncal:UnionOfEventJournalTodo ;
  rdfs:label "created" ;
  rdfs:range xsd:dateTime ;
  rdfs:subPropertyOf <http://www.semanticdesktop.org/ontologies/2007/01/19/nie#created> ;
.
ncal:cutype
  rdf:type owl:ObjectProperty ;
  rdfs:comment "To specify the type of calendar user specified by the property. Inspired by RFC 2445 sec. 4.2.3. This parameter has a limited vocabulary. The terms that may serve as values for this property have been expressed as instances of CalendarUserType class. The user may use instances provided with this ontology or create his own." ;
  rdfs:domain ncal:Attendee ;
  rdfs:label "cutype" ;
  rdfs:range ncal:CalendarUserType ;
.
ncal:daily
  rdf:type ncal:RecurrenceFrequency ;
  rdf:type owl:NamedIndividual ;
  rdfs:label "daily" ;
.
ncal:date
  rdf:type owl:DatatypeProperty ;
  nrl:maxCardinality 1 ;
  rdfs:comment "Date an instance of NcalDateTime refers to. It was conceived to express values in DATE datatype specified in RFC 2445 4.3.4" ;
  rdfs:domain ncal:NcalDateTime ;
  rdfs:label "date" ;
  rdfs:range xsd:date ;
.
ncal:dateTime
  rdf:type owl:DatatypeProperty ;
  nrl:maxCardinality 1 ;
  rdfs:comment "Representation of a date an instance of NcalDateTime actually refers to. It's purpose is to express values in DATE-TIME datatype, as defined in RFC 2445 sec. 4.3.5" ;
  rdfs:domain ncal:NcalDateTime ;
  rdfs:label "dateTime" ;
  rdfs:range xsd:dateTime ;
.
ncal:daylight
  rdf:type owl:ObjectProperty ;
  nrl:maxCardinality 1 ;
  rdfs:comment "Links a timezone with it's daylight observance. This property has no direct equivalent in the RFC 2445. It has been inspired by the structure of the Vtimezone component defined in sec.4.6.5" ;
  rdfs:domain ncal:Timezone ;
  rdfs:label "daylight" ;
  rdfs:range ncal:TimezoneObservance ;
.
ncal:declinedParticipationStatus
  rdf:type ncal:ParticipationStatus ;
  rdf:type owl:NamedIndividual ;
  rdfs:label "declinedParticipationStatus" ;
.
ncal:delegatedFrom
  rdf:type owl:ObjectProperty ;
  rdfs:comment "To specify the calendar users that have delegated their participation to the calendar user specified by the property. Inspired by RFC 2445 sec. 4.2.4. Originally the value type for this property was CAL-ADDRESS. This has been expressed as nco:Contact to promote integration between NCAL and NCO." ;
  rdfs:domain ncal:Attendee ;
  rdfs:label "delegatedFrom" ;
  rdfs:range <http://www.semanticdesktop.org/ontologies/2007/03/22/nco#Contact> ;
.
ncal:delegatedParticipationStatus
  rdf:type ncal:ParticipationStatus ;
  rdf:type owl:NamedIndividual ;
  rdfs:label "delegatedParticipationStatus" ;
.
ncal:delegatedTo
  rdf:type owl:ObjectProperty ;
  rdfs:comment "To specify the calendar users to whom the calendar user specified by the property has delegated participation. Inspired by RFC 2445 sec. 4.2.5. Originally the value type for this parameter was CAL-ADDRESS. This has been expressed as nco:Contact to promote integration between NCAL and NCO." ;
  rdfs:domain ncal:Attendee ;
  rdfs:label "delegatedTo" ;
  rdfs:range <http://www.semanticdesktop.org/ontologies/2007/03/22/nco#Contact> ;
.
ncal:description
  rdf:type owl:AnnotationProperty ;
  rdf:type owl:DatatypeProperty ;
  rdfs:comment "A more complete description of the calendar component, than  that provided by the ncal:summary property.Inspired by RFC 2445 sec. 4.8.1.5 with following reservations:  the LANGUAGE parameter has been discarded. Please use xml:lang literals to express language. For the ALTREP parameter use the descriptionAltRep property." ;
  rdfs:domain ncal:UnionOfAlarmEventJournalTodo ;
  rdfs:label "description" ;
  rdfs:range xsd:string ;
  rdfs:subPropertyOf <http://www.semanticdesktop.org/ontologies/2007/01/19/nie#description> ;
.
ncal:descriptionAltRep
  rdf:type owl:ObjectProperty ;
  rdfs:comment """Alternate representation of the calendar entity description. Introduced to cover 
the ALTREP parameter of the DESCRIPTION property. See 
documentation of ncal:description for details.""" ;
  rdfs:domain ncal:UnionOfAlarmEventJournalTodo ;
  rdfs:label "descriptionAltRep" ;
  rdfs:range rdfs:Resource ;
.
ncal:dir
  rdf:type owl:ObjectProperty ;
  rdfs:comment "Specifies a reference to a directory entry associated with the calendar user specified by the property. Inspired by RFC 2445 sec. 4.2.6. Originally the data type of the value of this parameter was URI (Usually an LDAP URI). This has been expressed as rdfs:resource." ;
  rdfs:domain ncal:AttendeeOrOrganizer ;
  rdfs:label "dir" ;
  rdfs:range rdfs:Resource ;
.
ncal:displayAction
  rdf:type ncal:AlarmAction ;
  rdf:type owl:NamedIndividual ;
  rdfs:label "displayAction" ;
.
ncal:draftStatus
  rdf:type ncal:JournalStatus ;
  rdf:type owl:NamedIndividual ;
  rdfs:label "draftStatus" ;
.
ncal:dtend
  rdf:type owl:ObjectProperty ;
  nrl:maxCardinality 1 ;
  rdfs:comment "This property specifies the date and time that a calendar component ends. Inspired by RFC 2445 sec. 4.8.2.2" ;
  rdfs:domain ncal:UnionOfEventFreebusy ;
  rdfs:label "dtend" ;
  rdfs:range ncal:NcalDateTime ;
.
ncal:dtstamp
  rdf:type owl:DatatypeProperty ;
  nrl:maxCardinality 1 ;
  rdfs:comment "The property indicates the date/time that the instance of the iCalendar object was created. Inspired by RFC 2445 sec. 4.8.7.1. Note that the RFC allows ONLY UTC values for this property." ;
  rdfs:domain ncal:UnionOfEventFreebusyJournalTodo ;
  rdfs:label "dtstamp" ;
  rdfs:range xsd:dateTime ;
.
ncal:dtstart
  rdf:type owl:ObjectProperty ;
  nrl:maxCardinality 1 ;
  rdfs:comment "This property specifies when the calendar component begins. Inspired by RFC 2445 sec. 4.8.2.4" ;
  rdfs:domain ncal:UnionOfTimezoneObservanceEventFreebusyTimezoneTodo ;
  rdfs:label "dtstart" ;
  rdfs:range ncal:NcalDateTime ;
.
ncal:due
  rdf:type owl:ObjectProperty ;
  nrl:maxCardinality 1 ;
  rdfs:comment "This property defines the date and time that a to-do is expected to be completed. Inspired by RFC 2445 sec. 4.8.2.3" ;
  rdfs:domain ncal:Todo ;
  rdfs:label "due" ;
  rdfs:range ncal:NcalDateTime ;
.
ncal:duration
  rdf:type owl:DatatypeProperty ;
  nrl:maxCardinality 1 ;
  rdfs:comment "The property specifies a positive duration of time. Inspired by RFC 2445 sec. 4.8.2.5" ;
  rdfs:domain ncal:UnionOfAlarmEventFreebusyTodo ;
  rdfs:label "duration" ;
  rdfs:range xsd:duration ;
.
ncal:emailAction
  rdf:type ncal:AlarmAction ;
  rdf:type owl:NamedIndividual ;
  rdfs:label "emailAction" ;
.
ncal:encoding
  rdf:type owl:ObjectProperty ;
  nrl:maxCardinality 1 ;
  rdfs:comment "To specify an alternate inline encoding for the property value. Inspired by RFC 2445 sec. 4.2.7. Originally this property had a limited vocabulary. ('8BIT' and 'BASE64'). The terms of this vocabulary have been expressed as instances of the AttachmentEncoding class" ;
  rdfs:domain ncal:Attachment ;
  rdfs:label "encoding" ;
  rdfs:range ncal:AttachmentEncoding ;
.
ncal:endTriggerRelation
  rdf:type ncal:TriggerRelation ;
  rdf:type owl:NamedIndividual ;
  rdfs:label "endTriggerRelation" ;
.
ncal:eventStatus
  rdf:type owl:ObjectProperty ;
  nrl:maxCardinality 1 ;
  rdfs:comment "Defines the overall status or confirmation for an Event. Based on the STATUS property defined in RFC 2445 sec. 4.8.1.11." ;
  rdfs:domain ncal:Event ;
  rdfs:label "status" ;
  rdfs:range ncal:EventStatus ;
.
ncal:exdate
  rdf:type owl:ObjectProperty ;
  rdfs:comment "This property defines the list of date/time exceptions for a recurring calendar component. Inspired by RFC 2445 sec. 4.8.5.1" ;
  rdfs:domain ncal:UnionOfEventJournalTimezoneTodo ;
  rdfs:label "exdate" ;
  rdfs:range ncal:NcalDateTime ;
.
ncal:exrule
  rdf:type owl:ObjectProperty ;
  rdfs:comment "This property defines a rule or repeating pattern for an exception to a recurrence set. Inspired by RFC 2445 sec. 4.8.5.2." ;
  rdfs:domain ncal:UnionOfEventJournalTodo ;
  rdfs:label "exrule" ;
  rdfs:range ncal:RecurrenceRule ;
.
ncal:fbtype
  rdf:type owl:ObjectProperty ;
  nrl:maxCardinality 1 ;
  rdfs:comment "To specify the free or busy time type. Inspired by RFC 2445 sec. 4.2.9. The RFC specified a limited vocabulary for the values of this property. The terms of this vocabulary have been expressed as instances of the FreebusyType class. The user can use instances provided with this ontology or create his own." ;
  rdfs:domain ncal:FreebusyPeriod ;
  rdfs:label "fbtype" ;
  rdfs:range ncal:FreebusyType ;
.
ncal:finalStatus
  rdf:type ncal:JournalStatus ;
  rdf:type owl:NamedIndividual ;
  rdfs:label "finalStatus" ;
.
ncal:fmttype
  rdf:type owl:DatatypeProperty ;
  nrl:maxCardinality 1 ;
  rdfs:comment "To specify the content type of a referenced object. Inspired by RFC 2445 sec. 4.2.8. The value of this property should be an IANA-registered content type (e.g. application/binary)" ;
  rdfs:domain ncal:Attachment ;
  rdfs:label "fmttype" ;
  rdfs:range xsd:string ;
.
ncal:freeFreebusyType
  rdf:type ncal:FreebusyType ;
  rdf:type owl:NamedIndividual ;
  rdfs:label "freeFreebusyType" ;
.
ncal:freebusy
  rdf:type owl:ObjectProperty ;
  rdfs:comment "The property defines one or more free or busy time intervals. Inspired by RFC 2445 sec. 4.8.2.6. Note that the periods specified by this property can only be expressed with UTC times. Originally this property could have many comma-separated values. Please use a separate triple for each value." ;
  rdfs:domain ncal:Freebusy ;
  rdfs:label "freebusy" ;
  rdfs:range ncal:FreebusyPeriod ;
.
ncal:freq
  rdf:type owl:ObjectProperty ;
  nrl:maxCardinality 1 ;
  rdfs:comment "Frequency of a recurrence rule. Defined in RFC 2445 sec. 4.3.10" ;
  rdfs:domain ncal:RecurrenceRule ;
  rdfs:label "freq" ;
  rdfs:range ncal:RecurrenceFrequency ;
.
ncal:friday
  rdf:type ncal:Weekday ;
  rdf:type owl:NamedIndividual ;
  rdfs:label "friday" ;
.
ncal:geo
  rdf:type owl:ObjectProperty ;
  nrl:maxCardinality 1 ;
  rdfs:comment "This property specifies information related to the global position for the activity specified by a calendar component. Inspired by RFC 2445 sec. 4.8.1.6" ;
  rdfs:domain ncal:UnionOfEventTodo ;
  rdfs:label "geo" ;
  rdfs:range <http://www.w3.org/2003/01/geo/wgs84_pos#Point> ;
.
ncal:gregorianCalendarScale
  rdf:type ncal:CalendarScale ;
  rdf:type owl:NamedIndividual ;
  rdfs:label "gregorianCalendarScale" ;
.
ncal:groupUserType
  rdf:type ncal:CalendarUserType ;
  rdf:type owl:NamedIndividual ;
  rdfs:label "groupUserType" ;
.
ncal:hasAlarm
  rdf:type owl:AnnotationProperty ;
  rdf:type owl:ObjectProperty ;
  rdfs:comment "Links an event or a todo with a DataObject that can be interpreted as an alarm. This property has no direct equivalent in the RFC 2445. It has been provided to express this relation." ;
  rdfs:domain ncal:UnionOfEventTodo ;
  rdfs:label "hasAlarm" ;
  rdfs:range ncal:CalendarDataObject ;
  rdfs:subPropertyOf <http://www.semanticdesktop.org/ontologies/2007/01/19/nie#hasPart> ;
.
ncal:hourly
  rdf:type ncal:RecurrenceFrequency ;
  rdf:type owl:NamedIndividual ;
  rdfs:label "hourly" ;
.
ncal:inProcessParticipationStatus
  rdf:type ncal:ParticipationStatus ;
  rdf:type owl:NamedIndividual ;
  rdfs:label "inProcessParticipationStatus" ;
.
ncal:inProcessStatus
  rdf:type ncal:TodoStatus ;
  rdf:type owl:NamedIndividual ;
  rdfs:label "inProcessStatus" ;
.
ncal:individualUserType
  rdf:type ncal:CalendarUserType ;
  rdf:type owl:NamedIndividual ;
  rdfs:label "individualUserType" ;
.
ncal:interval
  rdf:type owl:DatatypeProperty ;
  nrl:maxCardinality 1 ;
  rdfs:comment "The INTERVAL rule part contains a positive integer representing how often the recurrence rule repeats. The default value is \"1\", meaning every second for a SECONDLY rule, or every minute for a MINUTELY rule, every hour for an HOURLY rule, every day for a DAILY rule, every week for a WEEKLY rule, every month for a MONTHLY rule andevery year for a YEARLY rule. Defined in RFC 2445 sec. 4.3.10" ;
  rdfs:domain ncal:RecurrenceRule ;
  rdfs:label "interval" ;
  rdfs:range xsd:integer ;
.
ncal:involvedContact
  rdf:type owl:ObjectProperty ;
  rdfs:comment "A contact of the Attendee or the organizer involved in an event or other calendar entity. This property has been introduced to express the actual value of the ATTENDEE and ORGANIZER properties. The contact will also represent the CN parameter of those properties. See documentation of ncal:attendee or ncal:organizer for more details." ;
  rdfs:domain ncal:AttendeeOrOrganizer ;
  rdfs:label "involvedContact" ;
  rdfs:range <http://www.semanticdesktop.org/ontologies/2007/03/22/nco#Contact> ;
.
ncal:journalStatus
  rdf:type owl:ObjectProperty ;
  nrl:maxCardinality 1 ;
  rdfs:comment "Defines the overall status or confirmation for a journal entry. Based on the STATUS property defined in RFC 2445 sec. 4.8.1.11." ;
  rdfs:domain ncal:Journal ;
  rdfs:label "status" ;
  rdfs:range ncal:JournalStatus ;
.
ncal:lastModified
  rdf:type owl:DatatypeProperty ;
  nrl:maxCardinality 1 ;
  rdfs:comment "The property specifies the date and time that the information associated with the calendar component was last revised in the calendar store. Note: This is analogous to the modification date and time for a file in the file system. Inspired by RFC 2445 sec. 4.8.7.3. Note that the RFC allows ONLY UTC time values for this property." ;
  rdfs:domain ncal:UnionOfEventJournalTimezoneTodo ;
  rdfs:label "lastModified" ;
  rdfs:range xsd:dateTime ;
.
ncal:location
  rdf:type owl:DatatypeProperty ;
  nrl:maxCardinality 1 ;
  rdfs:comment "Defines the intended venue for the activity defined by a calendar component. Inspired by RFC 2445 sec 4.8.1.7 with the following reservations:  the LANGUAGE parameter has been discarded. Please use xml:lang literals to express language.  For the ALTREP parameter use the locationAltRep property." ;
  rdfs:domain ncal:UnionOfEventTodo ;
  rdfs:label "location" ;
  rdfs:range xsd:string ;
.
ncal:locationAltRep
  rdf:type owl:ObjectProperty ;
  rdfs:comment """Alternate representation of the event or todo location. 
Introduced to cover the ALTREP parameter of the LOCATION 
property. See documentation of ncal:location for details.""" ;
  rdfs:domain ncal:UnionOfEventTodo ;
  rdfs:label "locationAltRep" ;
  rdfs:range rdfs:Resource ;
.
ncal:member
  rdf:type owl:ObjectProperty ;
  rdfs:comment "To specify the group or list membership of the calendar user specified by the property. Inspired by RFC 2445 sec. 4.2.11. Originally this parameter had a value type of CAL-ADDRESS. This has been expressed as nco:Contact to promote integration between NCAL and NCO" ;
  rdfs:domain ncal:Attendee ;
  rdfs:label "member" ;
  rdfs:range <http://www.semanticdesktop.org/ontologies/2007/03/22/nco#Contact> ;
.
ncal:method
  rdf:type owl:DatatypeProperty ;
  nrl:maxCardinality 1 ;
  rdfs:comment "This property defines the iCalendar object method associated with the calendar object. Defined in RFC 2445 sec. 4.7.2" ;
  rdfs:domain ncal:Calendar ;
  rdfs:label "method" ;
  rdfs:range xsd:string ;
.
ncal:minutely
  rdf:type ncal:RecurrenceFrequency ;
  rdf:type owl:NamedIndividual ;
  rdfs:label "minutely" ;
.
ncal:monday
  rdf:type ncal:Weekday ;
  rdf:type owl:NamedIndividual ;
  rdfs:label "monday" ;
.
ncal:monthly
  rdf:type ncal:RecurrenceFrequency ;
  rdf:type owl:NamedIndividual ;
  rdfs:label "monthly" ;
.
ncal:ncalRelation
  rdf:type owl:AnnotationProperty ;
  rdf:type owl:DatatypeProperty ;
  rdfs:comment "A common superproperty for all types of ncal relations. It is not to be used directly." ;
  rdfs:domain ncal:UnionOfEventJournalTodo ;
  rdfs:label "ncalRelation" ;
  rdfs:range xsd:string ;
  rdfs:subPropertyOf dc:relation ;
.
ncal:ncalTimezone
  rdf:type owl:ObjectProperty ;
  nrl:maxCardinality 1 ;
  rdfs:comment "The timezone instance that should be used to interpret an NcalDateTime. The purpose of this property is similar to the TZID parameter specified in RFC 2445 sec. 4.2.19" ;
  rdfs:domain ncal:NcalDateTime ;
  rdfs:label "ncalTimezone" ;
  rdfs:range ncal:Timezone ;
.
ncal:needsActionParticipationStatus
  rdf:type ncal:ParticipationStatus ;
  rdf:type owl:NamedIndividual ;
  rdfs:label "needsActionParticipationStatus" ;
.
ncal:needsActionStatus
  rdf:type ncal:TodoStatus ;
  rdf:type owl:NamedIndividual ;
  rdfs:label "needsActionStatus" ;
.
ncal:nonParticipantRole
  rdf:type ncal:AttendeeRole ;
  rdf:type owl:NamedIndividual ;
  rdfs:label "nonParticipantRole" ;
.
ncal:opaqueTransparency
  rdf:type ncal:TimeTransparency ;
  rdf:type owl:NamedIndividual ;
  rdfs:label "opaqueTransparency" ;
.
ncal:optParticipantRole
  rdf:type ncal:AttendeeRole ;
  rdf:type owl:NamedIndividual ;
  rdfs:label "optParticipantRole" ;
.
ncal:organizer
  rdf:type owl:ObjectProperty ;
  rdfs:comment "The property defines the organizer for a calendar component. Inspired by RFC 2445 sec. 4.8.4.3. Originally this property accepted many parameters. The Organizer class has been introduced to express them all. Note that NCAL is aligned with NCO. The actual value (of the CAL-ADDRESS type) is expressed as an instance of nco:Contact. Remember that the CN parameter has been removed from NCAL. Instead that value should be expressed using nco:fullname property of the above mentioned nco:Contact instance." ;
  rdfs:domain ncal:UnionOfEventFreebusyJournalTodo ;
  rdfs:label "organizer" ;
  rdfs:range ncal:Organizer ;
.
ncal:partstat
  rdf:type owl:ObjectProperty ;
  rdfs:comment "To specify the participation status for the calendar user specified by the property. Inspired by RFC 2445 sec. 4.2.12. Originally this parameter had three sets of allowed values. Which set applied to a particular case - depended on the type of calendar entity this parameter occured in. (event, todo, journal entry). This would be awkward to model in RDF so a single ParticipationStatus class has been introduced. Terms of the values vocabulary are expressed as instances of this class. Users are advised to pay attention which instances they use." ;
  rdfs:domain ncal:Attendee ;
  rdfs:label "partstat" ;
  rdfs:range ncal:ParticipationStatus ;
.
ncal:percentComplete
  rdf:type owl:DatatypeProperty ;
  rdfs:comment "This property is used by an assignee or delegatee of a to-do to convey the percent completion of a to-do to the Organizer. Inspired by RFC 2445 sec. 4.8.1.8" ;
  rdfs:domain ncal:Todo ;
  rdfs:label "percentComplete" ;
  rdfs:range xsd:integer ;
.
ncal:periodBegin
  rdf:type owl:DatatypeProperty ;
  nrl:maxCardinality 1 ;
  rdfs:comment "Beginng of a period. Inspired by the first part of a structured value of the PERIOD datatype specified in RFC 2445 sec. 4.3.9" ;
  rdfs:domain ncal:NcalPeriod ;
  rdfs:label "periodBegin" ;
  rdfs:range xsd:dateTime ;
.
ncal:periodDuration
  rdf:type owl:DatatypeProperty ;
  nrl:maxCardinality 1 ;
  rdfs:comment "Duration of a period of time. Inspired by the second part of a structured value of the PERIOD datatype specified in RFC 2445 sec. 4.3.9. Note that a single NcalPeriod instance shouldn't have the periodEnd and periodDuration properties specified simultaneously." ;
  rdfs:domain ncal:NcalPeriod ;
  rdfs:label "periodDuration" ;
  rdfs:range xsd:duration ;
.
ncal:periodEnd
  rdf:type owl:DatatypeProperty ;
  nrl:maxCardinality 1 ;
  rdfs:comment "End of a period of time. Inspired by the second part of a structured value of a PERIOD datatype specified in RFC 2445 sec. 4.3.9. Note that a single NcalPeriod instance shouldn't have the periodEnd and periodDuration properties specified simultaneously." ;
  rdfs:domain ncal:NcalPeriod ;
  rdfs:label "periodEnd" ;
  rdfs:range xsd:dateTime ;
.
ncal:priority
  rdf:type owl:DatatypeProperty ;
  nrl:maxCardinality 1 ;
  rdfs:comment "The property defines the relative priority for a calendar component. Inspired by RFC 2445 sec. 4.8.1.9" ;
  rdfs:domain ncal:UnionOfEventTodo ;
  rdfs:label "priority" ;
  rdfs:range xsd:integer ;
.
ncal:privateClassification
  rdf:type ncal:AccessClassification ;
  rdf:type owl:NamedIndividual ;
  rdfs:label "privateClassification" ;
.
ncal:procedureAction
  rdf:type ncal:AlarmAction ;
  rdf:type owl:NamedIndividual ;
  rdfs:label "procedureAction" ;
.
ncal:prodid
  rdf:type owl:AnnotationProperty ;
  rdf:type owl:DatatypeProperty ;
  rdfs:comment "This property specifies the identifier for the product that created the iCalendar object. Defined in RFC 2445 sec. 4.7.2" ;
  rdfs:domain ncal:Calendar ;
  rdfs:label "prodid" ;
  rdfs:range xsd:string ;
  rdfs:subPropertyOf <http://www.semanticdesktop.org/ontologies/2007/01/19/nie#generator> ;
.
ncal:publicClassification
  rdf:type ncal:AccessClassification ;
  rdf:type owl:NamedIndividual ;
  rdfs:label "publicClassification" ;
.
ncal:range
  rdf:type owl:ObjectProperty ;
  nrl:maxCardinality 1 ;
  rdfs:comment "To specify the effective range of recurrence instances from the instance specified by the recurrence identifier specified by the property. It is intended to express the RANGE parameter specified in RFC 2445 sec. 4.2.13. The set of possible values for this property is limited. See also the documentation for ncal:recurrenceId for more details." ;
  rdfs:domain ncal:RecurrenceIdentifier ;
  rdfs:label "range" ;
  rdfs:range ncal:RecurrenceIdentifierRange ;
.
ncal:rdate
  rdf:type owl:ObjectProperty ;
  rdfs:comment "This property defines the list of date/times for a recurrence set. Inspired by RFC 2445 sec. 4.8.5.3. Note that RFC allows both DATE, DATE-TIME and PERIOD values for this property. That's why the range has been set to NcalTimeEntity." ;
  rdfs:domain ncal:UnionOfTimezoneObservanceEventJournalTimezoneTodo ;
  rdfs:label "rdate" ;
  rdfs:range ncal:NcalTimeEntity ;
.
ncal:recurrenceId
  rdf:type owl:ObjectProperty ;
  nrl:maxCardinality 1 ;
  rdfs:comment "This property is used in conjunction with the \"UID\" and \"SEQUENCE\" property to identify a specific instance of a recurring \"VEVENT\", \"VTODO\" or \"VJOURNAL\" calendar component. The property value is the effective value of the \"DTSTART\" property of the recurrence instance. Inspired by the RFC 2445 sec. 4.8.4.4" ;
  rdfs:domain ncal:UnionOfEventJournalTimezoneTodo ;
  rdfs:label "recurrenceId" ;
  rdfs:range ncal:RecurrenceIdentifier ;
.
ncal:recurrenceIdDateTime
  rdf:type owl:ObjectProperty ;
  nrl:maxCardinality 1 ;
  rdfs:comment "The date and time of a recurrence identifier. Provided to express the actual value of the ncal:recurrenceId property. See documentation for ncal:recurrenceId for details." ;
  rdfs:domain ncal:RecurrenceIdentifier ;
  rdfs:label "recurrenceIdDateTime" ;
  rdfs:range ncal:NcalDateTime ;
.
ncal:related
  rdf:type owl:ObjectProperty ;
  rdfs:comment "To specify the relationship of the alarm trigger with respect to the start or end of the calendar component. Inspired by RFC 2445 4.2.14. The RFC has specified two possible values for this property ('START' and 'END') they have been expressed as instances of the TriggerRelation class." ;
  rdfs:domain ncal:Trigger ;
  rdfs:label "related" ;
  rdfs:range ncal:TriggerRelation ;
.
ncal:relatedToChild
  rdf:type owl:DatatypeProperty ;
  rdfs:comment "The property is used to represent a relationship or reference between one calendar component and another. Inspired by RFC 2445 sec. 4.8.4.5. Originally this property had a RELTYPE parameter. It has been decided to introduce three different properties to express the values of that parameter. This property expresses the RELATED-TO property with RELTYPE=CHILD parameter." ;
  rdfs:domain ncal:UnionOfEventJournalTodo ;
  rdfs:label "relatedToChild" ;
  rdfs:range xsd:string ;
  rdfs:subPropertyOf ncal:ncalRelation ;
.
ncal:relatedToParent
  rdf:type owl:DatatypeProperty ;
  rdfs:comment "The property is used to represent a relationship or reference between one calendar component and another. Inspired by RFC 2445 sec. 4.8.4.5. Originally this property had a RELTYPE parameter. It has been decided that it is more natural to introduce three different properties to express the values of that parameter. This property expresses the RELATED-TO property with no RELTYPE parameter (the default value is PARENT), or with explicit RELTYPE=PARENT parameter." ;
  rdfs:domain ncal:UnionOfEventJournalTodo ;
  rdfs:label "relatedToParent" ;
  rdfs:range xsd:string ;
  rdfs:subPropertyOf ncal:ncalRelation ;
.
ncal:relatedToSibling
  rdf:type owl:DatatypeProperty ;
  rdfs:comment "The property is used to represent a relationship or reference between one calendar component and another. Inspired by RFC 2445 sec. 4.8.4.5. Originally this property had a RELTYPE parameter. It has been decided that it is more natural to introduce three different properties to express the values of that parameter. This property expresses the RELATED-TO property with RELTYPE=SIBLING parameter." ;
  rdfs:domain ncal:UnionOfEventJournalTodo ;
  rdfs:label "relatedToSibling" ;
  rdfs:range xsd:string ;
  rdfs:subPropertyOf ncal:ncalRelation ;
.
ncal:repeat
  rdf:type owl:DatatypeProperty ;
  nrl:maxCardinality 1 ;
  rdfs:comment "This property defines the number of time the alarm should be repeated, after the initial trigger. Inspired by RFC 2445 sec. 4.8.6.2" ;
  rdfs:domain ncal:Alarm ;
  rdfs:label "repeat" ;
  rdfs:range xsd:integer ;
.
ncal:reqParticipantRole
  rdf:type ncal:AttendeeRole ;
  rdf:type owl:NamedIndividual ;
  rdfs:label "reqParticipantRole" ;
.
ncal:requestStatus
  rdf:type owl:ObjectProperty ;
  nrl:maxCardinality 1 ;
  rdfs:comment "This property defines the status code returned for a scheduling request. Inspired by RFC 2445 sec. 4.8.8.2. Original value of this property was a four-element structure. The RequestStatus class has been introduced to express it. In RFC 2445 this property could have the LANGUAGE parameter. This has been discarded in this ontology. Use xml:lang literals to express it if necessary." ;
  rdfs:domain ncal:UnionOfEventFreebusyJournalTodo ;
  rdfs:label "requestStatus" ;
  rdfs:range ncal:RequestStatus ;
.
ncal:requestStatusData
  rdf:type owl:DatatypeProperty ;
  rdfs:comment "Additional data associated with a request status. Inspired by the third part of the structured value for the REQUEST-STATUS property defined in RFC 2445 sec. 4.8.8.2 (\"Textual exception data. For example, the offending property name and value or complete property line\")" ;
  rdfs:domain ncal:RequestStatus ;
  rdfs:label "requestStatusData" ;
  rdfs:range xsd:string ;
.
ncal:resourceUserType
  rdf:type ncal:CalendarUserType ;
  rdf:type owl:NamedIndividual ;
  rdfs:label "resourceUserType" ;
.
ncal:resources
  rdf:type owl:DatatypeProperty ;
  rdfs:comment "Defines the equipment or resources anticipated for an activity specified by a calendar entity. Inspired by RFC 2445 sec. 4.8.1.10 with the following reservations:  the LANGUAGE parameter has been discarded. Please use xml:lang literals to express language. For the ALTREP parameter use the resourcesAltRep property. This property specifies multiple resources. The order is not important. it is recommended to introduce a separate triple for each resource." ;
  rdfs:domain ncal:UnionOfEventTodo ;
  rdfs:label "resources" ;
  rdfs:range xsd:string ;
.
ncal:resourcesAltRep
  rdf:type owl:ObjectProperty ;
  rdfs:comment "Alternate representation of the resources needed for an event or todo. Introduced to cover the ALTREP parameter of the resources property. See documentation for ncal:resources for details." ;
  rdfs:domain ncal:UnionOfEventTodo ;
  rdfs:label "resourcesAltRep" ;
  rdfs:range rdfs:Resource ;
.
ncal:returnStatus
  rdf:type owl:DatatypeProperty ;
  nrl:maxCardinality 1 ;
  rdfs:comment """Short return status. Inspired by the first element of the structured value of the REQUEST-STATUS property described in RFC 2445 sec. 4.8.8.2.

The short return status is a PERIOD character (US-ASCII decimal 46) separated 3-tuple of integers. For example, \"3.1.1\". The successive  levels of integers provide for a successive level of status code granularity.

The following are initial classes for the return status code. Individual iCalendar object methods will define specific return status codes for these classes. In addition, other classes for the return status code may be defined using the registration process defined later in this memo.

 1.xx - Preliminary success. This class of status of status code indicates that the request has request has been initially processed but that completion is pending.

2.xx -Successful. This class of status code indicates that the request was completed successfuly. However, the exact status code can indicate that a fallback has been taken.

3.xx - Client Error. This class of status code indicates that the request was not successful. The error is the result of either a syntax or a semantic error in the client formatted request. Request should not be retried until the condition in the request is corrected.

4.xx - Scheduling Error. This class of status code indicates that the request was not successful. Some sort of error occurred within the  calendaring and scheduling service, not directly related to the request itself.""" ;
  rdfs:domain ncal:RequestStatus ;
  rdfs:label "returnStatus" ;
  rdfs:range xsd:string ;
.
ncal:role
  rdf:type owl:ObjectProperty ;
  rdfs:comment "To specify the participation role for the calendar user specified by the property. Inspired by the RFC 2445 sec. 4.2.16. Originally this property had a limited vocabulary for values. The terms of that vocabulary have been expressed as instances of the AttendeeRole class." ;
  rdfs:domain ncal:Attendee ;
  rdfs:label "role" ;
  rdfs:range ncal:AttendeeRole ;
.
ncal:roomUserType
  rdf:type ncal:CalendarUserType ;
  rdf:type owl:NamedIndividual ;
  rdfs:label "roomUserType" ;
.
ncal:rrule
  rdf:type owl:ObjectProperty ;
  rdfs:comment "This property defines a rule or repeating pattern for recurring events, to-dos, or time zone definitions. sec. 4.8.5.4" ;
  rdfs:domain ncal:UnionOfTimezoneObservanceEventJournalTimezoneTodo ;
  rdfs:label "rrule" ;
  rdfs:range ncal:RecurrenceRule ;
.
ncal:rsvp
  rdf:type owl:DatatypeProperty ;
  nrl:maxCardinality 1 ;
  rdfs:comment "To specify whether there is an expectation of a favor of a reply from the calendar user specified by the property value. Inspired by RFC 2445 sec. 4.2.17" ;
  rdfs:domain ncal:Attendee ;
  rdfs:label "rsvp" ;
  rdfs:range xsd:boolean ;
.
ncal:saturday
  rdf:type ncal:Weekday ;
  rdf:type owl:NamedIndividual ;
  rdfs:label "saturday" ;
.
ncal:secondly
  rdf:type ncal:RecurrenceFrequency ;
  rdf:type owl:NamedIndividual ;
  rdfs:label "secondly" ;
.
ncal:sentBy
  rdf:type owl:ObjectProperty ;
  rdfs:comment "To specify the calendar user that is acting on behalf of the calendar user specified by the property. Inspired by RFC 2445 sec. 4.2.18. The original data type of this property was a mailto: URI. This has been changed to nco:Contact to promote integration between NCO and NCAL." ;
  rdfs:domain ncal:AttendeeOrOrganizer ;
  rdfs:label "sentBy" ;
  rdfs:range <http://www.semanticdesktop.org/ontologies/2007/03/22/nco#Contact> ;
.
ncal:sequence
  rdf:type owl:DatatypeProperty ;
  nrl:maxCardinality 1 ;
  rdfs:comment "This property defines the revision sequence number of the calendar component within a sequence of revisions. Inspired by RFC 2445 sec. 4.8.7.4" ;
  rdfs:domain ncal:UnionOfEventJournalTodo ;
  rdfs:label "sequence" ;
  rdfs:range xsd:integer ;
.
ncal:standard
  rdf:type owl:ObjectProperty ;
  nrl:maxCardinality 1 ;
  rdfs:comment "Links the timezone with the standard timezone observance. This property has no direct equivalent in the RFC 2445. It has been inspired by the structure of the Vtimezone component defined in sec.4.6.5" ;
  rdfs:domain ncal:Timezone ;
  rdfs:label "standard" ;
  rdfs:range ncal:TimezoneObservance ;
.
ncal:startTriggerRelation
  rdf:type ncal:TriggerRelation ;
  rdf:type owl:NamedIndividual ;
  rdfs:label "startTriggerRelation" ;
.
ncal:statusDescription
  rdf:type owl:DatatypeProperty ;
  nrl:maxCardinality 1 ;
  rdfs:comment "Longer return status description. Inspired by the second part of the structured value of the REQUEST-STATUS property defined in RFC 2445 sec. 4.8.8.2" ;
  rdfs:domain ncal:RequestStatus ;
  rdfs:label "statusDescription" ;
  rdfs:range xsd:string ;
.
ncal:summary
  rdf:type owl:DatatypeProperty ;
  rdfs:comment "Defines a short summary or subject for the calendar component. Inspired by RFC 2445 sec 4.8.1.12 with the following reservations: the LANGUAGE parameter has been discarded. Please use xml:lang literals to express language. For the ALTREP parameter use the summaryAltRep property." ;
  rdfs:domain ncal:UnionOfAlarmEventJournalTodo ;
  rdfs:label "summary" ;
  rdfs:range xsd:string ;
.
ncal:summaryAltRep
  rdf:type owl:ObjectProperty ;
  rdfs:comment """Alternate representation of the comment. Introduced to cover 
the ALTREP parameter of the SUMMARY property. See 
documentation of ncal:summary for details.""" ;
  rdfs:domain ncal:UnionOfAlarmEventJournalTodo ;
  rdfs:label "summaryAltRep" ;
  rdfs:range rdfs:Resource ;
.
ncal:sunday
  rdf:type ncal:Weekday ;
  rdf:type owl:NamedIndividual ;
  rdfs:label "sunday" ;
.
ncal:tentativeParticipationStatus
  rdf:type ncal:ParticipationStatus ;
  rdf:type owl:NamedIndividual ;
  rdfs:label "tentativeParticipationStatus" ;
.
ncal:tentativeStatus
  rdf:type ncal:EventStatus ;
  rdf:type owl:NamedIndividual ;
  rdfs:label "tentativeStatus" ;
.
ncal:thisAndFutureRange
  rdf:type ncal:RecurrenceIdentifierRange ;
  rdf:type owl:NamedIndividual ;
  rdfs:label "thisAndFutureRange" ;
.
ncal:thisAndPriorRange
  rdf:type ncal:RecurrenceIdentifierRange ;
  rdf:type owl:NamedIndividual ;
  rdfs:label "thisAndPriorRange" ;
.
ncal:thursday
  rdf:type ncal:Weekday ;
  rdf:type owl:NamedIndividual ;
  rdfs:label "thursday" ;
.
ncal:todoStatus
  rdf:type owl:ObjectProperty ;
  nrl:maxCardinality 1 ;
  rdfs:comment "Defines the overall status or confirmation for a todo. Based on the STATUS property defined in RFC 2445 sec. 4.8.1.11." ;
  rdfs:domain ncal:Todo ;
  rdfs:label "status" ;
  rdfs:range ncal:TodoStatus ;
.
ncal:transp
  rdf:type owl:ObjectProperty ;
  nrl:maxCardinality 1 ;
  rdfs:comment "Defines whether an event is transparent or not  to busy time searches. Inspired by RFC 2445 sec.4.8.2.7. Values for this property can be chosen from a limited vocabulary. To express this a TimeTransparency class has been introduced." ;
  rdfs:domain ncal:Event ;
  rdfs:label "transp" ;
  rdfs:range ncal:TimeTransparency ;
.
ncal:transparentTransparency
  rdf:type ncal:TimeTransparency ;
  rdf:type owl:NamedIndividual ;
  rdfs:label "transparentTransparency" ;
.
ncal:trigger
  rdf:type owl:ObjectProperty ;
  rdfs:comment "This property specifies when an alarm will trigger. Inspired by RFC 2445 sec. 4.8.6.3 Originally the value of this property could accept two types : duration and date-time. To express this fact a Trigger class has been introduced. It also has a related property to account for the RELATED parameter." ;
  rdfs:domain ncal:UnionOfAlarmEventTodo ;
  rdfs:label "trigger" ;
  rdfs:range ncal:Trigger ;
.
ncal:triggerDateTime
  rdf:type owl:DatatypeProperty ;
  nrl:maxCardinality 1 ;
  rdfs:comment "The exact date and time of the trigger. This property has been created to express the VALUE=DATE, and VALUE=DATE-TIME parameters of the TRIGGER property. See the documentation for ncal:trigger for more details" ;
  rdfs:domain ncal:Trigger ;
  rdfs:label "triggerDateTime" ;
  rdfs:range xsd:dateTime ;
.
ncal:triggerDuration
  rdf:type owl:DatatypeProperty ;
  nrl:maxCardinality 1 ;
  rdfs:comment "The duration of a trigger. This property has been created to express the VALUE=DURATION parameter of the TRIGGER property. See documentation for ncal:trigger for more details." ;
  rdfs:domain ncal:Trigger ;
  rdfs:label "triggerDuration" ;
  rdfs:range xsd:duration ;
.
ncal:tuesday
  rdf:type ncal:Weekday ;
  rdf:type owl:NamedIndividual ;
  rdfs:label "tuesday" ;
.
ncal:tzid
  rdf:type owl:DatatypeProperty ;
  nrl:maxCardinality 1 ;
  rdfs:comment "This property specifies the text value that uniquely identifies the \"VTIMEZONE\" calendar component. Inspired by RFC 2445 sec 4.8.3.1" ;
  rdfs:domain ncal:Timezone ;
  rdfs:label "tzid" ;
  rdfs:range xsd:string ;
.
ncal:tzname
  rdf:type owl:DatatypeProperty ;
  rdfs:comment "Specifies the customary designation for a timezone description. Inspired by RFC 2445 sec. 4.8.3.2 The LANGUAGE parameter has been discarded. Please xml:lang literals to express languages. Original specification for the domain of this property stated that it must appear within the timezone component. In this ontology the TimezoneObservance class has been itroduced to clarify this specification." ;
  rdfs:domain ncal:TimezoneObservance ;
  rdfs:label "tzname" ;
  rdfs:range xsd:string ;
.
ncal:tzoffsetfrom
  rdf:type owl:DatatypeProperty ;
  nrl:maxCardinality 1 ;
  rdfs:comment "This property specifies the offset which is in use prior to this time zone observance. Inspired by RFC 2445 sec. 4.8.3.3. The original domain was underspecified. It said that this property must appear within a Timezone component. In this ontology a TimezoneObservance class has been introduced to clarify this specification. The original range was UTC-OFFSET. There is no equivalent among the XSD datatypes so plain string was chosen." ;
  rdfs:domain ncal:TimezoneObservance ;
  rdfs:label "tzoffsetfrom" ;
  rdfs:range xsd:string ;
.
ncal:tzoffsetto
  rdf:type owl:DatatypeProperty ;
  nrl:maxCardinality 1 ;
  rdfs:comment "This property specifies the offset which is in use in this time zone observance. nspired by RFC 2445 sec. 4.8.3.4. The original domain was underspecified. It said that this property must appear within a Timezone component. In this ontology a TimezoneObservance class has been introduced to clarify this specification. The original range was UTC-OFFSET. There is no equivalent among the XSD datatypes so plain string was chosen." ;
  rdfs:domain ncal:TimezoneObservance ;
  rdfs:label "tzoffsetto" ;
  rdfs:range xsd:string ;
.
ncal:tzurl
  rdf:type owl:ObjectProperty ;
  rdfs:comment "The TZURL provides a means for a VTIMEZONE component to point to a network location that can be used to retrieve an up-to- date version of itself. Inspired by RFC 2445 sec. 4.8.3.5. Originally the range of this property had been specified as URI." ;
  rdfs:domain ncal:Timezone ;
  rdfs:label "tzurl" ;
  rdfs:range rdfs:Resource ;
.
ncal:uid
  rdf:type owl:AnnotationProperty ;
  rdf:type owl:DatatypeProperty ;
  nrl:maxCardinality 1 ;
  rdfs:comment "This property defines the persistent, globally unique identifier for the calendar component. Inspired by the RFC 2445 sec 4.8.4.7" ;
  rdfs:domain ncal:UnionOfEventFreebusyJournalTodo ;
  rdfs:label "uid" ;
  rdfs:range xsd:string ;
  rdfs:subPropertyOf <http://www.semanticdesktop.org/ontologies/2007/01/19/nie#identifier> ;
.
ncal:unknownUserType
  rdf:type ncal:CalendarUserType ;
  rdf:type owl:NamedIndividual ;
  rdfs:label "unknownUserType" ;
.
ncal:until
  rdf:type owl:DatatypeProperty ;
  rdfs:comment "The UNTIL rule part defines a date-time value which bounds the recurrence rule in an inclusive manner. If the value specified by UNTIL is synchronized with the specified recurrence, this date or date-time becomes the last instance of the recurrence. If specified as a date-time value, then it MUST be specified in an UTC time format. If not present, and the COUNT rule part is also not present, the RRULE is considered to repeat forever." ;
  rdfs:domain ncal:RecurrenceRule ;
  rdfs:label "until" ;
  rdfs:range xsd:dateTime ;
.
ncal:url
  rdf:type owl:ObjectProperty ;
  nrl:maxCardinality 1 ;
  rdfs:comment "This property defines a Uniform Resource Locator (URL) associated with the iCalendar object. Inspired by the RFC 2445 sec. 4.8.4.6. Original range had been specified as URI." ;
  rdfs:domain ncal:UnionOfEventFreebusyJournalTodo ;
  rdfs:label "url" ;
  rdfs:range rdfs:Resource ;
.
ncal:version
  rdf:type owl:AnnotationProperty ;
  rdf:type owl:DatatypeProperty ;
  rdfs:comment "This property specifies the identifier corresponding to the highest version number or the minimum and maximum range of the iCalendar specification that is required in order to interpret the iCalendar object. Defined in RFC 2445 sec. 4.7.4" ;
  rdfs:domain ncal:Calendar ;
  rdfs:label "version" ;
  rdfs:range xsd:string ;
  rdfs:subPropertyOf <http://www.semanticdesktop.org/ontologies/2007/01/19/nie#generatorOption> ;
.
ncal:wednesday
  rdf:type ncal:Weekday ;
  rdf:type owl:NamedIndividual ;
  rdfs:label "wednesday" ;
.
ncal:weekly
  rdf:type ncal:RecurrenceFrequency ;
  rdf:type owl:NamedIndividual ;
  rdfs:label "weekly" ;
.
ncal:wkst
  rdf:type owl:ObjectProperty ;
  nrl:maxCardinality 1 ;
  rdfs:comment "The day that's counted as the start of the week. It is used to disambiguate the byweekno rule. Defined in RFC 2445 sec. 4.3.10" ;
  rdfs:domain ncal:RecurrenceRule ;
  rdfs:label "wkst" ;
  rdfs:range ncal:Weekday ;
.
ncal:yearly
  rdf:type ncal:RecurrenceFrequency ;
  rdf:type owl:NamedIndividual ;
  rdfs:label "yearly" ;
.
nrl:maxCardinality
  rdf:type owl:AnnotationProperty ;
.
:Voice_1-type-vcard_Voice
  rdf:type rdf:Statement ;
  rdf:object vcard:Voice ;
  rdf:predicate rdf:type ;
  rdf:subject :Voice_1 ;
.
:Weekday_1-type-ncal_Weekday
  rdf:type rdf:Statement ;
  rdf:object ncal:Weekday ;
  rdf:predicate rdf:type ;
  rdf:subject :Weekday_1 ;
.
:Weekday_1-type-ncal_Weekday-type-rdf_Statement
  rdf:type rdf:Statement ;
  rdf:object rdf:Statement ;
  rdf:predicate rdf:type ;
  rdf:subject :Weekday_1-type-ncal_Weekday ;
.
rdfs:Class
  rdf:type owl:Class ;
.
rdfs:Resource
  rdf:type owl:Class ;
.
xsd:date
  rdf:type rdfs:Datatype ;
.
xsd:duration
  rdf:type rdfs:Datatype ;
.
<http://www.w3.org/2003/01/geo/wgs84_pos#Point>
  rdf:type owl:Class ;
.
skos:note
  rdf:type owl:AnnotationProperty ;
.
vcard:Contact_1
  rdf:type owl:NamedIndividual ;
  rdf:type vcard:Contact ;
  rdfs:label "Bill Smith"@en ;
.
vcard:Voice_1
  rdf:type vcard:Voice ;
.
vcard:Voice_2
  rdf:type vcard:Voice ;
.
vcard:hasEmail
  rdf:type owl:Class ;
.
vcard:hasTelephone
  rdf:type owl:Class ;
.
vcard:hasURL
  rdf:type owl:Class ;
.
vcard:url
  rdf:type owl:AnnotationProperty ;
  rdf:type owl:DatatypeProperty ;
.
org:identifier
  rdf:type owl:Class ;
.
airs:
  rdf:type owl:Ontology ;
  <http://purl.org/dc/elements/1.1/description> "The AIRS Linked Open Vocabulary is a way to describe human services information and referral (I&R) concepts.  AIRS is the Alliance of Information and Referral Services (airs.org), which possesses over 1,000 member agencies primarily in the United States and Canada.  The AIRS LOV is based on the AIRS XML Schema, available at: https://airs-xml.googlecode.com/hg/tags/3.1/airs.xsd"@en ;
  <http://purl.org/dc/elements/1.1/title> "The Alliance of Information and Referral Services (AIRS) Linked Open Vocabulary"^^xsd:string ;
  owl:imports dc: ;
  owl:imports appearances: ;
  owl:imports ncal: ;
  owl:imports vcard: ;
  owl:imports org: ;
  owl:priorVersion <http://github.com/airs-linked-data/lov/releases/v0.0.7/src/airs_vocabulary.ttl#> ;
  owl:versionIRI <http://github.com/airs-linked-data/lov/releases/v0.0.8/src/airs_vocabulary.ttl#> ;
.
airs:Address
  rdf:type owl:Class ;
  rdfs:comment "airs:hasDescription is a description of the physical location or other information pertinent to this address, and hasExplanationForNoPhysicalAddress clarifies why the address doesn't have a physical presence."@en ;
  rdfs:subClassOf owl:Thing ;
  rdfs:subClassOf vcard:Address ;
  rdfs:subClassOf [
      rdf:type owl:Restriction ;
      owl:allValuesFrom xsd:boolean ;
      owl:onProperty airs:isMailingAddress ;
    ] ;
  rdfs:subClassOf [
      rdf:type owl:Restriction ;
      owl:allValuesFrom xsd:boolean ;
      owl:onProperty airs:isPhysicalAddress ;
    ] ;
  rdfs:subClassOf [
      rdf:type owl:Restriction ;
      owl:allValuesFrom xsd:string ;
      owl:onProperty dct:description ;
    ] ;
  rdfs:subClassOf [
      rdf:type owl:Restriction ;
      owl:allValuesFrom xsd:string ;
      owl:onProperty airs:hasExplanationForNoPhysicalAddress ;
    ] ;
  rdfs:subClassOf [
      rdf:type owl:Restriction ;
      owl:allValuesFrom airs:ResourceInfo ;
      owl:onProperty airs:hasResourceInfo ;
    ] ;
.
airs:Address_1
  rdf:type owl:NamedIndividual ;
  rdf:type airs:Address ;
  dct:description "Esta es la dirección principal de esta agencia."@es ;
  dct:description "This is the main address for this agency."@en ;
  vcard:country-name "United States of America"@en ;
  vcard:locality "Marietta"@en ;
  vcard:postal-code "30008"^^xsd:string ;
  vcard:region "Georgia"@en ;
  vcard:street-address "331 Main Street"^^xsd:string ;
  airs:hasResourceInfo :ResourceInfo_1 ;
  airs:isMailingAddress "true"^^xsd:boolean ;
  airs:isPhysicalAddress "true"^^xsd:boolean ;
.
airs:Agency
  rdf:type owl:Class ;
  rdfs:comment "Agencies are organizations that offer services at locations. Agencies provide services directly or they may have \"child\" agencies that offer these services. Services are offered at sites that belong to an agency. Services are represented by the combination of taxonomy codes offered at a location; this idea is called a SiteService. To recap: Agencies don't provide services directly, they provide them through sites. For property <http://www.w3.org/2006/vcard/ns:hasRelated> This represents the agency contact.  1) Contact is the person at an Agency, or Site who will interface with the public or who has responsibility for the entity, like a site manager or director."@en ;
  rdfs:label "Agence"@fr ;
  rdfs:label "Agencia"@es ;
  rdfs:label "Agency"@en ;
  rdfs:subClassOf org:FormalOrganization ;
  rdfs:subClassOf [
      rdf:type owl:Restriction ;
      owl:allValuesFrom xsd:boolean ;
      owl:onProperty airs:excludesFromDirectory ;
    ] ;
  rdfs:subClassOf [
      rdf:type owl:Restriction ;
      owl:allValuesFrom xsd:boolean ;
      owl:onProperty airs:excludesFromWebsite ;
    ] ;
  rdfs:subClassOf [
      rdf:type owl:Restriction ;
      owl:allValuesFrom xsd:gYear ;
      owl:onProperty airs:hasYearIncorporated ;
    ] ;
  rdfs:subClassOf [
      rdf:type owl:Restriction ;
      owl:allValuesFrom xsd:string ;
      owl:onProperty dct:description ;
    ] ;
  rdfs:subClassOf [
      rdf:type owl:Restriction ;
      owl:allValuesFrom xsd:string ;
      owl:onProperty vcard:organization-name ;
    ] ;
  rdfs:subClassOf [
      rdf:type owl:Restriction ;
      owl:allValuesFrom xsd:string ;
      owl:onProperty vcard:url ;
    ] ;
  rdfs:subClassOf [
      rdf:type owl:Restriction ;
      owl:allValuesFrom xsd:string ;
      owl:onProperty airs:hasFEIN ;
    ] ;
  rdfs:subClassOf [
      rdf:type owl:Restriction ;
      owl:allValuesFrom xsd:string ;
      owl:onProperty airs:hasLegalStatus ;
    ] ;
  rdfs:subClassOf [
      rdf:type owl:Restriction ;
      owl:allValuesFrom xsd:string ;
      owl:onProperty airs:hasRecordOwner ;
    ] ;
  rdfs:subClassOf [
      rdf:type owl:Restriction ;
      owl:allValuesFrom vcard:Contact ;
      owl:onProperty vcard:hasRelated ;
    ] ;
  rdfs:subClassOf [
      rdf:type owl:Restriction ;
      owl:allValuesFrom vcard:Email ;
      owl:onProperty vcard:hasEmail ;
    ] ;
  rdfs:subClassOf [
      rdf:type owl:Restriction ;
      owl:allValuesFrom vcard:TelephoneType ;
      owl:onProperty vcard:hasTelephone ;
    ] ;
  rdfs:subClassOf [
      rdf:type owl:Restriction ;
      owl:allValuesFrom airs:AlternateName ;
      owl:onProperty airs:hasAlternateName ;
    ] ;
  rdfs:subClassOf [
      rdf:type owl:Restriction ;
      owl:allValuesFrom airs:InternetResource ;
      owl:onProperty airs:hasInternetResource ;
    ] ;
  rdfs:subClassOf [
      rdf:type owl:Restriction ;
      owl:allValuesFrom airs:LicenseAccreditation ;
      owl:onProperty airs:hasLicenseAccreditation ;
    ] ;
  rdfs:subClassOf [
      rdf:type owl:Restriction ;
      owl:allValuesFrom airs:ResourceInfo ;
      owl:onProperty airs:hasResourceInfo ;
    ] ;
  rdfs:subClassOf [
      rdf:type owl:Restriction ;
      owl:allValuesFrom airs:Service ;
      owl:onProperty airs:offersService ;
    ] ;
  rdfs:subClassOf [
      rdf:type owl:Restriction ;
      owl:allValuesFrom airs:ServiceGroup ;
      owl:onProperty airs:hasServiceGroup ;
    ] ;
  rdfs:subClassOf [
      rdf:type owl:Restriction ;
      owl:maxCardinality "1"^^xsd:nonNegativeInteger ;
      owl:onProperty airs:hasStatus ;
    ] ;
.
airs:Agency_1
  rdf:type owl:NamedIndividual ;
  rdf:type airs:Agency ;
  dct:description "The community clinic provides basic health care for members of the community."@en ;
  vcard:hasRelated vcard:Contact_1 ;
  vcard:hasTelephone :Voice_1 ;
  vcard:organization-name "The Community Clinic"@en ;
  vcard:url "http://community_clinic.com"^^xsd:string ;
  org:hasSite airs:Site_1 ;
  airs:excludesFromDirectory "false"^^xsd:boolean ;
  airs:excludesFromWebsite "true"^^xsd:boolean ;
  airs:hasAlternateName airs:AlternateName_1 ;
  airs:hasFEIN "12345"^^xsd:string ;
  airs:hasInternetResource airs:InternetResource_1 ;
  airs:hasLegalStatus "incorporated 501c3"^^xsd:string ;
  airs:hasLicenseAccreditation airs:LicenseAccreditation_1 ;
  airs:hasRecordOwner "Jim Smith"^^xsd:string ;
  airs:hasResourceInfo :ResourceInfo_1 ;
  airs:hasServiceGroup :ServiceGroup_1 ;
  airs:hasStatus "active"^^xsd:string ;
  airs:hasYearIncorporated "1970"^^xsd:gYear ;
  airs:offersService airs:Service_1 ;
.
airs:AlternateName
  rdf:type owl:Class ;
  rdfs:subClassOf owl:Thing ;
  rdfs:subClassOf [
      rdf:type owl:Restriction ;
      owl:allValuesFrom xsd:boolean ;
      owl:onProperty airs:isConfidential ;
    ] ;
  rdfs:subClassOf [
      rdf:type owl:Restriction ;
      owl:allValuesFrom xsd:string ;
      owl:onProperty dct:description ;
    ] ;
  rdfs:subClassOf [
      rdf:type owl:Restriction ;
      owl:allValuesFrom xsd:string ;
      owl:onProperty dct:title ;
    ] ;
.
airs:AlternateName_1
  rdf:type owl:NamedIndividual ;
  rdf:type airs:AlternateName ;
  dct:description "The locals call it this."^^xsd:string ;
  dct:title "Clinic by the Bridge"^^xsd:string ;
  airs:isConfidential "false"^^xsd:boolean ;
.
airs:ApplicationProcess
  rdf:type owl:Class ;
  rdfs:comment "ApplicationProcess describes the steps taken to apply for or access the service; also known as the 'intake process'. For example, \"Call for an appointment\" or \"Walk in only\"."@en ;
  rdfs:subClassOf owl:Thing ;
  rdfs:subClassOf [
      rdf:type owl:Restriction ;
      owl:allValuesFrom xsd:string ;
      owl:onProperty dct:description ;
    ] ;
  rdfs:subClassOf [
      rdf:type owl:Restriction ;
      owl:allValuesFrom xsd:string ;
      owl:onProperty dct:title ;
    ] ;
.
airs:ApplicationProcess_1
  rdf:type airs:ApplicationProcess ;
  dct:description "The prospective enrollee must have their income verified."@en ;
  dct:title "income verification"@en ;
.
airs:Document
  rdf:type owl:Class ;
  rdfs:comment "A document that is required in order to access services offered at a SiteService."@en ;
  rdfs:subClassOf owl:Thing ;
  rdfs:subClassOf [
      rdf:type owl:Restriction ;
      owl:allValuesFrom xsd:string ;
      owl:onProperty dct:description ;
    ] ;
  rdfs:subClassOf [
      rdf:type owl:Restriction ;
      owl:allValuesFrom xsd:string ;
      owl:onProperty dct:title ;
    ] ;
.
airs:Document_1
  rdf:type airs:Document ;
  dct:description "A valid State of Georgia Driver's License."@en ;
  dct:title "driver's license"@en ;
.
airs:GenderRequirement
  rdf:type owl:Class ;
  rdfs:subClassOf owl:Thing ;
  rdfs:subClassOf [
      rdf:type owl:Restriction ;
      owl:allValuesFrom appearances:GenderStrict ;
      owl:onProperty airs:requiresGender ;
    ] ;
  rdfs:subClassOf [
      rdf:type owl:Restriction ;
      owl:allValuesFrom xsd:nonNegativeInteger ;
      owl:onProperty airs:requiresMaximumAge ;
    ] ;
  rdfs:subClassOf [
      rdf:type owl:Restriction ;
      owl:allValuesFrom xsd:nonNegativeInteger ;
      owl:onProperty airs:requiresMinimumAge ;
    ] ;
.
airs:GenderRequirement_1
  rdf:type airs:GenderRequirement ;
  airs:requiresGender <http://rdf.muninn-project.org/ontologies/organization#GenderStrict-M> ;
  airs:requiresMinimumAge "0"^^xsd:nonNegativeInteger ;
.
airs:InternetResource
  rdf:type owl:Class ;
  rdfs:comment "A web location that has more information related to the SiteService, Agency, etc..  For example a facebook page for the Agency, that is supplementary to the Agency's main website."@en ;
  rdfs:subClassOf owl:Thing ;
  rdfs:subClassOf [
      rdf:type owl:Restriction ;
      owl:allValuesFrom xsd:string ;
      owl:onProperty dct:description ;
    ] ;
  rdfs:subClassOf [
      rdf:type owl:Restriction ;
      owl:allValuesFrom xsd:string ;
      owl:onProperty vcard:url ;
    ] ;
.
airs:InternetResource_1
  rdf:type airs:InternetResource ;
  dct:description "A facebook page that the clinic keeps to maintain a social media presence."^^xsd:string ;
  vcard:url "http://facebook.com/community_clinic"^^xsd:string ;
.
airs:InternetResource_2
  rdf:type airs:InternetResource ;
  dct:description "A twitter page that the clinic keeps to maintain a social media presence."^^xsd:string ;
  vcard:url "http://twitter.com/community_clinic"^^xsd:string ;
.
airs:LanguageAvailability
  rdf:type owl:Class ;
  rdfs:comment "Languages offered, and available times, at the SiteService"@en ;
  rdfs:subClassOf owl:Thing ;
  rdfs:subClassOf [
      rdf:type owl:Restriction ;
      owl:allValuesFrom ncal:Calendar ;
      owl:onProperty airs:hasLanguageTimeOpen ;
    ] ;
  rdfs:subClassOf [
      rdf:type owl:Restriction ;
      owl:allValuesFrom xsd:string ;
      owl:onProperty dc:language ;
    ] ;
  rdfs:subClassOf [
      rdf:type owl:Restriction ;
      owl:allValuesFrom xsd:string ;
      owl:onProperty dct:description ;
    ] ;
.
airs:LanguageAvailability_1
  rdf:type airs:LanguageAvailability ;
  dc:language "French"@en ;
  dct:description "A native French speaker is often available at this location."@en ;
  airs:hasLanguageTimeOpen ncal:Calendar_1 ;
.
airs:LicenseAccreditation
  rdf:type owl:Class ;
  rdfs:comment "If applicable, information about the license type (dct:title)/accreditation held by the agency and the body that licensed/accredited it."@en ;
  rdfs:subClassOf owl:Thing ;
  rdfs:subClassOf [
      rdf:type owl:Restriction ;
      owl:allValuesFrom xsd:string ;
      owl:onProperty dct:title ;
    ] ;
  rdfs:subClassOf [
      rdf:type owl:Restriction ;
      owl:allValuesFrom xsd:string ;
      owl:onProperty airs:isLicensedBy ;
    ] ;
.
airs:LicenseAccreditation_1
  rdf:type airs:LicenseAccreditation ;
  dct:title "AIRS Resource Specialist Accreditation"^^xsd:string ;
  airs:isLicensedBy "Alliance of Information and Referral Services (AIRS)"^^xsd:string ;
.
airs:OpenHours
  rdf:type owl:Class ;
  rdfs:comment "The hours that the SiteService is open.  Can have complex schedules.  See http://tools.ietf.org/html/rfc2445."^^xsd:string ;
  rdfs:subClassOf owl:Thing ;
  rdfs:subClassOf [
      rdf:type owl:Restriction ;
      owl:allValuesFrom ncal:Calendar ;
      owl:onProperty airs:opensAtTimes ;
    ] ;
  rdfs:subClassOf [
      rdf:type owl:Restriction ;
      owl:allValuesFrom xsd:string ;
      owl:onProperty dct:description ;
    ] ;
.
airs:OpenHours_1
  rdf:type airs:OpenHours ;
  dct:description "This program is open every weekday."@en ;
  airs:opensAtTimes ncal:Calendar_2 ;
.
airs:ResourceInfo
  rdf:type owl:Class ;
  rdfs:comment "For property <http://www.w3.org/2006/vcard/ns:hasRelated>, it indicates the person within each agency who has overall responsibility for updating the information about the agency, its sites and its services, etc."@en ;
  rdfs:subClassOf owl:Thing ;
  rdfs:subClassOf [
      rdf:type owl:Restriction ;
      owl:allValuesFrom xsd:boolean ;
      owl:onProperty airs:isAvailableForDirectory ;
    ] ;
  rdfs:subClassOf [
      rdf:type owl:Restriction ;
      owl:allValuesFrom xsd:boolean ;
      owl:onProperty airs:isAvailableForReferral ;
    ] ;
  rdfs:subClassOf [
      rdf:type owl:Restriction ;
      owl:allValuesFrom xsd:boolean ;
      owl:onProperty airs:isAvailableForResearch ;
    ] ;
  rdfs:subClassOf [
      rdf:type owl:Restriction ;
      owl:allValuesFrom xsd:dateTime ;
      owl:onProperty dct:created ;
    ] ;
  rdfs:subClassOf [
      rdf:type owl:Restriction ;
      owl:allValuesFrom xsd:dateTime ;
      owl:onProperty airs:hasDateLastVerified ;
    ] ;
  rdfs:subClassOf [
      rdf:type owl:Restriction ;
      owl:allValuesFrom xsd:dateTime ;
      owl:onProperty airs:hasDateOfLastAction ;
    ] ;
  rdfs:subClassOf [
      rdf:type owl:Restriction ;
      owl:allValuesFrom xsd:string ;
      owl:onProperty airs:attributesResourceSpecialist ;
    ] ;
  rdfs:subClassOf [
      rdf:type owl:Restriction ;
      owl:allValuesFrom xsd:string ;
      owl:onProperty airs:hasLastActionType ;
    ] ;
  rdfs:subClassOf [
      rdf:type owl:Restriction ;
      owl:allValuesFrom vcard:Contact ;
      owl:onProperty vcard:hasRelated ;
    ] ;
  rdfs:subClassOf [
      rdf:type owl:Restriction ;
      owl:cardinality "1"^^xsd:nonNegativeInteger ;
      owl:onProperty dct:created ;
    ] ;
.
airs:ResourceInfo_1
  rdf:type airs:ResourceInfo ;
  dct:created "2014-06-01T00:00:00.0Z"^^xsd:dateTime ;
  airs:attributesResourceSpecialist "Donald Truman"^^xsd:string ;
  airs:hasDateLastVerified "2014-06-03T18:13:51.0Z"^^xsd:dateTime ;
  airs:hasDateOfLastAction "2014-06-07T00:00:00.0Z"^^xsd:dateTime ;
  airs:hasLastActionType "updated ZIP Code"^^xsd:string ;
  airs:isAvailableForDirectory "true"^^xsd:boolean ;
  airs:isAvailableForReferral "true"^^xsd:boolean ;
  airs:isAvailableForResearch "true"^^xsd:boolean ;
.
airs:ResourceInfo_2
  rdf:type airs:ResourceInfo ;
  dct:created "2014-06-01T00:00:00.0Z"^^xsd:dateTime ;
  airs:attributesResourceSpecialist "Angie Capers"^^xsd:string ;
  airs:hasDateLastVerified "2014-06-03T18:13:51.0Z"^^xsd:dateTime ;
  airs:hasDateOfLastAction "2014-06-07T00:00:00.0Z"^^xsd:dateTime ;
  airs:hasLastActionType "updated ZIP Code"^^xsd:string ;
  airs:isAvailableForDirectory "true"^^xsd:boolean ;
  airs:isAvailableForReferral "true"^^xsd:boolean ;
  airs:isAvailableForResearch "true"^^xsd:boolean ;
.
airs:ResourceInfo_3
  rdf:type airs:ResourceInfo ;
  dct:created "2014-06-01T00:00:00.0Z"^^xsd:dateTime ;
  airs:attributesResourceSpecialist "Billy Bigglesworth"^^xsd:string ;
  airs:hasDateLastVerified "2014-06-03T18:13:51.0Z"^^xsd:dateTime ;
  airs:hasDateOfLastAction "2014-06-07T00:00:00.0Z"^^xsd:dateTime ;
  airs:hasLastActionType "updated ZIP Code"^^xsd:string ;
  airs:isAvailableForDirectory "true"^^xsd:boolean ;
  airs:isAvailableForReferral "true"^^xsd:boolean ;
  airs:isAvailableForResearch "true"^^xsd:boolean ;
.
airs:Seasonal
  rdf:type owl:Class ;
  rdfs:comment "Activities that are only offered a certain time of year, such as seasonal tax preparation, summer camps and holiday meals."@en ;
  rdfs:subClassOf owl:Thing ;
  rdfs:subClassOf [
      rdf:type owl:Restriction ;
      owl:allValuesFrom ncal:Calendar ;
      owl:onProperty airs:hasSeasonalSchedule ;
    ] ;
  rdfs:subClassOf [
      rdf:type owl:Restriction ;
      owl:allValuesFrom xsd:boolean ;
      owl:onProperty airs:isSeasonal ;
    ] ;
  rdfs:subClassOf [
      rdf:type owl:Restriction ;
      owl:allValuesFrom xsd:string ;
      owl:onProperty dct:description ;
    ] ;
.
airs:Seasonal_1
  rdf:type airs:Seasonal ;
  dct:description "This program is available only during the month of June."@en ;
  airs:hasSeasonalSchedule ncal:Event_3 ;
  airs:isSeasonal "true"^^xsd:boolean ;
.
airs:Service
  rdf:type owl:Class ;
  rdfs:comment "Akin to a \"Program\", as in for example \"a homeless outreach program\".  Can be delivered at many \"airs:Site[s]\", and the nexus of the two is an airs:SiteService"@en ;
  rdfs:subClassOf owl:Thing ;
  rdfs:subClassOf [
      rdf:type owl:Restriction ;
      owl:allValuesFrom xsd:string ;
      owl:onProperty dct:description ;
    ] ;
  rdfs:subClassOf [
      rdf:type owl:Restriction ;
      owl:allValuesFrom airs:Agency ;
      owl:onProperty airs:hasAgency ;
    ] ;
  rdfs:subClassOf [
      rdf:type owl:Restriction ;
      owl:allValuesFrom airs:ResourceInfo ;
      owl:onProperty airs:hasResourceInfo ;
    ] ;
  rdfs:subClassOf [
      rdf:type owl:Restriction ;
      owl:allValuesFrom airs:SiteService ;
      owl:onProperty airs:hasSiteService ;
    ] ;
  rdfs:subClassOf [
      rdf:type owl:Restriction ;
      owl:maxCardinality "1"^^xsd:nonNegativeInteger ;
      owl:onProperty airs:hasStatus ;
    ] ;
  rdfs:subClassOf [
      rdf:type owl:Restriction ;
      owl:onProperty airs:hasServiceGroup ;
      owl:someValuesFrom airs:ServiceGroup ;
    ] ;
.
airs:ServiceArea
  rdf:type owl:Class ;
  rdfs:comment "This is the geographic area served by the SiteService. This can be anything from a single neighborhood to an entire country. Types can also be mixed; perhaps one city and 6 nearby ZIP codes. In this case the required element would be City and there would be additional ZIP codes. A national 1-800 hotline would have one Country element."@en ;
  rdfs:subClassOf owl:Thing ;
  rdfs:subClassOf [
      rdf:type owl:Restriction ;
      owl:allValuesFrom dct:Location ;
      owl:onProperty airs:servesGeographicArea ;
    ] ;
  rdfs:subClassOf [
      rdf:type owl:Restriction ;
      owl:allValuesFrom xsd:string ;
      owl:onProperty dct:description ;
    ] ;
  rdfs:subClassOf [
      rdf:type owl:Restriction ;
      owl:allValuesFrom xsd:string ;
      owl:onProperty airs:isInCensusTrack ;
    ] ;
.
airs:ServiceArea_1
  rdf:type airs:ServiceArea ;
  airs:isInCensusTrack "12345"^^xsd:string ;
  airs:servesGeographicArea :Location_1 ;
.
airs:ServiceGroup
  rdf:type owl:Class ;
  rdfs:comment "Groups together multiple Services that are related somehow."@en ;
  rdfs:subClassOf owl:Thing ;
  rdfs:subClassOf [
      rdf:type owl:Restriction ;
      owl:allValuesFrom xsd:string ;
      owl:onProperty dct:description ;
    ] ;
  rdfs:subClassOf [
      rdf:type owl:Restriction ;
      owl:allValuesFrom xsd:string ;
      owl:onProperty dct:title ;
    ] ;
  rdfs:subClassOf [
      rdf:type owl:Restriction ;
      owl:allValuesFrom airs:ResourceInfo ;
      owl:onProperty airs:hasResourceInfo ;
    ] ;
  rdfs:subClassOf [
      rdf:type owl:Restriction ;
      owl:allValuesFrom airs:Service ;
      owl:onProperty airs:offersService ;
    ] ;
.
airs:ServiceGroup_1
  rdf:type airs:ServiceGroup ;
.
airs:Service_1
  rdf:type airs:Service ;
  dct:description "Marrietta Regional Community Clinics"^^xsd:string ;
  airs:hasAgency airs:Agency_1 ;
  airs:hasServiceGroup :ServiceGroup_1 ;
.
airs:Site
  rdf:type owl:Class ;
  rdfs:comment "Sites are physical locations or none physical locations (a website or hotline). Site is used for two purposes. First, it is used by Agency to provide the location of the agency in Agency.AgencyLocation (note this type of Site would never have any SiteService children). Second, sites are also the location where services are provided. This would be the Agency.Site element (note this type of Site would have SiteService children)."@en ;
  rdfs:subClassOf org:Site ;
  rdfs:subClassOf [
      rdf:type owl:Restriction ;
      owl:allValuesFrom <http://purl.org/dc/terms#:description> ;
      owl:onProperty airs:hasDescription ;
    ] ;
  rdfs:subClassOf [
      rdf:type owl:Restriction ;
      owl:allValuesFrom <http://www.opengis.net/rdf#:Point> ;
      owl:onProperty airs:hasSpatialLocation ;
    ] ;
  rdfs:subClassOf [
      rdf:type owl:Restriction ;
      owl:allValuesFrom xsd:boolean ;
      owl:onProperty airs:excludesFromDirectory ;
    ] ;
  rdfs:subClassOf [
      rdf:type owl:Restriction ;
      owl:allValuesFrom xsd:boolean ;
      owl:onProperty airs:excludesFromWebsite ;
    ] ;
  rdfs:subClassOf [
      rdf:type owl:Restriction ;
      owl:allValuesFrom xsd:boolean ;
      owl:onProperty airs:isConfidential ;
    ] ;
  rdfs:subClassOf [
      rdf:type owl:Restriction ;
      owl:allValuesFrom xsd:boolean ;
      owl:onProperty airs:publicAccessToTransportation ;
    ] ;
  rdfs:subClassOf [
      rdf:type owl:Restriction ;
      owl:allValuesFrom xsd:string ;
      owl:onProperty dct:title ;
    ] ;
  rdfs:subClassOf [
      rdf:type owl:Restriction ;
      owl:allValuesFrom xsd:string ;
      owl:onProperty vcard:url ;
    ] ;
  rdfs:subClassOf [
      rdf:type owl:Restriction ;
      owl:allValuesFrom xsd:string ;
      owl:onProperty airs:describesSpatialLocation ;
    ] ;
  rdfs:subClassOf [
      rdf:type owl:Restriction ;
      owl:allValuesFrom xsd:string ;
      owl:onProperty airs:hasBusServiceAccess ;
    ] ;
  rdfs:subClassOf [
      rdf:type owl:Restriction ;
      owl:allValuesFrom xsd:string ;
      owl:onProperty airs:hasDisabilitiesAccess ;
    ] ;
  rdfs:subClassOf [
      rdf:type owl:Restriction ;
      owl:allValuesFrom xsd:string ;
      owl:onProperty airs:hasReasonAddressWithheld ;
    ] ;
  rdfs:subClassOf [
      rdf:type owl:Restriction ;
      owl:allValuesFrom xsd:string ;
      owl:onProperty airs:isLocatedAtCrossStreet ;
    ] ;
  rdfs:subClassOf [
      rdf:type owl:Restriction ;
      owl:allValuesFrom vcard:Contact ;
      owl:onProperty vcard:hasRelated ;
    ] ;
  rdfs:subClassOf [
      rdf:type owl:Restriction ;
      owl:allValuesFrom vcard:TelephoneType ;
      owl:onProperty vcard:hasTelephone ;
    ] ;
  rdfs:subClassOf [
      rdf:type owl:Restriction ;
      owl:allValuesFrom airs:Agency ;
      owl:onProperty airs:hasAgency ;
    ] ;
  rdfs:subClassOf [
      rdf:type owl:Restriction ;
      owl:allValuesFrom airs:AlternateName ;
      owl:onProperty airs:hasAlternateName ;
    ] ;
  rdfs:subClassOf [
      rdf:type owl:Restriction ;
      owl:allValuesFrom airs:InternetResource ;
      owl:onProperty airs:hasInternetResource ;
    ] ;
  rdfs:subClassOf [
      rdf:type owl:Restriction ;
      owl:allValuesFrom airs:LanguageAvailability ;
      owl:onProperty airs:hasLanguageAvailability ;
    ] ;
  rdfs:subClassOf [
      rdf:type owl:Restriction ;
      owl:allValuesFrom airs:OpenHours ;
      owl:onProperty airs:opensAtTimes ;
    ] ;
  rdfs:subClassOf [
      rdf:type owl:Restriction ;
      owl:allValuesFrom airs:ResourceInfo ;
      owl:onProperty airs:hasResourceInfo ;
    ] ;
  rdfs:subClassOf [
      rdf:type owl:Restriction ;
      owl:allValuesFrom airs:Seasonal ;
      owl:onProperty airs:hasSeasonalSchedule ;
    ] ;
  rdfs:subClassOf [
      rdf:type owl:Restriction ;
      owl:allValuesFrom airs:SiteService ;
      owl:onProperty airs:hasSiteService ;
    ] ;
  rdfs:subClassOf [
      rdf:type owl:Restriction ;
      owl:cardinality "1"^^xsd:nonNegativeInteger ;
      owl:onProperty airs:hasAgency ;
    ] ;
  rdfs:subClassOf [
      rdf:type owl:Restriction ;
      owl:maxCardinality "1"^^xsd:nonNegativeInteger ;
      owl:onProperty airs:hasStatus ;
    ] ;
  rdfs:subClassOf [
      rdf:type owl:Restriction ;
      owl:maxCardinality "1"^^xsd:nonNegativeInteger ;
      owl:onProperty airs:isConfidential ;
    ] ;
.
airs:SiteService
  rdf:type owl:Class ;
  rdfs:comment "SiteService is the smallest unit describing a \"service\" that is offered at a Site. It can be thought of as the intersection of a Site and a Taxonomy code (or related Taxonomy codes) and meta data about what is offered. A \"Service\" however is not represented as its own element because the \"Service\" cannot exist without a location (the site)."@en ;
  rdfs:subClassOf owl:Thing ;
  rdfs:subClassOf [
      rdf:type owl:Restriction ;
      owl:allValuesFrom xsd:boolean ;
      owl:onProperty airs:isNotAlwaysAvailable ;
    ] ;
  rdfs:subClassOf [
      rdf:type owl:Restriction ;
      owl:allValuesFrom xsd:string ;
      owl:onProperty dct:description ;
    ] ;
  rdfs:subClassOf [
      rdf:type owl:Restriction ;
      owl:allValuesFrom xsd:string ;
      owl:onProperty dct:title ;
    ] ;
  rdfs:subClassOf [
      rdf:type owl:Restriction ;
      owl:allValuesFrom xsd:string ;
      owl:onProperty airs:acceptsPaymentMethod ;
    ] ;
  rdfs:subClassOf [
      rdf:type owl:Restriction ;
      owl:allValuesFrom xsd:string ;
      owl:onProperty airs:hasTaxonomyCode ;
    ] ;
  rdfs:subClassOf [
      rdf:type owl:Restriction ;
      owl:allValuesFrom xsd:string ;
      owl:onProperty airs:requiresFamily ;
    ] ;
  rdfs:subClassOf [
      rdf:type owl:Restriction ;
      owl:allValuesFrom xsd:string ;
      owl:onProperty airs:requiresGeneralEligibility ;
    ] ;
  rdfs:subClassOf [
      rdf:type owl:Restriction ;
      owl:allValuesFrom xsd:string ;
      owl:onProperty airs:requiresIncome ;
    ] ;
  rdfs:subClassOf [
      rdf:type owl:Restriction ;
      owl:allValuesFrom xsd:string ;
      owl:onProperty airs:requiresResidency ;
    ] ;
  rdfs:subClassOf [
      rdf:type owl:Restriction ;
      owl:allValuesFrom xsd:string ;
      owl:onProperty airs:structuresFees ;
    ] ;
  rdfs:subClassOf [
      rdf:type owl:Restriction ;
      owl:allValuesFrom vcard:TelephoneType ;
      owl:onProperty vcard:hasTelephone ;
    ] ;
  rdfs:subClassOf [
      rdf:type owl:Restriction ;
      owl:allValuesFrom airs:Address ;
      owl:onProperty airs:hasAddress ;
    ] ;
  rdfs:subClassOf [
      rdf:type owl:Restriction ;
      owl:allValuesFrom airs:ApplicationProcess ;
      owl:onProperty airs:hasApplicationProcess ;
    ] ;
  rdfs:subClassOf [
      rdf:type owl:Restriction ;
      owl:allValuesFrom airs:Document ;
      owl:onProperty airs:requiresDocument ;
    ] ;
  rdfs:subClassOf [
      rdf:type owl:Restriction ;
      owl:allValuesFrom airs:GenderRequirement ;
      owl:onProperty airs:hasGenderRequirement ;
    ] ;
  rdfs:subClassOf [
      rdf:type owl:Restriction ;
      owl:allValuesFrom airs:InternetResource ;
      owl:onProperty airs:hasInternetResource ;
    ] ;
  rdfs:subClassOf [
      rdf:type owl:Restriction ;
      owl:allValuesFrom airs:LanguageAvailability ;
      owl:onProperty airs:hasLanguageAvailability ;
    ] ;
  rdfs:subClassOf [
      rdf:type owl:Restriction ;
      owl:allValuesFrom airs:LanguageAvailability ;
      owl:onProperty airs:offersSpokenLanguage ;
    ] ;
  rdfs:subClassOf [
      rdf:type owl:Restriction ;
      owl:allValuesFrom airs:ResourceInfo ;
      owl:onProperty airs:hasResourceInfo ;
    ] ;
  rdfs:subClassOf [
      rdf:type owl:Restriction ;
      owl:allValuesFrom airs:Service ;
      owl:onProperty airs:offersService ;
    ] ;
  rdfs:subClassOf [
      rdf:type owl:Restriction ;
      owl:allValuesFrom airs:ServiceArea ;
      owl:onProperty airs:servesGeographicArea ;
    ] ;
  rdfs:subClassOf [
      rdf:type owl:Restriction ;
      owl:allValuesFrom airs:Site ;
      owl:onProperty airs:hasSite ;
    ] ;
  rdfs:subClassOf [
      rdf:type owl:Restriction ;
      owl:maxCardinality "1"^^xsd:nonNegativeInteger ;
      owl:onProperty airs:hasStatus ;
    ] ;
.
airs:SiteService_1
  rdf:type owl:NamedIndividual ;
  rdf:type airs:SiteService ;
  dct:description "This is a new service location on Main Street."@en ;
  dct:title "The Community Clinic Main Street Annex"@en ;
  vcard:hasTelephone :Voice_2 ;
  airs:acceptsPaymentMethod "Medicaid"^^xsd:string ;
  airs:hasAddress airs:Address_1 ;
  airs:hasApplicationProcess airs:ApplicationProcess_1 ;
  airs:hasGenderRequirement airs:GenderRequirement_1 ;
  airs:hasInternetResource airs:InternetResource_2 ;
  airs:hasLanguageAvailability airs:LanguageAvailability_1 ;
  airs:hasResourceInfo :ResourceInfo_2 ;
  airs:hasSite airs:Site_1 ;
  airs:hasStatus "active"^^xsd:string ;
  airs:hasTaxonomyCode "AB-123"^^xsd:string ;
  airs:hasTaxonomyCode "CD-345"^^xsd:string ;
  airs:isInCensusTrack "3452"^^xsd:string ;
  airs:isNotAlwaysAvailable "false"^^xsd:boolean ;
  airs:offersService airs:Service_1 ;
  airs:offersSpokenLanguage airs:LanguageAvailability_1 ;
  airs:requiresDocument airs:Document_1 ;
  airs:requiresFamily "Family is encouraged to enroll."@en ;
  airs:requiresGeneralEligibility "Must be receiving Medicaid."@en ;
  airs:requiresIncome "Must be at 150% of poverty level."@en ;
  airs:requiresResidency "Must be a resident of Marietta."@en ;
  airs:servesGeographicArea :ServiceArea_1 ;
.
airs:Site_1
  rdf:type owl:NamedIndividual ;
  rdf:type airs:Site ;
  org:siteOf airs:Agency_1 ;
  airs:hasStatus "active"^^xsd:string ;
.
airs:acceptsPaymentMethod
  rdf:type owl:DatatypeProperty ;
.
airs:attributesResourceSpecialist
  rdf:type owl:DatatypeProperty ;
.
airs:describesInternetResource
  rdf:type owl:DatatypeProperty ;
  rdfs:subPropertyOf airs:hasInternetResource ;
.
airs:describesPhysicalLocation
  rdf:type owl:DatatypeProperty ;
.
airs:describesSpatialLocation
  rdf:type owl:DatatypeProperty ;
  rdfs:subPropertyOf airs:hasSpatialLocation ;
.
airs:excludesFromDirectory
  rdf:type owl:DatatypeProperty ;
.
airs:excludesFromWebsite
  rdf:type owl:DatatypeProperty ;
  rdfs:range xsd:boolean ;
.
airs:explainsNoPhysicalAddress
  rdf:type owl:DatatypeProperty ;
.
airs:hasAddress
  rdf:type owl:ObjectProperty ;
.
airs:hasAgency
  rdf:type owl:ObjectProperty ;
.
airs:hasAlternateName
  rdf:type owl:ObjectProperty ;
  rdfs:comment "These are alternate names for an object. Confidential indicates that the alternate name won't be shared with the public."@en ;
.
airs:hasApplicationProcess
  rdf:type owl:ObjectProperty ;
.
airs:hasAreaDefinition
  rdf:type owl:DatatypeProperty ;
.
airs:hasBusServiceAccess
  rdf:type owl:DatatypeProperty ;
.
airs:hasDateAdded
  rdf:type owl:DatatypeProperty ;
.
airs:hasDateLastVerified
  rdf:type owl:DatatypeProperty ;
.
airs:hasDateOfLastAction
  rdf:type owl:DatatypeProperty ;
.
airs:hasDescription
  rdf:type owl:DatatypeProperty ;
  rdf:type owl:ObjectProperty ;
.
airs:hasDisabilitiesAccess
  rdf:type owl:DatatypeProperty ;
.
airs:hasExplanationForNoPhysicalAddress
  rdf:type owl:DatatypeProperty ;
.
airs:hasFEIN
  rdf:type owl:DatatypeProperty ;
.
airs:hasGenderRequirement
  rdf:type owl:ObjectProperty ;
.
airs:hasIRSStatus
  rdf:type owl:DatatypeProperty ;
.
airs:hasInternetResource
  rdf:type owl:ObjectProperty ;
.
airs:hasLanguageAvailability
  rdf:type owl:ObjectProperty ;
.
airs:hasLanguageName
  rdf:type owl:DatatypeProperty ;
.
airs:hasLanguageTimeOpen
  rdf:type owl:ObjectProperty ;
.
airs:hasLastActionType
  rdf:type owl:DatatypeProperty ;
  rdfs:comment "Describes what update action was taken to update the resource information, such as \"updated the resource specialist's name\"."^^xsd:string ;
.
airs:hasLegalStatus
  rdf:type owl:DatatypeProperty ;
.
airs:hasLicenseAccreditation
  rdf:type owl:ObjectProperty ;
.
airs:hasLicenseType
  rdf:type owl:DatatypeProperty ;
  rdf:type owl:ObjectProperty ;
.
airs:hasProgramName
  rdf:type owl:DatatypeProperty ;
.
airs:hasReasonAddressWithheld
  rdf:type owl:DatatypeProperty ;
  rdfs:comment "Use this if the address can not be shared due to security concerns, such as an assaulted women's shelter. While it is possible to code an address as Confidential=\"true\", in this case the address is so confidential that it won't be shared at all."@en ;
.
airs:hasRecordOwner
  rdf:type owl:DatatypeProperty ;
  rdfs:comment "This is a unique string indicating the organization that created and maintains this Agency record."@en ;
.
airs:hasResourceInfo
  rdf:type owl:AsymmetricProperty ;
  rdf:type owl:ObjectProperty ;
.
airs:hasSeasonalSchedule
  rdf:type owl:ObjectProperty ;
.
airs:hasServiceGroup
  rdf:type owl:AsymmetricProperty ;
  rdf:type owl:ObjectProperty ;
.
airs:hasServiceGroupName
  rdf:type owl:DatatypeProperty ;
.
airs:hasSite
  rdf:type owl:AsymmetricProperty ;
  rdf:type owl:ObjectProperty ;
.
airs:hasSiteService
  rdf:type owl:ObjectProperty ;
.
airs:hasSpatialLocation
  rdf:type owl:DatatypeProperty ;
  rdf:type owl:ObjectProperty ;
.
airs:hasStatus
  rdf:type owl:DatatypeProperty ;
  rdfs:range [
      rdf:type rdfs:Datatype ;
      owl:oneOf [
          rdf:type rdf:List ;
          rdf:first "active"^^xsd:string ;
          rdf:rest [
              rdf:type rdf:List ;
              rdf:first "defunct"^^xsd:string ;
              rdf:rest [
                  rdf:type rdf:List ;
                  rdf:first "inactive"^^xsd:string ;
                  rdf:rest () ;
                ] ;
            ] ;
        ] ;
    ] ;
.
airs:hasTaxonomyCode
  rdf:type owl:DatatypeProperty ;
.
airs:hasTelephone
  rdf:type owl:DatatypeProperty ;
  rdf:type owl:ObjectProperty ;
.
airs:hasYearIncorporated
  rdf:type owl:DatatypeProperty ;
.
airs:isAvailableForDirectory
  rdf:type owl:DatatypeProperty ;
.
airs:isAvailableForReferral
  rdf:type owl:DatatypeProperty ;
.
airs:isAvailableForResearch
  rdf:type owl:DatatypeProperty ;
.
airs:isConfidential
  rdf:type owl:DatatypeProperty ;
.
airs:isInCensusTrack
  rdf:type owl:DatatypeProperty ;
.
airs:isLicensedBy
  rdf:type owl:DatatypeProperty ;
.
airs:isLocatedAtCrossStreet
  rdf:type owl:DatatypeProperty ;
.
airs:isLocatedInCity
  rdf:type owl:DatatypeProperty ;
  rdfs:subPropertyOf airs:servesGeographicArea ;
.
airs:isLocatedInCounty
  rdf:type owl:DatatypeProperty ;
  rdfs:subPropertyOf airs:servesGeographicArea ;
.
airs:isLocatedInPostalCode
  rdf:type owl:DatatypeProperty ;
  rdfs:subPropertyOf airs:servesGeographicArea ;
.
airs:isLocatedInState
  rdf:type owl:DatatypeProperty ;
  rdfs:subPropertyOf airs:servesGeographicArea ;
.
airs:isLocatedWithinCountry
  rdf:type owl:DatatypeProperty ;
  rdfs:subPropertyOf airs:servesGeographicArea ;
.
airs:isMailingAddress
  rdf:type owl:DatatypeProperty ;
.
airs:isNotAlwaysAvailable
  rdf:type owl:DatatypeProperty ;
.
airs:isPhysicalAddress
  rdf:type owl:DatatypeProperty ;
  rdfs:range xsd:boolean ;
.
airs:isSeasonal
  rdf:type owl:DatatypeProperty ;
.
airs:offersLanguage
  rdf:type owl:ObjectProperty ;
.
airs:offersService
  rdf:type owl:ObjectProperty ;
.
airs:offersSpokenLanguage
  rdf:type owl:ObjectProperty ;
.
airs:opensAtTimes
  rdf:type owl:ObjectProperty ;
.
airs:opensAtTimesNotes
  rdf:type owl:DatatypeProperty ;
  rdf:type owl:ObjectProperty ;
.
airs:publicAccessToTransportation
  rdf:type owl:DatatypeProperty ;
.
airs:requiresDocument
  rdf:type owl:ObjectProperty ;
.
airs:requiresFamily
  rdf:type owl:DatatypeProperty ;
.
airs:requiresGender
  rdf:type owl:ObjectProperty ;
  rdfs:comment "Information about any age or gender related requirements or inclusions for a particular service at a particular location."@en ;
.
airs:requiresGeneralEligibility
  rdf:type owl:DatatypeProperty ;
  rdfs:comment "General eligibility is a text area to list any eligibility requirements for participation or services. This can include any exclusions, both negative and positive requirements (i.e. must have/ can't have are all requirements)"@en ;
.
airs:requiresIncome
  rdf:type owl:DatatypeProperty ;
.
airs:requiresMaximumAge
  rdf:type owl:DatatypeProperty ;
  rdfs:subPropertyOf airs:requiresGender ;
.
airs:requiresMinimumAge
  rdf:type owl:DatatypeProperty ;
  rdfs:subPropertyOf airs:requiresGender ;
.
airs:requiresResidency
  rdf:type owl:DatatypeProperty ;
.
airs:servesGeographicArea
  rdf:type owl:DatatypeProperty ;
  rdf:type owl:ObjectProperty ;
.
airs:structuresFees
  rdf:type owl:DatatypeProperty ;
.
